@prefix DnD5eCharacter: <https://w3id.org/DnD5eCharacter#> .
@prefix cc: <http://creativecommons.org/ns#> .
@prefix dct: <http://purl.org/dc/terms/> .
@prefix foaf: <http://xmlns.com/foaf/0.1/> .
@prefix owl: <http://www.w3.org/2002/07/owl#> .
@prefix rdf: <http://www.w3.org/1999/02/22-rdf-syntax-ns#> .
@prefix rdfs: <http://www.w3.org/2000/01/rdf-schema#> .
@prefix xsd: <http://www.w3.org/2001/XMLSchema#> .
@prefix TTRpg: <https://w3id.org/TTRpg#> .

DnD5eCharacter:	a foaf:Document ;
				foaf:primaryTopic DnD5eCharacter:Ontology;
				cc:license <http://creativecommons.org/licenses/by/4.0/>;
				dct:creator <https://rwambacq.solidweb.org/profile/card#me>.

<https://rwambacq.solidweb.org/profile/card#me> foaf:name "Ruben Wambacq"; foaf:mbox "ruben.wambacq@gmail.com".

DnD5eCharacter:Ontology a owl:Ontology ;
						rdfs:label "Dungeons & Dragons Fifth Edition Character"@en ;
						rdfs:comment "An extension to the TTRpg ontology, that includes every aspect of the game Dungeons & Dragons required for creating a character (only the freely available information has been included)."@en ;
            DnD5eCharacter:version "1.0.0" .

### Ontology Classes

## D&D Races

DnD5eCharacter:Race 	a rdfs:Class ;
						rdfs:subClassOf TTRpg:CharacterType ;
						rdfs:label "Race"@en ;
						rdfs:comment "A DnD5eCharacter:Race is the superclass that represents the concept of a race within Dungeons and Dragons. Every TTRpg:Character, playable or not, has a race."@en .

DnD5eCharacter:Dragonborn 	a rdfs:Class ;
              rdfs:subClassOf DnD5eCharacter:Race ;
              rdfs:label "Dragonborn"@en ;
              rdfs:comment "The dragonborn walk proudly through a world that greets them with fearful incomprehension. Shaped by the dragons themselves, dragonborn originally hatched from dragon eggs as a unique race, combining the best attributes of dragons and humanoids."@en .

DnD5eCharacter:Gnome 	a rdfs:Class ;
              rdfs:subClassOf DnD5eCharacter:Race ;
              rdfs:label "Gnome"@en ;
              rdfs:comment "A constant hum of busy activity pervades the warrens and neighborhoods where gnomes form their close-knit communities. Louder sounds punctuate the hum: a crunch of grinding gears here, a minor explosion there, a yelp of surprise or triumph, and especially bursts of laughter. Gnomes take delight in life, enjoying every moment of invention, exploration, investigation, creation, and play."@en .

DnD5eCharacter:Halfling 	a rdfs:Class ;
              rdfs:subClassOf DnD5eCharacter:Race ;
              rdfs:label "Halfling"@en ;
              rdfs:comment "The comforts of home are the goals of most halflings' lives: a place to settle in peace and quiet, far from marauding monsters and clashing armies. Others form nomadic bands that travel constantly, lured by the open road and the wide horizon to discover the wonders of new lands and peoples. Halflings work readily with others, and they are loyal to their friends, whether halfling or otherwise. They can display remarkable ferocity when their friends, families, or communities are threatened."@en .

DnD5eCharacter:Dwarf 	a rdfs:Class ;
              rdfs:subClassOf DnD5eCharacter:Race ;
              rdfs:label "Dwarf"@en ;
              rdfs:comment "Kingdoms rich in ancient grandeur, halls carved into the roots of mountains, the echoing of picks and hammers in deep mines and blazing forges, a commitment to clan and tradition, and a burning hatred of goblins and orcs - these common threads unite all dwarves."@en .

DnD5eCharacter:HalfElf 	a rdfs:Class ;
              rdfs:subClassOf DnD5eCharacter:Race ;
              rdfs:label "Half-Elf"@en ;
              rdfs:comment "Walking in two worlds but truly belonging to neither, half-elves combine what some say are the best qualities of their elf and human parents: human curiosity, inventiveness, and ambition tempered by the refined senses, love of nature, and artistic tastes of the elves."@en .

DnD5eCharacter:Elf 	a rdfs:Class ;
              rdfs:subClassOf DnD5eCharacter:Race ;
              rdfs:label "Elf"@en ;
              rdfs:comment "Elves are a magical people of otherworldly grace, living in places of ethereal beauty, in the midst of ancient forests or in silvery spires glittering with faerie light, where soft music drifts through the air and gentle fragrances waft on the breeze. Elves love nature and magic, art and artistry, music and poetry."@en .

DnD5eCharacter:HalfOrc 	a rdfs:Class ;
              rdfs:subClassOf DnD5eCharacter:Race ;
              rdfs:label "Half-Orc"@en ;
              rdfs:comment "When alliances between humans and orcs are sealed by marriages, half-orcs are born. Some half-orcs rise to become proud chiefs of orc tribes, their human blood giving them an edge over their full-blooded orc rivals. Some venture into the world to prove their worth among humans and other more civilized races. Many of these become adventurers, achieving greatness for their mighty deeds and notoriety for their barbaric customs and savage fury."@en .

DnD5eCharacter:Tiefling 	a rdfs:Class ;
              rdfs:subClassOf DnD5eCharacter:Race ;
              rdfs:label "Tiefling"@en ;
              rdfs:comment "To be greeted with stares and whispers, to suffer violence and insult on the street, to see mistrust and fear in every eye: this is the lot of the tiefling. And to twist the knife, tieflings know that this is because a pact struck generations ago infused the essence of Asmodeus, overlord of the Nine Hells (and many of the other powerful devils serving under him) into their bloodline. Their appearance and their nature are not their fault but the result of an ancient sin, for which they and their children and their children's children will always be held accountable."@en .

## D&D Subraces

DnD5eCharacter:Subrace 	a rdfs:Class ;
													rdfs:label "Subrace"@en ;
													rdfs:comment "A DnD5eCharacter:Subrace is the superclass that represents the concept of a subrace within Dungeons and Dragons. This further specifies the race of a character. Not every race has subraces tied to it."@en .

DnD5eCharacter:DraconicAncestry a rdfs:Class ;
              rdfs:subClassOf DnD5eCharacter:Subrace ;
              DnD5eCharacter:subraceOf DnD5eCharacter:Dragonborn ;
              rdfs:label "Draconic Ancestry"@en .

DnD5eCharacter:HillDwarf a rdfs:Class ;
              rdfs:subClassOf DnD5eCharacter:Subrace ;
              DnD5eCharacter:subraceOf DnD5eCharacter:Dwarf ;
              rdfs:label "Hill Dwarf"@en .

DnD5eCharacter:HighElf a rdfs:Class ;
              rdfs:subClassOf DnD5eCharacter:Subrace ;
              DnD5eCharacter:subraceOf DnD5eCharacter:Elf ;
              rdfs:label "High Elf"@en .

DnD5eCharacter:RockGnome a rdfs:Class ;
              rdfs:subClassOf DnD5eCharacter:Subrace ;
              DnD5eCharacter:subraceOf DnD5eCharacter:Gnome ;
              rdfs:label "Rock Gnome"@en .

DnD5eCharacter:Lightfoot a rdfs:Class ;
              rdfs:subClassOf DnD5eCharacter:Subrace ;
              DnD5eCharacter:subraceOf DnD5eCharacter:Halfling ;
              rdfs:label "Lightfoot"@en .

DnD5eCharacter:Callshite a rdfs:Class ;
              rdfs:subClassOf DnD5eCharacter:Subrace ;
              DnD5eCharacter:subraceOf DnD5eCharacter:Human ;
              rdfs:label "Callshite"@en .

DnD5eCharacter:Chondathan a rdfs:Class ;
              rdfs:subClassOf DnD5eCharacter:Subrace ;
              DnD5eCharacter:subraceOf DnD5eCharacter:Human ;
              rdfs:label "Chondathan"@en .

DnD5eCharacter:Damaran a rdfs:Class ;
              rdfs:subClassOf DnD5eCharacter:Subrace ;
              DnD5eCharacter:subraceOf DnD5eCharacter:Human ;
              rdfs:label "Damaran"@en .

DnD5eCharacter:Illuskan a rdfs:Class ;
              rdfs:subClassOf DnD5eCharacter:Subrace ;
              DnD5eCharacter:subraceOf DnD5eCharacter:Human ;
              rdfs:label "Illuskan"@en .

DnD5eCharacter:Mulan a rdfs:Class ;
              rdfs:subClassOf DnD5eCharacter:Subrace ;
              DnD5eCharacter:subraceOf DnD5eCharacter:Human ;
              rdfs:label "Mulan"@en .

DnD5eCharacter:Rashemi a rdfs:Class ;
              rdfs:subClassOf DnD5eCharacter:Subrace ;
              DnD5eCharacter:subraceOf DnD5eCharacter:Human ;
              rdfs:label "Rashemi"@en .

DnD5eCharacter:Shou a rdfs:Class ;
              rdfs:subClassOf DnD5eCharacter:Subrace ;
              DnD5eCharacter:subraceOf DnD5eCharacter:Human ;
              rdfs:label "Shou"@en .

DnD5eCharacter:Tethyrian a rdfs:Class ;
              rdfs:subClassOf DnD5eCharacter:Subrace ;
              DnD5eCharacter:subraceOf DnD5eCharacter:Human ;
              rdfs:label "Tethyrian"@en .

DnD5eCharacter:Turami a rdfs:Class ;
              rdfs:subClassOf DnD5eCharacter:Subrace ;
              DnD5eCharacter:subraceOf DnD5eCharacter:Human ;
              rdfs:label "Turami"@en .

DnD5eCharacter:Variant 	a rdfs:Class ;
													rdfs:label "Variant"@en ;
													rdfs:comment "A DnD5eCharacter:Variant is the superclass that represents the concept of a variant within Dungeons and Dragons. This further specifies the race of a character. Not every race has variants tied to it."@en .

DnD5eCharacter:StandardHuman a rdfs:Class ;
              rdfs:subClassOf DnD5eCharacter:Variant ;
              DnD5eCharacter:variantOf DnD5eCharacter:Human ;
              rdfs:label "Standard Human"@en .

DnD5eCharacter:VariantHuman a rdfs:Class ;
              rdfs:subClassOf DnD5eCharacter:Variant ;
              DnD5eCharacter:variantOf DnD5eCharacter:Human ;
              rdfs:label "Variant Human"@en .

## D&D Classes

DnD5eCharacter:Class 	a rdfs:Class ;
						rdfs:subClassOf TTRpg:CharacterType ;
						rdfs:label "Class"@en ;
						rdfs:comment "A DnD5eCharacter:Class is the superclass that represents the concept of a class within Dungeons and Dragons. Every TTRpg:Character, playable or not, has a class."@en .

DnD5eCharacter:Barbarian 	a rdfs:Class ;
              rdfs:subClassOf DnD5eCharacter:Class ;
              rdfs:label "Barbarian"@en ;
              rdfs:comment "For some, their rage springs from a communion with fierce animal spirits. Others draw from a roiling reservoir of anger at a world full of pain. For every barbarian, rage is a power that fuels not just a battle frenzy but also uncanny reflexes, resilience, and feats of strength."@en .

DnD5eCharacter:Druid 	a rdfs:Class ;
              rdfs:subClassOf DnD5eCharacter:Class ;
              rdfs:label "Druid"@en ;
              rdfs:comment "Whether calling on the elemental forces of nature or emulating the creatures of the animal world, druids are an embodiment of nature's resilience, cunning, and fury. They claim no mastery over nature, but see themselves as extensions of nature's indomitable will."@en .

DnD5eCharacter:Paladin 	a rdfs:Class ;
              rdfs:subClassOf DnD5eCharacter:Class ;
              rdfs:label "Paladin"@en ;
              rdfs:comment "Whether sworn before a god's altar and the witness of a priest, in a sacred glade before nature spirits and fey beings, or in a moment of desperation and grief with the dead as the only witness, a paladin's oath is a powerful bond."@en .

DnD5eCharacter:Sorcerer 	a rdfs:Class ;
              rdfs:subClassOf DnD5eCharacter:Class ;
              rdfs:label "Sorcerer"@en ;
              rdfs:comment "Sorcerers carry a magical birthright conferred upon them by an exotic bloodline, some otherworldly influence, or exposure to unknown cosmic forces. No one chooses sorcery; the power chooses the sorcerer."@en .

DnD5eCharacter:Bard 	a rdfs:Class ;
              rdfs:subClassOf DnD5eCharacter:Class ;
              rdfs:label "Bard"@en ;
              rdfs:comment "Whether scholar, skald, or scoundrel, a bard weaves magic through words and music to inspire allies, demoralize foes, manipulate minds, create illusions, and even heal wounds. The bard is a master of song, speech, and the magic they contain."@en .

DnD5eCharacter:Fighter 	a rdfs:Class ;
              rdfs:subClassOf DnD5eCharacter:Class ;
              rdfs:label "Fighter"@en ;
              rdfs:comment "Fighters share an unparalleled mastery with weapons and armor, and a thorough knowledge of the skills of combat. They are well acquainted with death, both meting it out and staring it defiantly in the face."@en .

DnD5eCharacter:Ranger 	a rdfs:Class ;
              rdfs:subClassOf DnD5eCharacter:Class ;
              rdfs:label "Ranger"@en ;
              rdfs:comment "Far from the bustle of cities and towns, past the hedges that shelter the most distant farms from the terrors of the wild, amid the dense-packed trees of trackless forests and across wide and empty plains, rangers keep their unending watch."@en .

DnD5eCharacter:Warlock 	a rdfs:Class ;
              rdfs:subClassOf DnD5eCharacter:Class ;
              rdfs:label "Warlock"@en ;
              rdfs:comment "Warlocks are seekers of the knowledge that lies hidden in the fabric of the multiverse. Through pacts made with mysterious beings of supernatural power, warlocks unlock magical effects both subtle and spectacular."@en .

DnD5eCharacter:Cleric 	a rdfs:Class ;
              rdfs:subClassOf DnD5eCharacter:Class ;
              rdfs:label "Cleric"@en ;
              rdfs:comment "Clerics are intermediaries between the mortal world and the distant planes of the gods. As varied as the gods they serve, clerics strive to embody the handiwork of their deities. No ordinary priest, a cleric is imbued with divine magic."@en .

DnD5eCharacter:Monk 	a rdfs:Class ;
              rdfs:subClassOf DnD5eCharacter:Class ;
              rdfs:label "Monk"@en ;
              rdfs:comment "Monks are united in their ability to magically harness the energy that flows in their bodies. Whether channeled as a striking display of combat prowess or a subtler focus of defensive ability and speed, this energy infuses all that a monk does."@en .

DnD5eCharacter:Rogue 	a rdfs:Class ;
              rdfs:subClassOf DnD5eCharacter:Class ;
              rdfs:label "Rogue"@en ;
              rdfs:comment "Rogues rely on skill, stealth, and their foes' vulnerabilities to get the upper hand in any situation. They have a knack for finding the solution to just about any problem, demonstrating a resourcefulness and versatility that is the cornerstone of any successful adventuring party."@en .

DnD5eCharacter:Wizard 	a rdfs:Class ;
              rdfs:subClassOf DnD5eCharacter:Class ;
              rdfs:label "Wizard"@en ;
              rdfs:comment "Wizards are supreme magic-users, defined and united as a class by the spells they cast. Drawing on the subtle weave of magic that permeates the cosmos, wizards cast spells of explosive fire, arcing lightning, subtle deception, brute-force mind control, and much more."@en .

DnD5eCharacter:ClassLevel	a rdfs:Class ;
							rdfs:label "Class Level" ;
							rdfs:comment ""@en .

DnD5eCharacter:Level	a rdfs:Class ;
						rdfs:label "Level" ;
						rdfs:comment ""@en .

## D&D Subclasses

DnD5eCharacter:Subclass 	a rdfs:Class ;
													rdfs:label "Subclass"@en ;
													rdfs:comment "A DnD5eCharacter:Subclass is the superclass that represents the concept of a subclass within Dungeons and Dragons. Every DnD5eCharacter:Class has one or more DnD5eCharacter:Subclass attached to it. These often unlock at later levels."@en .

DnD5eCharacter:PrimalPath 	a rdfs:Class ;
              rdfs:subClassOf DnD5eCharacter:Subclass ;
              DnD5eCharacter:subclassOf DnD5eCharacter:Barbarian ;
              DnD5eCharacter:unlocksAtClassLevel 3 ;
              rdfs:label "Primal Path"@en ;
              rdfs:comment "At 3rd level, you choose a path that shapes the nature of your rage."@en .

DnD5eCharacter:PathOfTheBerserker 	a rdfs:Class ;
              rdfs:subClassOf DnD5eCharacter:PrimalPath ;
              rdfs:label "Path Of The Berserker"@en .

DnD5eCharacter:DruidCircle 	a rdfs:Class ;
              rdfs:subClassOf DnD5eCharacter:Subclass ;
              DnD5eCharacter:subclassOf DnD5eCharacter:Druid ;
              DnD5eCharacter:unlocksAtClassLevel 2 ;
              rdfs:label "Druid Circle"@en ;
              rdfs:comment "At 2nd level, you choose to identify with a circle of druids."@en .

DnD5eCharacter:CircleOfTheLand 	a rdfs:Class ;
              rdfs:subClassOf DnD5eCharacter:DruidCircle ;
              rdfs:label "Circle Of The Land"@en .

DnD5eCharacter:SacredOath 	a rdfs:Class ;
              rdfs:subClassOf DnD5eCharacter:Subclass ;
              DnD5eCharacter:subclassOf DnD5eCharacter:Paladin ;
              DnD5eCharacter:unlocksAtClassLevel 3 ;
              rdfs:label "Sacred Oath"@en ;
              rdfs:comment "When you reach 3rd level, you swear the oath that binds you as a paladin forever. Up to this time you have been in a preparatory stage, committed to the path but not yet sworn to it."@en .

DnD5eCharacter:OathOfDevotion 	a rdfs:Class ;
              rdfs:subClassOf DnD5eCharacter:SacredOath ;
              rdfs:label "Oath Of Devotion"@en .

DnD5eCharacter:PaladinFightingStyle 	a rdfs:Class ;
              rdfs:subClassOf DnD5eCharacter:Subclass ;
              DnD5eCharacter:subclassOf DnD5eCharacter:Paladin ;
              DnD5eCharacter:unlocksAtClassLevel 2 ;
              rdfs:label "Paladin Fighting Style"@en ;
              rdfs:comment "Starting at 2nd level, you adopt a particular style of fighting as your specialty."@en .

DnD5eCharacter:SorcerousOrigin 	a rdfs:Class ;
              rdfs:subClassOf DnD5eCharacter:Subclass ;
              DnD5eCharacter:subclassOf DnD5eCharacter:Sorcerer ;
              DnD5eCharacter:unlocksAtClassLevel 1 ;
              rdfs:label "Sorcerous Origin"@en ;
              rdfs:comment "Choose a sorcerous origin, which describes the source of your innate magical power."@en .

DnD5eCharacter:DraconicBloodline 	a rdfs:Class ;
              rdfs:subClassOf DnD5eCharacter:SorcerousOrigin ;
              rdfs:label "Draconic Bloodline"@en .

DnD5eCharacter:BlueDragon 	a rdfs:Class ;
              rdfs:subClassOf DnD5eCharacter:DraconicAncestry ;
              rdfs:subClassOf DnD5eCharacter:DraconicBloodline ;
              rdfs:label "Blue Dragon"@en .

DnD5eCharacter:BlackDragon 	a rdfs:Class ;
              rdfs:subClassOf DnD5eCharacter:DraconicAncestry ;
              rdfs:subClassOf DnD5eCharacter:DraconicBloodline ;
              rdfs:label "Black Dragon"@en .

DnD5eCharacter:CopperDragon 	a rdfs:Class ;
              rdfs:subClassOf DnD5eCharacter:DraconicAncestry ;
              rdfs:subClassOf DnD5eCharacter:DraconicBloodline ;
              rdfs:label "Copper Dragon"@en .

DnD5eCharacter:RedDragon 	a rdfs:Class ;
              rdfs:subClassOf DnD5eCharacter:DraconicAncestry ;
              rdfs:subClassOf DnD5eCharacter:DraconicBloodline ;
              rdfs:label "Red Dragon"@en .

DnD5eCharacter:BrassDragon 	a rdfs:Class ;
              rdfs:subClassOf DnD5eCharacter:DraconicAncestry ;
              rdfs:subClassOf DnD5eCharacter:DraconicBloodline ;
              rdfs:label "Brass Dragon"@en .

DnD5eCharacter:GoldDragon 	a rdfs:Class ;
              rdfs:subClassOf DnD5eCharacter:DraconicAncestry ;
              rdfs:subClassOf DnD5eCharacter:DraconicBloodline ;
              rdfs:label "Gold Dragon"@en .

DnD5eCharacter:SilverDragon 	a rdfs:Class ;
              rdfs:subClassOf DnD5eCharacter:DraconicAncestry ;
              rdfs:subClassOf DnD5eCharacter:DraconicBloodline ;
              rdfs:label "Silver Dragon"@en .

DnD5eCharacter:BronzeDragon 	a rdfs:Class ;
              rdfs:subClassOf DnD5eCharacter:DraconicAncestry ;
              rdfs:subClassOf DnD5eCharacter:DraconicBloodline ;
              rdfs:label "Bronze Dragon"@en .

DnD5eCharacter:GreenDragon 	a rdfs:Class ;
              rdfs:subClassOf DnD5eCharacter:DraconicAncestry ;
              rdfs:subClassOf DnD5eCharacter:DraconicBloodline ;
              rdfs:label "Green Dragon"@en .

DnD5eCharacter:WhiteDragon 	a rdfs:Class ;
              rdfs:subClassOf DnD5eCharacter:DraconicAncestry ;
              rdfs:subClassOf DnD5eCharacter:DraconicBloodline ;
              rdfs:label "White Dragon"@en .

DnD5eCharacter:MetaMagic 	a rdfs:Class ;
              rdfs:subClassOf DnD5eCharacter:Subclass ;
              DnD5eCharacter:subclassOf DnD5eCharacter:Sorcerer ;
              DnD5eCharacter:unlocksAtClassLevel 3 ;
              rdfs:label "Meta Magic"@en ;
              rdfs:comment "At 3rd level, you gain the ability to twist your spells to suit your needs. You gain two Metamagic options of your choice."@en .

DnD5eCharacter:CarefulSpell 	a rdfs:Class ;
              rdfs:subClassOf DnD5eCharacter:MetaMagic ;
              rdfs:label "Careful Spell"@en .

DnD5eCharacter:HeightenedSpell 	a rdfs:Class ;
              rdfs:subClassOf DnD5eCharacter:MetaMagic ;
              rdfs:label "Heightened Spell"@en .

DnD5eCharacter:DistantSpell 	a rdfs:Class ;
              rdfs:subClassOf DnD5eCharacter:MetaMagic ;
              rdfs:label "Distant Spell"@en .

DnD5eCharacter:QuickenedSpell 	a rdfs:Class ;
              rdfs:subClassOf DnD5eCharacter:MetaMagic ;
              rdfs:label "Quickened Spell"@en .

DnD5eCharacter:EmpoweredSpell 	a rdfs:Class ;
              rdfs:subClassOf DnD5eCharacter:MetaMagic ;
              rdfs:label "Empowered Spell"@en .

DnD5eCharacter:SubtleSpell 	a rdfs:Class ;
              rdfs:subClassOf DnD5eCharacter:MetaMagic ;
              rdfs:label "Subtle Spell"@en .

DnD5eCharacter:ExtendedSpell 	a rdfs:Class ;
              rdfs:subClassOf DnD5eCharacter:MetaMagic ;
              rdfs:label "Extended Spell"@en .

DnD5eCharacter:TwinnedSpell 	a rdfs:Class ;
              rdfs:subClassOf DnD5eCharacter:MetaMagic ;
              rdfs:label "Twinned Spell"@en .

DnD5eCharacter:BardCollege 	a rdfs:Class ;
              rdfs:subClassOf DnD5eCharacter:Subclass ;
              DnD5eCharacter:subclassOf DnD5eCharacter:Bard ;
              DnD5eCharacter:unlocksAtClassLevel 3 ;
              rdfs:label "Bard College"@en ;
              rdfs:comment "At 3rd level, you delve into the advanced techniques of a bard college of your choice. "@en .

DnD5eCharacter:CollegeOfLore 	a rdfs:Class ;
              rdfs:subClassOf DnD5eCharacter:BardCollege ;
              rdfs:label "College Of Lore"@en .

DnD5eCharacter:FightingStyle  a rdfs:Class ;
              rdfs:label "Fighting Style" ;
              rdfs:comment "Abilities that give martial combatants an edge in battle. "@en .

DnD5eCharacter:FighterFightingStyle 	a rdfs:Class ;
              rdfs:subClassOf DnD5eCharacter:Subclass ;
              DnD5eCharacter:subclassOf DnD5eCharacter:Fighter ;
              DnD5eCharacter:unlocksAtClassLevel 1 ;
              rdfs:label "Fighter Fighting Style"@en ;
              rdfs:comment "You adopt a particular style of fighting as your specialty."@en .

DnD5eCharacter:Archery 	a rdfs:Class ;
              rdfs:subClassOf DnD5eCharacter:FightingStyle ;
              rdfs:subClassOf DnD5eCharacter:FighterFightingStyle ;
              rdfs:subClassOf DnD5eCharacter:RangerFightingStyle ;
              rdfs:label "Archery"@en .

DnD5eCharacter:Defense 	a rdfs:Class ;
              rdfs:subClassOf DnD5eCharacter:FightingStyle ;
              rdfs:subClassOf DnD5eCharacter:FighterFightingStyle ;
              rdfs:subClassOf DnD5eCharacter:RangerFightingStyle ;
              rdfs:subClassOf DnD5eCharacter:PaladinFightingStyle ;
              rdfs:label "Defense"@en .

DnD5eCharacter:Dueling 	a rdfs:Class ;
              rdfs:subClassOf DnD5eCharacter:FightingStyle ;
              rdfs:subClassOf DnD5eCharacter:FighterFightingStyle ;
              rdfs:subClassOf DnD5eCharacter:RangerFightingStyle ;
              rdfs:subClassOf DnD5eCharacter:PaladinFightingStyle ;
              rdfs:label "Dueling"@en .

DnD5eCharacter:GreatWeaponFighting 	a rdfs:Class ;
              rdfs:subClassOf DnD5eCharacter:FightingStyle ;
              rdfs:subClassOf DnD5eCharacter:FighterFightingStyle ;
              rdfs:subClassOf DnD5eCharacter:PaladinFightingStyle ;
              rdfs:label "Great Weapon Fighting"@en .

DnD5eCharacter:Protection 	a rdfs:Class ;
              rdfs:subClassOf DnD5eCharacter:FightingStyle ;
              rdfs:subClassOf DnD5eCharacter:FighterFightingStyle ;
              rdfs:subClassOf DnD5eCharacter:PaladinFightingStyle ;
              rdfs:label "Protection"@en .

DnD5eCharacter:TwoWeaponFighting 	a rdfs:Class ;
              rdfs:subClassOf DnD5eCharacter:FightingStyle ;
              rdfs:subClassOf DnD5eCharacter:FighterFightingStyle ;
              rdfs:subClassOf DnD5eCharacter:RangerFightingStyle ;
              rdfs:label "Two Weapon Fighting"@en .

DnD5eCharacter:RangerArchetype 	a rdfs:Class ;
              rdfs:subClassOf DnD5eCharacter:Subclass ;
              DnD5eCharacter:subclassOf DnD5eCharacter:Ranger ;
              DnD5eCharacter:unlocksAtClassLevel 3 ;
              rdfs:label "Ranger Archetype"@en ;
              rdfs:comment "At 3rd level, you choose to emulate the ideals and training of a ranger conclave."@en .

DnD5eCharacter:Hunter 	a rdfs:Class ;
              rdfs:subClassOf DnD5eCharacter:RangerArchetype ;
              rdfs:label "Hunter"@en .

DnD5eCharacter:Multiattack 	a rdfs:Class ;
              rdfs:subClassOf DnD5eCharacter:Hunter ;
              rdfs:label "Multiattack"@en .

DnD5eCharacter:Volley 	a rdfs:Class ;
              rdfs:subClassOf DnD5eCharacter:Multiattack ;
              rdfs:label "Volley"@en .

DnD5eCharacter:WhirlwindAttack 	a rdfs:Class ;
              rdfs:subClassOf DnD5eCharacter:Multiattack ;
              rdfs:label "WhirlwindAttack"@en .

DnD5eCharacter:DefensiveTactics 	a rdfs:Class ;
              rdfs:subClassOf DnD5eCharacter:Hunter ;
              rdfs:label "Defensive Tactics"@en .

DnD5eCharacter:HuntersPrey 	a rdfs:Class ;
              rdfs:subClassOf DnD5eCharacter:Hunter ;
              rdfs:label "Hunter's Prey"@en .

DnD5eCharacter:ColossusSlayer 	a rdfs:Class ;
              rdfs:subClassOf DnD5eCharacter:HuntersPrey ;
              rdfs:label "Colossus Slayer"@en .

DnD5eCharacter:HordeBreaker 	a rdfs:Class ;
              rdfs:subClassOf DnD5eCharacter:HuntersPrey ;
              rdfs:label "Horde Breaker"@en .

DnD5eCharacter:GiantKiller 	a rdfs:Class ;
              rdfs:subClassOf DnD5eCharacter:HuntersPrey ;
              rdfs:label "Giant Killer"@en .

DnD5eCharacter:SuperiorHuntersDefense 	a rdfs:Class ;
              rdfs:subClassOf DnD5eCharacter:Hunter ;
              rdfs:label "Superior Hunter's Defense"@en .

DnD5eCharacter:Evasion 	a rdfs:Class ;
              rdfs:subClassOf DnD5eCharacter:SuperiorHuntersDefense ;
              rdfs:label "Evasion"@en .

DnD5eCharacter:UncannyDodge 	a rdfs:Class ;
              rdfs:subClassOf DnD5eCharacter:SuperiorHuntersDefense ;
              rdfs:label "Uncanny Dodge"@en .

DnD5eCharacter:StandAgainstTheTide 	a rdfs:Class ;
              rdfs:subClassOf DnD5eCharacter:SuperiorHuntersDefense ;
              rdfs:label "Stand Against The Tide"@en .

DnD5eCharacter:FavoredEnemy 	a rdfs:Class ;
              rdfs:subClassOf DnD5eCharacter:Subclass ;
              DnD5eCharacter:subclassOf DnD5eCharacter:Ranger ;
              DnD5eCharacter:unlocksAtClassLevel 1 ;
              rdfs:label "Favored Enemy"@en ;
              rdfs:comment "Beginning at 1st level, you have significant experience studying, tracking, hunting, and even talking to a certain type of enemy."@en .

DnD5eCharacter:FavoredHumanoids 	a rdfs:Class ;
              rdfs:subClassOf DnD5eCharacter:FavoredEnemy ;
              DnD5eCharacter:chooseAmount 2 ;
              rdfs:label "Favored Humanoids"@en .

DnD5eCharacter:FavoredMonsterType 	a rdfs:Class ;
              rdfs:subClassOf DnD5eCharacter:FavoredEnemy ;
              rdfs:label "Favored Monster Type"@en .

DnD5eCharacter:FavoredTerrain 	a rdfs:Class ;
              rdfs:subClassOf DnD5eCharacter:Subclass ;
              DnD5eCharacter:subclassOf DnD5eCharacter:Ranger ;
              DnD5eCharacter:unlocksAtClassLevel 1 ;
              rdfs:label "Favored Terrain"@en ;
              rdfs:comment "At 1st level, you are particularly familiar with one type of natural environment and are adept at traveling and surviving in such regions."@en .

DnD5eCharacter:RangerFightingStyle 	a rdfs:Class ;
              rdfs:subClassOf DnD5eCharacter:Subclass ;
              DnD5eCharacter:subclassOf DnD5eCharacter:Ranger ;
              DnD5eCharacter:unlocksAtClassLevel 2 ;
              rdfs:label "Ranger Fighting Style"@en ;
              rdfs:comment "At 2nd level, you adopt a particular style of fighting as your specialty."@en .

DnD5eCharacter:OtherworldlyPatron 	a rdfs:Class ;
              rdfs:subClassOf DnD5eCharacter:Subclass ;
              DnD5eCharacter:subclassOf DnD5eCharacter:Warlock ;
              DnD5eCharacter:unlocksAtClassLevel 1 ;
              rdfs:label "Otherworldly Patron"@en ;
              rdfs:comment "At 1st level, you have struck a bargain with an otherworldly being of your choice."@en .

DnD5eCharacter:TheFiend 	a rdfs:Class ;
              rdfs:subClassOf DnD5eCharacter:OtherworldlyPatron ;
              rdfs:label "The Fiend"@en .

DnD5eCharacter:PactBoon 	a rdfs:Class ;
              rdfs:subClassOf DnD5eCharacter:Subclass ;
              DnD5eCharacter:subclassOf DnD5eCharacter:Warlock ;
              DnD5eCharacter:unlocksAtClassLevel 3 ;
              rdfs:label "Pact Boon"@en ;
              rdfs:comment "At 3rd level, your otherworldly patron bestows a gift upon you for your loyal service."@en .

DnD5eCharacter:PactOfTheBlade 	a rdfs:Class ;
              rdfs:subClassOf DnD5eCharacter:PactBoon ;
              rdfs:label "Pact Of The Blade"@en .

DnD5eCharacter:PactOfTheTome 	a rdfs:Class ;
              rdfs:subClassOf DnD5eCharacter:PactBoon ;
              rdfs:label "Pact Of The Tome"@en .

DnD5eCharacter:PactOfTheChain 	a rdfs:Class ;
              rdfs:subClassOf DnD5eCharacter:PactBoon ;
              rdfs:label "Pact Of The Chain"@en .

DnD5eCharacter:DivineDomain 	a rdfs:Class ;
              rdfs:subClassOf DnD5eCharacter:Subclass ;
              DnD5eCharacter:subclassOf DnD5eCharacter:Cleric ;
              DnD5eCharacter:unlocksAtClassLevel 1 ;
              rdfs:label "Divine Domain"@en ;
              rdfs:comment "At 1st level, you choose a domain shaped by your choice of Deity and the gifts they grant you."@en .

DnD5eCharacter:LifeDomain 	a rdfs:Class ;
              rdfs:subClassOf DnD5eCharacter:DivineDomain ;
              rdfs:label "Life Domain"@en .

DnD5eCharacter:MonkasticTradition 	a rdfs:Class ;
              rdfs:subClassOf DnD5eCharacter:Subclass ;
              DnD5eCharacter:subclassOf DnD5eCharacter:Monk ;
              DnD5eCharacter:unlocksAtClassLevel 3 ;
              rdfs:label "Monkastic Tradition"@en ;
              rdfs:comment "When you reach 3rd level, you commit yourself to a monastic tradition."@en .

DnD5eCharacter:WayOfTheOpenHand 	a rdfs:Class ;
              rdfs:subClassOf DnD5eCharacter:MonkasticTradition ;
              rdfs:label "Way Of The Open Hand"@en .

DnD5eCharacter:RoguishArchetype 	a rdfs:Class ;
              rdfs:subClassOf DnD5eCharacter:Subclass ;
              DnD5eCharacter:subclassOf DnD5eCharacter:Rogue ;
              DnD5eCharacter:unlocksAtClassLevel 3 ;
              rdfs:label "Roguish Archetype"@en ;
              rdfs:comment "At 3rd level, you choose an archetype that you emulate in the exercise of your rogue abilities."@en .

DnD5eCharacter:Thief 	a rdfs:Class ;
              rdfs:subClassOf DnD5eCharacter:RoguishArchetype ;
              rdfs:label "Thief"@en .

DnD5eCharacter:ArcaneTradition 	a rdfs:Class ;
              rdfs:subClassOf DnD5eCharacter:Subclass ;
              DnD5eCharacter:subclassOf DnD5eCharacter:Wizard ;
              DnD5eCharacter:unlocksAtClassLevel 2 ;
              rdfs:label "Arcane Tradition"@en ;
              rdfs:comment "When you reach 2nd level, you choose an arcane tradition, shaping your practice of magic through one of the following schools."@en .

DnD5eCharacter:SchoolOfEvocation 	a rdfs:Class ;
              rdfs:subClassOf DnD5eCharacter:ArcaneTradition ;
              rdfs:label "School Of Evocation"@en .

## D&D Abilities

DnD5eCharacter:AbilityScore 	a rdfs:Class ;
              rdfs:subClassOf TTRpg:CharacterType ;
              rdfs:label "Ability Score"@en ;
              rdfs:comment "An indicator of a characters aptness in a certain ability. These abilities are strength, dexterity, constitution, intelligence, wisdom and charisma."@en .

DnD5eCharacter:Strength 	a rdfs:Class ;
              rdfs:subClassOf DnD5eCharacter:AbilityScore ;
              rdfs:label "Strength"@en ;
              rdfs:comment "Strength measures bodily power, athletic Training, and the extent to which you can exert raw physical force."@en .

DnD5eCharacter:Dexterity 	a rdfs:Class ;
              rdfs:subClassOf DnD5eCharacter:AbilityScore ;
              rdfs:label "Dexterity"@en ;
              rdfs:comment "Dexterity measures agility, reflexes, and balance."@en .

DnD5eCharacter:Constitution 	a rdfs:Class ;
              rdfs:subClassOf DnD5eCharacter:AbilityScore ;
              rdfs:label "Constitution"@en ;
              rdfs:comment "Constitution measures health, stamina, and vital force."@en .

DnD5eCharacter:Intelligence 	a rdfs:Class ;
              rdfs:subClassOf DnD5eCharacter:AbilityScore ;
              rdfs:label "Intelligence"@en ;
              rdfs:comment "Intelligence measures mental acuity, accuracy of recall, and the ability to reason."@en .

DnD5eCharacter:Wisdom 	a rdfs:Class ;
              rdfs:subClassOf DnD5eCharacter:AbilityScore ;
              rdfs:label "Wisdom"@en ;
              rdfs:comment "Wisdom reflects how attuned you are to the world around you and represents perceptiveness and intuition."@en .

DnD5eCharacter:Charisma 	a rdfs:Class ;
              rdfs:subClassOf DnD5eCharacter:AbilityScore ;
              rdfs:label "Charisma"@en ;
              rdfs:comment "Charisma measures your ability to interact effectively with others. It includes such factors as confidence and eloquence, and it can represent a charming or commanding Personality."@en .

## D&D Skills

DnD5eCharacter:Skill 	a rdfs:Class ;
              rdfs:subClassOf TTRpg:CharacterType ;
              rdfs:label "Skill"@en ;
              rdfs:comment "An indicator of a characters aptness in a certain skill that is derived from a parent ability."@en .

DnD5eCharacter:Acrobatics 	a rdfs:Class ;
              rdfs:subClassOf DnD5eCharacter:Skill ;
              DnD5eCharacter:basedOn DnD5eCharacter:Dexterity ;
              rdfs:label "Acrobatics"@en ;
              rdfs:comment "Your Acrobatics check covers your attempt to stay on your feet in a tricky situation, such as when you're trying to run across a sheet of ice, balance on a tightrope, or stay upright on a rocking ship's deck."@en .

DnD5eCharacter:AnimalHandling 	a rdfs:Class ;
              rdfs:subClassOf DnD5eCharacter:Skill ;
              DnD5eCharacter:basedOn DnD5eCharacter:Wisdom ;
              rdfs:label "Animal Handling"@en ;
              rdfs:comment "When there is any question whether you can calm down a domesticated animal, keep a mount from getting spooked, or intuit an animal's intentions, the GM might call for a Animal Handling check. You also make a Animal Handling check to control your mount when you attempt a risky maneuver."@en .

DnD5eCharacter:Arcana 	a rdfs:Class ;
              rdfs:subClassOf DnD5eCharacter:Skill ;
              DnD5eCharacter:basedOn DnD5eCharacter:Intelligence ;
              rdfs:label "Arcana"@en ;
              rdfs:comment "Your Arcana check measures your ability to recall lore about Spells, magic items, eldritch Symbols, magical traditions, The Planes of existence, and the inhabitants of those planes."@en .

DnD5eCharacter:Athletics 	a rdfs:Class ;
              rdfs:subClassOf DnD5eCharacter:Skill ;
              DnD5eCharacter:basedOn DnD5eCharacter:Strength ;
              rdfs:label "Athletics"@en ;
              rdfs:comment "Your Athletics check covers difficult situations you encounter while climbing, Jumping, or Swimming."@en .

DnD5eCharacter:Deception 	a rdfs:Class ;
              rdfs:subClassOf DnD5eCharacter:Skill ;
              DnD5eCharacter:basedOn DnD5eCharacter:Charisma ;
              rdfs:label "Deception"@en ;
              rdfs:comment "Your Deception check determines whether you can convincingly hide the truth, either verbally or through your Actions. This Deception can encompass everything from misleading others through ambiguity to telling outright lies. Typical situations include trying to fast- talk a guard, con a merchant, earn money through Gambling, pass yourself off in a disguise, dull someone's suspicions with false assurances, or maintain a straight face while telling a blatant lie."@en .

DnD5eCharacter:History 	a rdfs:Class ;
              rdfs:subClassOf DnD5eCharacter:Skill ;
              DnD5eCharacter:basedOn DnD5eCharacter:Intelligence ;
              rdfs:label "History"@en ;
              rdfs:comment "Your History check measures your ability to recall lore about historical events, legendary people, ancient kingdoms, past disputes, recent wars, and lost civilizations."@en .

DnD5eCharacter:Insight 	a rdfs:Class ;
              rdfs:subClassOf DnD5eCharacter:Skill ;
              DnD5eCharacter:basedOn DnD5eCharacter:Wisdom ;
              rdfs:label "Insight"@en ;
              rdfs:comment "Your Insight check decides whether you can determine the true intentions of a creature, such as when searching out a lie or predicting someone's next move. Doing so involves gleaning clues from body language, Speech habits, and changes in mannerisms."@en .

DnD5eCharacter:Initimidation 	a rdfs:Class ;
              rdfs:subClassOf DnD5eCharacter:Skill ;
              DnD5eCharacter:basedOn DnD5eCharacter:Charisma ;
              rdfs:label "Initimidation"@en ;
              rdfs:comment "When you attempt to Influence someone through overt threats, Hostile Actions, and physical violence, the GM might ask you to make a Intimidation check. Examples include trying to pry information out of a prisoner, convincing street thugs to back down from a confrontation, or using the edge of a broken bottle to convince a sneering vizier to reconsider a decision."@en .

DnD5eCharacter:Investigation 	a rdfs:Class ;
              rdfs:subClassOf DnD5eCharacter:Skill ;
              DnD5eCharacter:basedOn DnD5eCharacter:Intelligence ;
              rdfs:label "Investigation"@en ;
              rdfs:comment "When you look around for clues and make deductions based on those clues, you make an Investigation check. You might deduce the Location of a hidden object, discern from the Appearance of a wound what kind of weapon dealt it, or determine the weakest point in a tunnel that could cause it to collapse. Poring through ancient Scrolls in Search of a hidden fragment of knowledge might also call for an Investigation check."@en .

DnD5eCharacter:Medicine 	a rdfs:Class ;
              rdfs:subClassOf DnD5eCharacter:Skill ;
              DnD5eCharacter:basedOn DnD5eCharacter:Wisdom ;
              rdfs:label "Medicine"@en ;
              rdfs:comment "A Medicine check lets you try to stabilize a dying Companion or diagnose an illness."@en .

DnD5eCharacter:Nature 	a rdfs:Class ;
              rdfs:subClassOf DnD5eCharacter:Skill ;
              DnD5eCharacter:basedOn DnD5eCharacter:Intelligence ;
              rdfs:label "Nature"@en ;
              rdfs:comment "Your Nature check measures your ability to recall lore about terrain, Plants and animals, the weather, and natural cycles."@en .

DnD5eCharacter:Perception 	a rdfs:Class ;
              rdfs:subClassOf DnD5eCharacter:Skill ;
              DnD5eCharacter:basedOn DnD5eCharacter:Wisdom ;
              rdfs:label "Perception"@en ;
              rdfs:comment "Your Perception check lets you spot, hear, or otherwise detect the presence of something. It measures your general awareness of your surroundings and the keenness of your Senses. For example, you might try to hear a conversation through a closed door, eavesdrop under an open window, or hear Monsters moving stealthily in the Forest. Or you might try to spot things that are obscured or easy to miss, whether they are orcs lying in Ambush on a road, thugs Hiding in the shadows of an alley, or candlelight under a closed Secret door."@en .

DnD5eCharacter:Performance 	a rdfs:Class ;
              rdfs:subClassOf DnD5eCharacter:Skill ;
              DnD5eCharacter:basedOn DnD5eCharacter:Charisma ;
              rdfs:label "Performance"@en ;
              rdfs:comment "Your Performance check determines how well you can delight an audience with music, dance, Acting, Storytelling, or some other form of entertainment."@en .

DnD5eCharacter:Persuasion 	a rdfs:Class ;
              rdfs:subClassOf DnD5eCharacter:Skill ;
              DnD5eCharacter:basedOn DnD5eCharacter:Charisma ;
              rdfs:label "Persuasion"@en ;
              rdfs:comment "When you attempt to Influence someone or a group of people with tact, social graces, or good Nature, the GM might ask you to make a Persuasion check. Typically, you use Persuasion when Acting in good faith, to foster friendships, make cordial requests, or exhibit proper etiquette. Examples of persuading others include convincing a chamberlain to let your party see the king, negotiating peace between warring tribes, or inspiring a crowd of townsfolk."@en .

DnD5eCharacter:Religion 	a rdfs:Class ;
              rdfs:subClassOf DnD5eCharacter:Skill ;
              DnD5eCharacter:basedOn DnD5eCharacter:Intelligence ;
              rdfs:label "Religion"@en ;
              rdfs:comment "Your Religion check measures your ability to recall lore about deities, rites and prayers, religious hierarchies, holy Symbols, and the practices of Secret cults."@en .

DnD5eCharacter:SleightOfHand 	a rdfs:Class ;
              rdfs:subClassOf DnD5eCharacter:Skill ;
              DnD5eCharacter:basedOn DnD5eCharacter:Dexterity ;
              rdfs:label "Sleight Of Hand"@en ;
              rdfs:comment "Whenever you attempt an act of legerdemain or manual trickery, such as planting something on someone else or concealing an object on your person, make a Sleight of Hand check."@en .

DnD5eCharacter:Stealth 	a rdfs:Class ;
              rdfs:subClassOf DnD5eCharacter:Skill ;
              DnD5eCharacter:basedOn DnD5eCharacter:Dexterity ;
              rdfs:label "Stealth"@en ;
              rdfs:comment "Make a Stealth check when you attempt to conceal yourself from enemies, slink past guards, slip away without Being Noticed, or sneak up on someone without being seen or heard."@en .

DnD5eCharacter:Survival 	a rdfs:Class ;
              rdfs:subClassOf DnD5eCharacter:Skill ;
              DnD5eCharacter:basedOn DnD5eCharacter:Wisdom ;
              rdfs:label "Survival"@en ;
              rdfs:comment "The GM might ask you to make a Survival check to follow tracks, hunt wild game, guide your group through frozen wastelands, Identify signs that owlbears live nearby, predict the weather, or avoid Quicksand and other natural Hazards."@en .

DnD5eCharacter:Proficiency 	a rdfs:Class ;
              rdfs:subClassOf TTRpg:CharacterType ;
              rdfs:label "Proficiency"@en ;
              rdfs:comment "This means a character is proficient in a certain skill. The acommpanying skill can be indicated using the DnD5eCharacter:proficientIn property."@en .

DnD5eCharacter:Expertise 	a rdfs:Class ;
              rdfs:subClassOf TTRpg:CharacterType ;
              rdfs:label "Expertise"@en ;
              rdfs:comment "This means a character is an expert in a certain skill. The acommpanying skill can be indicated using the DnD5eCharacter:expertIn property."@en .

## D&D Alignments

DnD5eCharacter:Alignemnt 	a rdfs:Class ;
              rdfs:subClassOf DnD5eCharacter:Alignment ;
              rdfs:label "Alignment"@en ;
              rdfs:comment "A typical creature in the game world has an alignment, which broadly describes its moral and personal attitudes. Alignment is a combination of two factors: one identifies morality (good, evil, or neutral), and the other describes attitudes toward society and order (lawful, chaotic, or neutral)."@en .

DnD5eCharacter:LawfulGood 	a rdfs:Class ;
              rdfs:subClassOf DnD5eCharacter:Alignment ;
              rdfs:label "Lawful Good"@en ;
              rdfs:comment "Lawful good (LG) creatures can be counted on to do the right thing as expected by society. Gold dragons, paladins, and most dwarves are lawful good."@en .

DnD5eCharacter:NeutralGood 	a rdfs:Class ;
              rdfs:subClassOf DnD5eCharacter:Alignment ;
              rdfs:label "Neutral Good"@en ;
              rdfs:comment "Neutral good (NG) folk do the best they can to help others according to their needs. Many celestials, some cloud giants, and most gnomes are neutral good."@en .

DnD5eCharacter:ChaoticGood 	a rdfs:Class ;
              rdfs:subClassOf DnD5eCharacter:Alignment ;
              rdfs:label "Chaotic Good"@en ;
              rdfs:comment "Chaotic good (CG) creatures act as their conscience directs, with little regard for what others expect. Copper dragons, many elves, and unicorns are chaotic good."@en .

DnD5eCharacter:LawfulNeutral 	a rdfs:Class ;
              rdfs:subClassOf DnD5eCharacter:Alignment ;
              rdfs:label "Lawful Neutral"@en ;
              rdfs:comment "Lawful neutral (LN) individuals act in accordance with law, tradition, or personal codes. Many monks and some wizards are lawful neutral."@en .

DnD5eCharacter:Neutral 	a rdfs:Class ;
              rdfs:subClassOf DnD5eCharacter:Alignment ;
              rdfs:label "Neutral"@en ;
              rdfs:comment "Neutral (N) is the alignment of those who prefer to steer clear of moral questions and don't take sides, doing what seems best at the time. Lizardfolk, most druids, and many humans are neutral."@en .

DnD5eCharacter:ChaoticNeutral 	a rdfs:Class ;
              rdfs:subClassOf DnD5eCharacter:Alignment ;
              rdfs:label "Chaotic Neutral"@en ;
              rdfs:comment "Chaotic neutral (CN) creatures follow their whims, holding their personal freedom above all else. Many barbarians and rogues, and some bards, are chaotic neutral."@en .

DnD5eCharacter:LawfulEvil 	a rdfs:Class ;
              rdfs:subClassOf DnD5eCharacter:Alignment ;
              rdfs:label "Lawful Evil"@en ;
              rdfs:comment "Lawful evil (LE) creatures methodically take what they want, within the limits of a code of tradition, loyalty, or order. Devils, blue dragons, and hobgoblins are lawful evil."@en .

DnD5eCharacter:NeutralEvil 	a rdfs:Class ;
              rdfs:subClassOf DnD5eCharacter:Alignment ;
              rdfs:label "Neutral Evil"@en ;
              rdfs:comment "Neutral evil (NE) is the alignment of those who do whatever they can get away with, without compassion or qualms. Many drow, some cloud giants, and goblins are neutral evil."@en .

DnD5eCharacter:ChaoticEvil 	a rdfs:Class ;
              rdfs:subClassOf DnD5eCharacter:Alignment ;
              rdfs:label "Chaotic Evil"@en ;
              rdfs:comment "Chaotic evil (CE) creatures act with arbitrary violence, spurred by their greed, hatred, or bloodlust. Demons, red dragons, and orcs are chaotic evil."@en .

## D&D Backgrounds

DnD5eCharacter:Background 	a rdfs:Class ;
              rdfs:subClassOf TTRpg:CharacterType ;
              rdfs:label "Background"@en ;
              rdfs:comment "A background gives more information about a character and can help you play that character by explaining their motivations and their past."@en .

DnD5eCharacter:Acolyte 	a rdfs:Class ;
              rdfs:subClassOf TTRpg:Background ;
              rdfs:label "Acolyte"@en ;
              rdfs:comment "You have spent your life in the service of a temple to a specific god or pantheon of gods. You act as an intermediary between the realm of the holy and the mortal world, performing sacred rites and offering sacrifices in order to conduct worshipers into the presence of the divine. You are not necessarily a cleric - performing sacred rites is not the same thing as channeling divine power."@en .

## D&D Monsters & Monster Types

DnD5eCharacter:Monster 	a rdfs:Class ;
              rdfs:subClassOf TTRpg:CharacterType ;
              DnD5eCharacter:type DnD5eCharacter:MonsterType ;
              rdfs:label "Monster"@en ;
              rdfs:comment "A monster in Dungeons & Dragons, usually the actions of such a monster are decided by the DM."@en .

DnD5eCharacter:MonsterType 	a rdfs:Class ;
              rdfs:label "Monster Type"@en ;
              rdfs:comment "A type of monster."@en .

DnD5eCharacter:Abberation 	a rdfs:Class ;
              rdfs:subClassOf DnD5eCharacter:MonsterType ;
              rdfs:subClassOf DnD5eCharacter:FavoredMonsterType ;
              rdfs:label "Abberation"@en ;
              rdfs:comment "An aberration has a bizarre anatomy, strange abilities, alien mindset, or any combination thereof. All aberrations have darkvision. Examples include aboleths, beholders, and mind flayers."@en .

DnD5eCharacter:Beast 	a rdfs:Class ;
              rdfs:subClassOf DnD5eCharacter:MonsterType ;
              rdfs:subClassOf DnD5eCharacter:FavoredMonsterType ;
              rdfs:label "Beast"@en ;
              rdfs:comment "An animal is a nonhuman, usually vertebrate creature. Animals have very low intelligence and usually low-light vision. This category does not include invertebrates, which are classed as vermin. Examples include bears, crocodiles, horses, and wolves. Dire animals are also considered animals."@en .

DnD5eCharacter:Celestial 	a rdfs:Class ;
              rdfs:subClassOf DnD5eCharacter:MonsterType ;
              rdfs:subClassOf DnD5eCharacter:FavoredMonsterType ;
              rdfs:label "Celestial"@en ;
              rdfs:comment "Celestials are creatures native to the Upper Planes, and good by nature. Examples include angels, couatls, and pegasi."@en .

DnD5eCharacter:Construct 	a rdfs:Class ;
              rdfs:subClassOf DnD5eCharacter:MonsterType ;
              rdfs:subClassOf DnD5eCharacter:FavoredMonsterType ;
              rdfs:label "Construct"@en ;
              rdfs:comment "Constructs are creatures that are created artificially. Examples include golems, although modrons are also constructs."@en .

DnD5eCharacter:Dragon 	a rdfs:Class ;
              rdfs:subClassOf DnD5eCharacter:MonsterType ;
              rdfs:subClassOf DnD5eCharacter:FavoredMonsterType ;
              rdfs:label "Dragon"@en ;
              rdfs:comment "Dragons are large, powerful reptilian creatures. This includes both true dragons such as the chromatic and metallic dragons, but also related creatures such as wyverns."@en .

DnD5eCharacter:Elemental 	a rdfs:Class ;
              rdfs:subClassOf DnD5eCharacter:MonsterType ;
              rdfs:subClassOf DnD5eCharacter:FavoredMonsterType ;
              rdfs:label "Elemental"@en ;
              rdfs:comment "Elementals are creatures from the Elemental Planes. Examples include the common elementals as well as azer, genies, and invisible stalkers."@en .

DnD5eCharacter:Fey 	a rdfs:Class ;
              rdfs:subClassOf DnD5eCharacter:MonsterType ;
              rdfs:subClassOf DnD5eCharacter:FavoredMonsterType ;
              rdfs:label "Fey"@en ;
              rdfs:comment "Fey are creatures of magic with a connection to nature. Often they are connected to the Feywild, or certain Outer Planes such as Arboreaor the Beastlands. Examples include dryads and satyrs."@en .

DnD5eCharacter:Fiend 	a rdfs:Class ;
              rdfs:subClassOf DnD5eCharacter:MonsterType ;
              rdfs:subClassOf DnD5eCharacter:FavoredMonsterType ;
              rdfs:label "Fiend"@en ;
              rdfs:comment "Fiends are creatures native to the Lower Planes, and evil by nature. Examples include demons, devils, and rakshasa."@en .

DnD5eCharacter:Giant 	a rdfs:Class ;
              rdfs:subClassOf DnD5eCharacter:MonsterType ;
              rdfs:subClassOf DnD5eCharacter:FavoredMonsterType ;
              rdfs:label "Giant"@en ;
              rdfs:comment "Giants are human-like but larger thanhumans. Examples include the true giants as well as ogres and trolls."@en .

DnD5eCharacter:Humanoid 	a rdfs:Class ;
              rdfs:subClassOf DnD5eCharacter:MonsterType ;
              rdfs:subClassOf DnD5eCharacter:FavoredMonsterType ;
              rdfs:label "Humanoid"@en ;
              rdfs:comment "Humanoids are the main people of most worlds, bipeds with culture but few natural magical abilities. Examples include humans, dwarves, elves and the goblinoid races."@en .

DnD5eCharacter:Monstrosity 	a rdfs:Class ;
              rdfs:subClassOf DnD5eCharacter:MonsterType ;
              rdfs:subClassOf DnD5eCharacter:FavoredMonsterType ;
              rdfs:label "Monstrosity"@en ;
              rdfs:comment "Monstrosities are unnatural creatures from a variety of origins, including curses and magical experimentation. Examples include minotaurs and owlbears. The monstrosity type is also a 'catch-all' category for monsters that don't fit into other types."@en .

DnD5eCharacter:Ooze 	a rdfs:Class ;
              rdfs:subClassOf DnD5eCharacter:MonsterType ;
              rdfs:subClassOf DnD5eCharacter:FavoredMonsterType ;
              rdfs:label "Ooze"@en ;
              rdfs:comment "Oozes are gelatinous creatures with no fixed form. Examples include black puddings and gelatinous cubes."@en .

DnD5eCharacter:Plant 	a rdfs:Class ;
              rdfs:subClassOf DnD5eCharacter:MonsterType ;
              rdfs:subClassOf DnD5eCharacter:FavoredMonsterType ;
              rdfs:label "Plant"@en ;
              rdfs:comment "Plants include both vegetable and fungal creatures. Examples include hambling mounds and myconids."@en .

DnD5eCharacter:Undead 	a rdfs:Class ;
              rdfs:subClassOf DnD5eCharacter:MonsterType ;
              rdfs:subClassOf DnD5eCharacter:FavoredMonsterType ;
              rdfs:label "Undead"@en ;
              rdfs:comment "Undead creatures were once alive, but reanimated by unnatural forces. Examples includeghosts,specters,vampires and zombies."@en .

DnD5eCharacter:Bugbear 	a rdfs:Class ;
              rdfs:subClassOf DnD5eCharacter:Humanoid ;
              rdfs:subClassOf DnD5eCharacter:FavoredHumanoids ;
              rdfs:label "Bugbear"@en ;
              rdfs:comment "Bugbears resembled hairy, feral goblins standing 7?feet (2.1?meters) tall. They took their name from their noses and claws, which were similar to those of bears."@en .

DnD5eCharacter:Bullywug 	a rdfs:Class ;
              rdfs:subClassOf DnD5eCharacter:Humanoid ;
              rdfs:subClassOf DnD5eCharacter:FavoredHumanoids ;
              rdfs:label "Bullywug"@en ;
              rdfs:comment "Bullywugs were a primitive race of frog-like humanoids found throughout the bogs and marshes of Toril, the self-proclaimed lords of the swamp. Savage and self-destructive, the bullywugs regularly tampered with forces beyond their understanding, threatening the safety of others and their own brutish, noisome, and wet lives."@en .

DnD5eCharacter:Githyanki 	a rdfs:Class ;
              rdfs:subClassOf DnD5eCharacter:Humanoid ;
              rdfs:subClassOf DnD5eCharacter:FavoredHumanoids ;
              rdfs:label "Githyanki"@en ;
              rdfs:comment "The githyanki were a race of Astral Plane-dwellers. Survivors of a long enslavement by mind flayers, they became ruthless pillagers and raiders of many worlds in the Prime Material plane."@en .

DnD5eCharacter:Gitzerai 	a rdfs:Class ;
              rdfs:subClassOf DnD5eCharacter:Humanoid ;
              rdfs:subClassOf DnD5eCharacter:FavoredHumanoids ;
              rdfs:label "Gitzerai"@en ;
              rdfs:comment "The githzerai were a humanoid race that dwelt primarily in the plane of Limbo. They descended from a splinter group of gith, a race that had been enslaved by mind flayers for centuries until they rebelled for their freedom. Philosophical differences led to a long and bloody civil war among the gith, who ended up divided into the militaristic githyanki and the ascetic githzerai."@en .

DnD5eCharacter:Gnoll 	a rdfs:Class ;
              rdfs:subClassOf DnD5eCharacter:Humanoid ;
              rdfs:subClassOf DnD5eCharacter:FavoredHumanoids ;
              rdfs:label "Gnoll"@en ;
              rdfs:comment "Gnolls were a humanoid race that most closely resembled human-hyena hybrids within Faerûn. They were carnivorous humanoids, known for their savage culture and warlike ways."@en .

DnD5eCharacter:Goblin 	a rdfs:Class ;
              rdfs:subClassOf DnD5eCharacter:Humanoid ;
              rdfs:subClassOf DnD5eCharacter:FavoredHumanoids ;
              rdfs:label "Goblin"@en ;
              rdfs:comment "Goblins were a race of small and numerous goblinoids common throughout Toril, often living in underground caverns near the surface known as lairs. The race was often, though not always, dominated by other goblinoids, most commonly hobgoblins. Goblins may have, in fact, been initially created by this related race to serve as scouts and infiltrators."@en .

DnD5eCharacter:Grimlock 	a rdfs:Class ;
              rdfs:subClassOf DnD5eCharacter:Humanoid ;
              rdfs:subClassOf DnD5eCharacter:FavoredHumanoids ;
              rdfs:label "Grimlock"@en ;
              rdfs:comment "Grimlocks were a race of monstrous humanoids that lived in the Underdark, the degenerated descendants of humans who had wandered into its depths centuries ago."@en .

DnD5eCharacter:Hobgoblin 	a rdfs:Class ;
              rdfs:subClassOf DnD5eCharacter:Humanoid ;
              rdfs:subClassOf DnD5eCharacter:FavoredHumanoids ;
              rdfs:label "Hobgoblin"@en ;
              rdfs:comment "Hobgoblins were larger, stronger, smarter, and more menacing forms of goblinoids than goblins, but not as powerful as bugbears."@en .

DnD5eCharacter:KoaToa 	a rdfs:Class ;
              rdfs:subClassOf DnD5eCharacter:Humanoid ;
              rdfs:subClassOf DnD5eCharacter:FavoredHumanoids ;
              rdfs:label "Koa Toa"@en ;
              rdfs:comment "Kuo-toa (pronounced: Koa Toa), also known as gogglers and men-fish, were a debased, piscine race of warm-blooded and amphibious creatures that dwelt in the Underdark. Sinister secrets lurked below the surface of their alien minds, for the kuo-toa were fanatics plagued by mental instability that saw things others couldn't and worshiped gods that didn't exist — at least until they believed hard enough."@en .

DnD5eCharacter:Kobold 	a rdfs:Class ;
              rdfs:subClassOf DnD5eCharacter:Humanoid ;
              rdfs:subClassOf DnD5eCharacter:FavoredHumanoids ;
              rdfs:label "Kobold"@en ;
              rdfs:comment "Kobolds were aggressive, insular, yet industrious small humanoid creatures. They were noted for their skill at building traps and preparing ambushes, and mining. They were distantly related to dragons and urds and were often found serving as their minions."@en .

DnD5eCharacter:Lizardfolk 	a rdfs:Class ;
              rdfs:subClassOf DnD5eCharacter:Humanoid ;
              rdfs:subClassOf DnD5eCharacter:FavoredHumanoids ;
              rdfs:label "Lizardfolk"@en ;
              rdfs:comment "Lizardfolk, also known as lizard men, were a race of reptilian humanoids native to Toril."@en .

DnD5eCharacter:Merfolk 	a rdfs:Class ;
              rdfs:subClassOf DnD5eCharacter:Humanoid ;
              rdfs:subClassOf DnD5eCharacter:FavoredHumanoids ;
              rdfs:label "Merfolk"@en ;
              rdfs:comment "Merfolk were aquatic humanoids with upper body, arm and head of a human and legs resembling the tail of a fish."@en .

DnD5eCharacter:Orc 	a rdfs:Class ;
              rdfs:subClassOf DnD5eCharacter:Humanoid ;
              rdfs:subClassOf DnD5eCharacter:FavoredHumanoids ;
              rdfs:label "Orc"@en ;
              rdfs:comment "Orcs were a race of humanoids that had been a threat to the civilized cultures of Toril, particularly Faerûn, for as long as any could remember. This changed somewhat in the years preceding and immediately after the Spellplague, when a horde of mountain orcs under the command of King Obould Many-Arrows unified into a single kingdom, one that was remarkably civilized."@en .

DnD5eCharacter:ThriKreen 	a rdfs:Class ;
              rdfs:subClassOf DnD5eCharacter:Humanoid ;
              rdfs:subClassOf DnD5eCharacter:FavoredHumanoids ;
              rdfs:label "Thri Kreen"@en ;
              rdfs:comment "The thri-kreen were an insectoid monstrous humanoid race that primarily lived in the Shaar. The thri-kreen were a race of nomads and hunters. They were also known as mantis warriors and sometimes called tri-kreen."@en .

DnD5eCharacter:Troglodyte 	a rdfs:Class ;
              rdfs:subClassOf DnD5eCharacter:Humanoid ;
              rdfs:subClassOf DnD5eCharacter:FavoredHumanoids ;
              rdfs:label "Troglodyte"@en ;
              rdfs:comment "Troglodytes, often referred to as stinkmeat by the duergar, were cave-dwelling reptilian humanoids, with a barbaric culture centered around food and scent. The stench of an angry or frightened troglodyte was so foul that it sickened all living creatures nearby, even after the troglodyte had died."@en .

DnD5eCharacter:YuanTiPureblood 	a rdfs:Class ;
              rdfs:subClassOf DnD5eCharacter:Humanoid ;
              rdfs:subClassOf DnD5eCharacter:FavoredHumanoids ;
              rdfs:label "Yuan Ti Pureblood"@en ;
              rdfs:comment "Purebloods were the most human-seeming of all true yuan-ti and one of three main breeds—the other two being the halfbloods and the abominations."@en .

## D&D Terrain

DnD5eCharacter:Terrain 	a rdfs:Class ;
              rdfs:label "Terrain"@en .

DnD5eCharacter:Arctic 	a rdfs:Class ;
              rdfs:subClassOf DnD5eCharacter:Terrain ;
							rdfs:subClassOf DnD5eCharacter:FavoredTerrain ;
              rdfs:label "Arctic"@en .

DnD5eCharacter:Grassland 	a rdfs:Class ;
              rdfs:subClassOf DnD5eCharacter:Terrain ;
							rdfs:subClassOf DnD5eCharacter:FavoredTerrain ;
              rdfs:label "Grassland"@en .

DnD5eCharacter:Coast 	a rdfs:Class ;
              rdfs:subClassOf DnD5eCharacter:Terrain ;
							rdfs:subClassOf DnD5eCharacter:FavoredTerrain ;
              rdfs:label "Coast"@en .

DnD5eCharacter:Mountain 	a rdfs:Class ;
              rdfs:subClassOf DnD5eCharacter:Terrain ;
							rdfs:subClassOf DnD5eCharacter:FavoredTerrain ;
              rdfs:label "Mountain"@en .

DnD5eCharacter:Desert 	a rdfs:Class ;
              rdfs:subClassOf DnD5eCharacter:Terrain ;
							rdfs:subClassOf DnD5eCharacter:FavoredTerrain ;
              rdfs:label "Desert"@en .

DnD5eCharacter:Swamp 	a rdfs:Class ;
              rdfs:subClassOf DnD5eCharacter:Terrain ;
							rdfs:subClassOf DnD5eCharacter:FavoredTerrain ;
              rdfs:label "Swamp"@en .

DnD5eCharacter:Forest 	a rdfs:Class ;
              rdfs:subClassOf DnD5eCharacter:Terrain ;
							rdfs:subClassOf DnD5eCharacter:FavoredTerrain ;
              rdfs:label "Forest"@en .

DnD5eCharacter:Underdark 	a rdfs:Class ;
              rdfs:subClassOf DnD5eCharacter:Terrain ;
							rdfs:subClassOf DnD5eCharacter:FavoredTerrain ;
              rdfs:label "Underdark"@en .

## D&D Items

DnD5eCharacter:ItemEnhancement 	a rdfs:Class ;
              rdfs:subClassOf TTRpg:ItemType ;
              rdfs:label "Item Enhancement"@en .

DnD5eCharacter:PlusOne 	a rdfs:Class ;
              rdfs:subClassOf TTRpg:ItemEnhancement ;
              rdfs:label "+1"@en ;
              rdfs:comment "Adds 1 to the chance to hit and to the damage dealt."@en .

DnD5eCharacter:PlusTwo 	a rdfs:Class ;
              rdfs:subClassOf TTRpg:ItemEnhancement ;
              rdfs:label "+2"@en ;
              rdfs:comment "Adds 2 to the chance to hit and to the damage dealt."@en .

DnD5eCharacter:PlusThree 	a rdfs:Class ;
              rdfs:subClassOf TTRpg:ItemEnhancement ;
              rdfs:label "+2"@en ;
              rdfs:comment "Adds 3 to the chance to hit and to the damage dealt."@en .

DnD5eCharacter:BattleAxe 	a rdfs:Class ;
              rdfs:subClassOf TTRpg:Weapon ;
              rdfs:label "Battle Axe"@en .

DnD5eCharacter:Blowgun 	a rdfs:Class ;
              rdfs:subClassOf TTRpg:Weapon ;
              rdfs:label "Blowgun"@en .

DnD5eCharacter:Club 	a rdfs:Class ;
              rdfs:subClassOf TTRpg:Weapon ;
              rdfs:label "Club"@en .

DnD5eCharacter:HandCrossbow 	a rdfs:Class ;
              rdfs:subClassOf TTRpg:Weapon ;
              rdfs:label "Hand Crossbow"@en .

DnD5eCharacter:HeavyCrossbow 	a rdfs:Class ;
              rdfs:subClassOf TTRpg:Weapon ;
              rdfs:label "Heavy Crossbow"@en .

DnD5eCharacter:LightCrossbow 	a rdfs:Class ;
              rdfs:subClassOf TTRpg:Weapon ;
              rdfs:label "Light Crossbow"@en .

DnD5eCharacter:Dagger 	a rdfs:Class ;
              rdfs:subClassOf TTRpg:Weapon ;
              rdfs:label "Dagger"@en .

DnD5eCharacter:Dart 	a rdfs:Class ;
              rdfs:subClassOf TTRpg:Weapon ;
              rdfs:label "Dart"@en .

DnD5eCharacter:Flail 	a rdfs:Class ;
              rdfs:subClassOf TTRpg:Weapon ;
              rdfs:label "Flail"@en .

DnD5eCharacter:Glaive 	a rdfs:Class ;
              rdfs:subClassOf TTRpg:Weapon ;
              rdfs:label "Glaive"@en .

DnD5eCharacter:Greataxe 	a rdfs:Class ;
              rdfs:subClassOf TTRpg:Weapon ;
              rdfs:label "Greataxe"@en .

DnD5eCharacter:Greatclub 	a rdfs:Class ;
              rdfs:subClassOf TTRpg:Weapon ;
              rdfs:label "Greatclub"@en .

DnD5eCharacter:Greatsword 	a rdfs:Class ;
              rdfs:subClassOf TTRpg:Weapon ;
              rdfs:label "Greatsword"@en .

DnD5eCharacter:Halberd 	a rdfs:Class ;
              rdfs:subClassOf TTRpg:Weapon ;
              rdfs:label "Halberd"@en .

DnD5eCharacter:Handaxe 	a rdfs:Class ;
              rdfs:subClassOf TTRpg:Weapon ;
              rdfs:label "Handaxe"@en .

DnD5eCharacter:Javelin 	a rdfs:Class ;
              rdfs:subClassOf TTRpg:Weapon ;
              rdfs:label "Javelin"@en .

DnD5eCharacter:Lance 	a rdfs:Class ;
              rdfs:subClassOf TTRpg:Weapon ;
              rdfs:label "Lance"@en .

DnD5eCharacter:LightHammer 	a rdfs:Class ;
              rdfs:subClassOf TTRpg:Weapon ;
              rdfs:label "Light Hammer"@en .

DnD5eCharacter:Longbow 	a rdfs:Class ;
              rdfs:subClassOf TTRpg:Weapon ;
              rdfs:label "Longbow"@en .

DnD5eCharacter:Longsword 	a rdfs:Class ;
              rdfs:subClassOf TTRpg:Weapon ;
              rdfs:label "Longsword"@en .

DnD5eCharacter:Mace 	a rdfs:Class ;
              rdfs:subClassOf TTRpg:Weapon ;
              rdfs:label "Mace"@en .

DnD5eCharacter:Maul 	a rdfs:Class ;
              rdfs:subClassOf TTRpg:Weapon ;
              rdfs:label "Maul"@en .

DnD5eCharacter:Morningstar 	a rdfs:Class ;
              rdfs:subClassOf TTRpg:Weapon ;
              rdfs:label "Morningstar"@en .

DnD5eCharacter:Net 	a rdfs:Class ;
              rdfs:subClassOf TTRpg:Weapon ;
              rdfs:label "Net"@en .

DnD5eCharacter:Pike 	a rdfs:Class ;
              rdfs:subClassOf TTRpg:Weapon ;
              rdfs:label "Pike"@en .

DnD5eCharacter:Quarterstaff 	a rdfs:Class ;
              rdfs:subClassOf TTRpg:Weapon ;
              rdfs:label "Quarterstaff"@en .

DnD5eCharacter:Rapier 	a rdfs:Class ;
              rdfs:subClassOf TTRpg:Weapon ;
              rdfs:label "Rapier"@en .

DnD5eCharacter:Scimitar 	a rdfs:Class ;
              rdfs:subClassOf TTRpg:Weapon ;
              rdfs:label "Scimitar"@en .

DnD5eCharacter:Shortbow 	a rdfs:Class ;
              rdfs:subClassOf TTRpg:Weapon ;
              rdfs:label "Shortbow"@en .

DnD5eCharacter:Shortsword 	a rdfs:Class ;
              rdfs:subClassOf TTRpg:Weapon ;
              rdfs:label "Shortsword"@en .

DnD5eCharacter:Sickle 	a rdfs:Class ;
              rdfs:subClassOf TTRpg:Weapon ;
              rdfs:label "Sickle"@en .

DnD5eCharacter:Sling 	a rdfs:Class ;
              rdfs:subClassOf TTRpg:Weapon ;
              rdfs:label "Sling"@en .

DnD5eCharacter:Spear 	a rdfs:Class ;
              rdfs:subClassOf TTRpg:Weapon ;
              rdfs:label "Spear"@en .

DnD5eCharacter:Trident 	a rdfs:Class ;
              rdfs:subClassOf TTRpg:Weapon ;
              rdfs:label "Trident"@en .

DnD5eCharacter:WarPick 	a rdfs:Class ;
              rdfs:subClassOf TTRpg:Weapon ;
              rdfs:label "War Pick"@en .

DnD5eCharacter:Warhammer 	a rdfs:Class ;
              rdfs:subClassOf TTRpg:Weapon ;
              rdfs:label "Warhammer"@en .

DnD5eCharacter:Whip 	a rdfs:Class ;
              rdfs:subClassOf TTRpg:Weapon ;
              rdfs:label "Whip"@en .

DnD5eCharacter:Breastplate 	a rdfs:Class ;
              rdfs:subClassOf TTRpg:Armor ;
              rdfs:label "Breastplate"@en .

DnD5eCharacter:ChainShirt 	a rdfs:Class ;
              rdfs:subClassOf TTRpg:Armor ;
              rdfs:label "Chain Shirt"@en .

DnD5eCharacter:ChainMail 	a rdfs:Class ;
              rdfs:subClassOf TTRpg:Armor ;
              rdfs:label "ChainMail"@en .

DnD5eCharacter:HalfPlate 	a rdfs:Class ;
              rdfs:subClassOf TTRpg:Armor ;
              rdfs:label "HalfPlate"@en .

DnD5eCharacter:Hide 	a rdfs:Class ;
              rdfs:subClassOf TTRpg:Armor ;
              rdfs:label "Hide"@en .

DnD5eCharacter:Leather 	a rdfs:Class ;
              rdfs:subClassOf TTRpg:Armor ;
              rdfs:label "Leather"@en .

DnD5eCharacter:Padded 	a rdfs:Class ;
              rdfs:subClassOf TTRpg:Armor ;
              rdfs:label "Padded"@en .

DnD5eCharacter:Plate 	a rdfs:Class ;
              rdfs:subClassOf TTRpg:Armor ;
              rdfs:label "Plate"@en .

DnD5eCharacter:RingMail 	a rdfs:Class ;
              rdfs:subClassOf TTRpg:Armor ;
              rdfs:label "Ring Mail"@en .

DnD5eCharacter:ScaleMail 	a rdfs:Class ;
              rdfs:subClassOf TTRpg:Armor ;
              rdfs:label "Scale Mail"@en .

DnD5eCharacter:Shield 	a rdfs:Class ;
              rdfs:subClassOf TTRpg:Armor ;
              rdfs:label "Shield"@en .

DnD5eCharacter:SpikedArmor 	a rdfs:Class ;
              rdfs:subClassOf TTRpg:Armor ;
              rdfs:label "Spiked Armor"@en .

DnD5eCharacter:Splint 	a rdfs:Class ;
              rdfs:subClassOf TTRpg:Armor ;
              rdfs:label "Splint"@en .

DnD5eCharacter:Studded 	a rdfs:Class ;
              rdfs:subClassOf TTRpg:Armor ;
              rdfs:label "Studded"@en .

DnD5eCharacter:Copper 	a rdfs:Class ;
              rdfs:subClassOf TTRpg:Currency ;
              rdfs:label "Copper"@en .

DnD5eCharacter:Silver 	a rdfs:Class ;
              rdfs:subClassOf TTRpg:Currency ;
              rdfs:label "Silver"@en .

DnD5eCharacter:Electrum 	a rdfs:Class ;
              rdfs:subClassOf TTRpg:Currency ;
              rdfs:label "Electrum"@en .

DnD5eCharacter:Gold 	a rdfs:Class ;
              rdfs:subClassOf TTRpg:Currency ;
              rdfs:label "Gold"@en .

DnD5eCharacter:Platinum 	a rdfs:Class ;
              rdfs:subClassOf TTRpg:Currency ;
              rdfs:label "Platinum"@en .

DnD5eCharacter:Abacus 	a rdfs:Class ;
              rdfs:subClassOf TTRpg:Tools ;
              rdfs:label "Abacus"@en .

DnD5eCharacter:Acid 	a rdfs:Class ;
              rdfs:subClassOf TTRpg:Tools ;
              rdfs:label "Acid"@en .

DnD5eCharacter:AlmsBox 	a rdfs:Class ;
              rdfs:subClassOf TTRpg:Tools ;
              rdfs:label "Alms Box"@en .

DnD5eCharacter:Amulet 	a rdfs:Class ;
              rdfs:subClassOf TTRpg:Tools ;
              rdfs:label "Amulet"@en .

DnD5eCharacter:Antitoxin 	a rdfs:Class ;
              rdfs:subClassOf TTRpg:Tools ;
              rdfs:label "Antitoxin"@en .

DnD5eCharacter:Arrow 	a rdfs:Class ;
              rdfs:subClassOf TTRpg:Tools ;
              rdfs:label "Arrow"@en .

DnD5eCharacter:Backpack 	a rdfs:Class ;
              rdfs:subClassOf TTRpg:Tools ;
              rdfs:label "Backpack"@en .

DnD5eCharacter:BagOfSand 	a rdfs:Class ;
              rdfs:subClassOf TTRpg:Tools ;
              rdfs:label "Bag Of Sand"@en .

DnD5eCharacter:Bagpipes 	a rdfs:Class ;
              rdfs:subClassOf TTRpg:Tools ;
              rdfs:label "Bagpipes"@en .

DnD5eCharacter:BallBearings 	a rdfs:Class ;
              rdfs:subClassOf TTRpg:Tools ;
              rdfs:label "Ball Bearings"@en .

DnD5eCharacter:Barrel 	a rdfs:Class ;
              rdfs:subClassOf TTRpg:Tools ;
              rdfs:label "Barrel"@en .

DnD5eCharacter:Basket 	a rdfs:Class ;
              rdfs:subClassOf TTRpg:Tools ;
              rdfs:label "Basket"@en .

DnD5eCharacter:Bedroll 	a rdfs:Class ;
              rdfs:subClassOf TTRpg:Tools ;
              rdfs:label "Bedroll"@en .

DnD5eCharacter:Bell 	a rdfs:Class ;
              rdfs:subClassOf TTRpg:Tools ;
              rdfs:label "Bell"@en .

DnD5eCharacter:Blanket 	a rdfs:Class ;
              rdfs:subClassOf TTRpg:Tools ;
              rdfs:label "Blanket"@en .

DnD5eCharacter:BlockAndTackle 	a rdfs:Class ;
              rdfs:subClassOf TTRpg:Tools ;
              rdfs:label "Block And Tackle"@en .

DnD5eCharacter:BlowgunNeedle 	a rdfs:Class ;
              rdfs:subClassOf TTRpg:Tools ;
              rdfs:label "Blowgun Needle"@en .

DnD5eCharacter:Book 	a rdfs:Class ;
              rdfs:subClassOf TTRpg:Tools ;
              rdfs:label "Book"@en .

DnD5eCharacter:GlassBottle 	a rdfs:Class ;
              rdfs:subClassOf TTRpg:Tools ;
              rdfs:label "Glass Bottle"@en .

DnD5eCharacter:Bucket 	a rdfs:Class ;
              rdfs:subClassOf TTRpg:Tools ;
              rdfs:label "Bucket"@en .

DnD5eCharacter:Caltrops 	a rdfs:Class ;
              rdfs:subClassOf TTRpg:Tools ;
              rdfs:label "Caltrops"@en .

DnD5eCharacter:Candle 	a rdfs:Class ;
              rdfs:subClassOf TTRpg:Tools ;
              rdfs:label "Candle"@en .

DnD5eCharacter:Cart 	a rdfs:Class ;
              rdfs:subClassOf TTRpg:Tools ;
              rdfs:label "Cart"@en .

DnD5eCharacter:CrossbowBoltCase 	a rdfs:Class ;
              rdfs:subClassOf TTRpg:Tools ;
              rdfs:label "Crossbow Bolt Case"@en .

DnD5eCharacter:MapOrScrollCase 	a rdfs:Class ;
              rdfs:subClassOf TTRpg:Tools ;
              rdfs:label "Map Or Scroll Case"@en .

DnD5eCharacter:Censer 	a rdfs:Class ;
              rdfs:subClassOf TTRpg:Tools ;
              rdfs:label "Censer"@en .

DnD5eCharacter:Chain 	a rdfs:Class ;
              rdfs:subClassOf TTRpg:Tools ;
              rdfs:label "Chain"@en .

DnD5eCharacter:Chalk 	a rdfs:Class ;
              rdfs:subClassOf TTRpg:Tools ;
              rdfs:label "Chalk"@en .

DnD5eCharacter:Chest 	a rdfs:Class ;
              rdfs:subClassOf TTRpg:Tools ;
              rdfs:label "Chest"@en .

DnD5eCharacter:CommonClothes 	a rdfs:Class ;
              rdfs:subClassOf TTRpg:Tools ;
              rdfs:label "Common Clothes"@en .

DnD5eCharacter:CostumeClothes 	a rdfs:Class ;
              rdfs:subClassOf TTRpg:Tools ;
              rdfs:label "Costume Clothes"@en .

DnD5eCharacter:FineClothes 	a rdfs:Class ;
              rdfs:subClassOf TTRpg:Tools ;
              rdfs:label "Fine Clothes"@en .

DnD5eCharacter:ComponentPouch 	a rdfs:Class ;
              rdfs:subClassOf TTRpg:Tools ;
              rdfs:label "Component Pouch"@en .

DnD5eCharacter:Costume 	a rdfs:Class ;
              rdfs:subClassOf TTRpg:Tools ;
              rdfs:label "Costume"@en .

DnD5eCharacter:CrossbowBolt 	a rdfs:Class ;
              rdfs:subClassOf TTRpg:Tools ;
              rdfs:label "Crossbow Bolt"@en .

DnD5eCharacter:Crowbar 	a rdfs:Class ;
              rdfs:subClassOf TTRpg:Tools ;
              rdfs:label "Crowbar"@en .

DnD5eCharacter:Crystal 	a rdfs:Class ;
              rdfs:subClassOf TTRpg:Tools ;
              rdfs:label "Crystal"@en .

DnD5eCharacter:DiceSet 	a rdfs:Class ;
              rdfs:subClassOf TTRpg:Tools ;
              rdfs:label "Dice Set"@en .

DnD5eCharacter:DisguiseKit 	a rdfs:Class ;
              rdfs:subClassOf TTRpg:Tools ;
              rdfs:label "Disguise Kit"@en .

DnD5eCharacter:DragonchessSet 	a rdfs:Class ;
              rdfs:subClassOf TTRpg:Tools ;
              rdfs:label "Dragonchess Set"@en .

DnD5eCharacter:Drum 	a rdfs:Class ;
              rdfs:subClassOf TTRpg:Tools ;
              rdfs:label "Drum"@en .

DnD5eCharacter:Dulcimer 	a rdfs:Class ;
              rdfs:subClassOf TTRpg:Tools ;
              rdfs:label "Dulcimer"@en .

DnD5eCharacter:Emblem 	a rdfs:Class ;
              rdfs:subClassOf TTRpg:Tools ;
              rdfs:label "Emblem"@en .

DnD5eCharacter:FishingTackle 	a rdfs:Class ;
              rdfs:subClassOf TTRpg:Tools ;
              rdfs:label "Fishing Tackle"@en .

DnD5eCharacter:FlaskOrTankard 	a rdfs:Class ;
              rdfs:subClassOf TTRpg:Tools ;
              rdfs:label "Flask Or Tankard"@en .

DnD5eCharacter:Flute 	a rdfs:Class ;
              rdfs:subClassOf TTRpg:Tools ;
              rdfs:label "Flute"@en .

DnD5eCharacter:ForgeryKit 	a rdfs:Class ;
              rdfs:subClassOf TTRpg:Tools ;
              rdfs:label "Forgery Kit"@en .

DnD5eCharacter:GrapplingHook 	a rdfs:Class ;
              rdfs:subClassOf TTRpg:Tools ;
              rdfs:label "Grappling Hook"@en .

DnD5eCharacter:Hammer 	a rdfs:Class ;
              rdfs:subClassOf TTRpg:Tools ;
              rdfs:label "Hammer"@en .

DnD5eCharacter:SledgeHammer 	a rdfs:Class ;
              rdfs:subClassOf TTRpg:Tools ;
              rdfs:label "Sledge Hammer"@en .

DnD5eCharacter:HerbalismKit 	a rdfs:Class ;
              rdfs:subClassOf TTRpg:Tools ;
              rdfs:label "Herbalism Kit"@en .

DnD5eCharacter:HolySymbol 	a rdfs:Class ;
              rdfs:subClassOf TTRpg:Tools ;
              rdfs:label "Holy Symbol"@en .

DnD5eCharacter:HolyWater 	a rdfs:Class ;
              rdfs:subClassOf TTRpg:Tools ;
              rdfs:label "Holy Water"@en .

DnD5eCharacter:Horn 	a rdfs:Class ;
              rdfs:subClassOf TTRpg:Tools ;
              rdfs:label "Horn"@en .

DnD5eCharacter:Hourglass 	a rdfs:Class ;
              rdfs:subClassOf TTRpg:Tools ;
              rdfs:label "Hourglass"@en .

DnD5eCharacter:HuntingTrap 	a rdfs:Class ;
              rdfs:subClassOf TTRpg:Tools ;
              rdfs:label "Hunting Trap"@en .

DnD5eCharacter:Incense 	a rdfs:Class ;
              rdfs:subClassOf TTRpg:Tools ;
              rdfs:label "Incense"@en .

DnD5eCharacter:Ink 	a rdfs:Class ;
              rdfs:subClassOf TTRpg:Tools ;
              rdfs:label "Ink"@en .

DnD5eCharacter:InkPen 	a rdfs:Class ;
              rdfs:subClassOf TTRpg:Tools ;
              rdfs:label "Ink Pen"@en .

DnD5eCharacter:Jug 	a rdfs:Class ;
              rdfs:subClassOf TTRpg:Tools ;
              rdfs:label "Jug"@en .

DnD5eCharacter:Pitcher 	a rdfs:Class ;
              rdfs:subClassOf TTRpg:Tools ;
              rdfs:label "Pitcher"@en .

DnD5eCharacter:SmallKnife 	a rdfs:Class ;
              rdfs:subClassOf TTRpg:Tools ;
              rdfs:label "Small Knife"@en .

DnD5eCharacter:Lamp 	a rdfs:Class ;
              rdfs:subClassOf TTRpg:Tools ;
              rdfs:label "Lamp"@en .

DnD5eCharacter:LandVehicles 	a rdfs:Class ;
              rdfs:subClassOf TTRpg:Tools ;
              rdfs:label "Land Vehicles"@en .

DnD5eCharacter:BullseyeLantern 	a rdfs:Class ;
              rdfs:subClassOf TTRpg:Tools ;
              rdfs:label "Bullseye Lantern"@en .

DnD5eCharacter:HoodedLantern 	a rdfs:Class ;
              rdfs:subClassOf TTRpg:Tools ;
              rdfs:label "Hooded Lantern"@en .

DnD5eCharacter:Lock 	a rdfs:Class ;
              rdfs:subClassOf TTRpg:Tools ;
              rdfs:label "Lock"@en .

DnD5eCharacter:Lute 	a rdfs:Class ;
              rdfs:subClassOf TTRpg:Tools ;
              rdfs:label "Lute"@en .

DnD5eCharacter:Lyre 	a rdfs:Class ;
              rdfs:subClassOf TTRpg:Tools ;
              rdfs:label "Lyre"@en .

DnD5eCharacter:MagnifyingGlass 	a rdfs:Class ;
              rdfs:subClassOf TTRpg:Tools ;
              rdfs:label "Magnifying Glass"@en .

DnD5eCharacter:Manacles 	a rdfs:Class ;
              rdfs:subClassOf TTRpg:Tools ;
              rdfs:label "Manacles"@en .

DnD5eCharacter:MessKit 	a rdfs:Class ;
              rdfs:subClassOf TTRpg:Tools ;
              rdfs:label "Mess Kit"@en .

DnD5eCharacter:SteelMirror 	a rdfs:Class ;
              rdfs:subClassOf TTRpg:Tools ;
              rdfs:label "Steel Mirror"@en .

DnD5eCharacter:Mule 	a rdfs:Class ;
              rdfs:subClassOf TTRpg:Tools ;
              rdfs:label "Mule"@en .

DnD5eCharacter:Oil 	a rdfs:Class ;
              rdfs:subClassOf TTRpg:Tools ;
              rdfs:label "Oil"@en .

DnD5eCharacter:Orb 	a rdfs:Class ;
              rdfs:subClassOf TTRpg:Tools ;
              rdfs:label "Orb"@en .

DnD5eCharacter:PanFlute 	a rdfs:Class ;
              rdfs:subClassOf TTRpg:Tools ;
              rdfs:label "Pan Flute"@en .

DnD5eCharacter:Paper 	a rdfs:Class ;
              rdfs:subClassOf TTRpg:Tools ;
              rdfs:label "Paper"@en .

DnD5eCharacter:Parchment 	a rdfs:Class ;
              rdfs:subClassOf TTRpg:Tools ;
              rdfs:label "Parchment"@en .

DnD5eCharacter:Perfume 	a rdfs:Class ;
              rdfs:subClassOf TTRpg:Tools ;
              rdfs:label "Perfume"@en .

DnD5eCharacter:Piton 	a rdfs:Class ;
              rdfs:subClassOf TTRpg:Tools ;
              rdfs:label "Piton"@en .

DnD5eCharacter:PlayingCardSet 	a rdfs:Class ;
              rdfs:subClassOf TTRpg:Tools ;
              rdfs:label "Playing Card Set"@en .

DnD5eCharacter:BasicPoison 	a rdfs:Class ;
              rdfs:subClassOf TTRpg:Tools ;
              rdfs:label "Basic Poison"@en .

DnD5eCharacter:IronPot 	a rdfs:Class ;
              rdfs:subClassOf TTRpg:Tools ;
              rdfs:label "Iron Pot"@en .

DnD5eCharacter:PotionOfHealing 	a rdfs:Class ;
              rdfs:subClassOf TTRpg:Tools ;
              rdfs:label "Potion Of Healing"@en .

DnD5eCharacter:Pouch 	a rdfs:Class ;
              rdfs:subClassOf TTRpg:Tools ;
              rdfs:label "Pouch"@en .

DnD5eCharacter:PrayerBook 	a rdfs:Class ;
              rdfs:subClassOf TTRpg:Tools ;
              rdfs:label "Prayer Book"@en .

DnD5eCharacter:PrayerWheel 	a rdfs:Class ;
              rdfs:subClassOf TTRpg:Tools ;
              rdfs:label "Prayer Wheel"@en .

DnD5eCharacter:Purse 	a rdfs:Class ;
              rdfs:subClassOf TTRpg:Tools ;
              rdfs:label "Purse"@en .

DnD5eCharacter:Quiver 	a rdfs:Class ;
              rdfs:subClassOf TTRpg:Tools ;
              rdfs:label "Quiver"@en .

DnD5eCharacter:PortableRam 	a rdfs:Class ;
              rdfs:subClassOf TTRpg:Tools ;
              rdfs:label "Portable Ram"@en .

DnD5eCharacter:Reliquary 	a rdfs:Class ;
              rdfs:subClassOf TTRpg:Tools ;
              rdfs:label "Reliquary"@en .

DnD5eCharacter:Robes 	a rdfs:Class ;
              rdfs:subClassOf TTRpg:Tools ;
              rdfs:label "Robes"@en .

DnD5eCharacter:Rod 	a rdfs:Class ;
              rdfs:subClassOf TTRpg:Tools ;
              rdfs:label "Rod"@en .

DnD5eCharacter:HempenRope 	a rdfs:Class ;
              rdfs:subClassOf TTRpg:Tools ;
              rdfs:label "Hempen Rope"@en .

DnD5eCharacter:SilkRope 	a rdfs:Class ;
              rdfs:subClassOf TTRpg:Tools ;
              rdfs:label "Silk Rope"@en .

DnD5eCharacter:Sack 	a rdfs:Class ;
              rdfs:subClassOf TTRpg:Tools ;
              rdfs:label "Sack"@en .

DnD5eCharacter:SealingWax 	a rdfs:Class ;
              rdfs:subClassOf TTRpg:Tools ;
              rdfs:label "Sealing Wax"@en .

DnD5eCharacter:Shawm 	a rdfs:Class ;
              rdfs:subClassOf TTRpg:Tools ;
              rdfs:label "Shawm"@en .

DnD5eCharacter:Shovel 	a rdfs:Class ;
              rdfs:subClassOf TTRpg:Tools ;
              rdfs:label "Shovel"@en .

DnD5eCharacter:SignalWhistle 	a rdfs:Class ;
              rdfs:subClassOf TTRpg:Tools ;
              rdfs:label "Signal Whistle"@en .

DnD5eCharacter:SignetRing 	a rdfs:Class ;
              rdfs:subClassOf TTRpg:Tools ;
              rdfs:label "Signet Ring"@en .

DnD5eCharacter:SlingBullet 	a rdfs:Class ;
              rdfs:subClassOf TTRpg:Tools ;
              rdfs:label "Sling Bullet"@en .

DnD5eCharacter:Soap 	a rdfs:Class ;
              rdfs:subClassOf TTRpg:Tools ;
              rdfs:label "Soap"@en .

DnD5eCharacter:Spellbook 	a rdfs:Class ;
              rdfs:subClassOf TTRpg:Tools ;
              rdfs:label "Spellbook"@en .

DnD5eCharacter:IronSpikes 	a rdfs:Class ;
              rdfs:subClassOf TTRpg:Tools ;
              rdfs:label "Iron Spikes"@en .

DnD5eCharacter:MistletoeSprig 	a rdfs:Class ;
              rdfs:subClassOf TTRpg:Tools ;
              rdfs:label "Mistletoe Sprig"@en .

DnD5eCharacter:Spyglass 	a rdfs:Class ;
              rdfs:subClassOf TTRpg:Tools ;
              rdfs:label "Spyglass"@en .

DnD5eCharacter:Staff 	a rdfs:Class ;
              rdfs:subClassOf TTRpg:Tools ;
              rdfs:label "Staff"@en .

DnD5eCharacter:String 	a rdfs:Class ;
              rdfs:subClassOf TTRpg:Tools ;
              rdfs:label "String"@en .

DnD5eCharacter:Tinderbox 	a rdfs:Class ;
              rdfs:subClassOf TTRpg:Tools ;
              rdfs:label "Tinderbox"@en .

DnD5eCharacter:Torch 	a rdfs:Class ;
              rdfs:subClassOf TTRpg:Tools ;
              rdfs:label "Torch"@en .

DnD5eCharacter:Totem 	a rdfs:Class ;
              rdfs:subClassOf TTRpg:Tools ;
              rdfs:label "Totem"@en .

DnD5eCharacter:Vestements 	a rdfs:Class ;
              rdfs:subClassOf TTRpg:Tools ;
              rdfs:label "Vestements"@en .

DnD5eCharacter:Vial 	a rdfs:Class ;
              rdfs:subClassOf TTRpg:Tools ;
              rdfs:label "Vial"@en .

DnD5eCharacter:Viol 	a rdfs:Class ;
              rdfs:subClassOf TTRpg:Tools ;
              rdfs:label "Viol"@en .

DnD5eCharacter:Wand 	a rdfs:Class ;
              rdfs:subClassOf TTRpg:Tools ;
              rdfs:label "Wand"@en .

DnD5eCharacter:WaterVehicles 	a rdfs:Class ;
              rdfs:subClassOf TTRpg:Tools ;
              rdfs:label "Water Vehicles"@en .

DnD5eCharacter:Waterskin 	a rdfs:Class ;
              rdfs:subClassOf TTRpg:Tools ;
              rdfs:label "Waterskin"@en .

DnD5eCharacter:Whetstone 	a rdfs:Class ;
              rdfs:subClassOf TTRpg:Tools ;
              rdfs:label "Whetstone"@en .

DnD5eCharacter:WoodenStake 	a rdfs:Class ;
              rdfs:subClassOf TTRpg:Tools ;
              rdfs:label "Wooden Stake"@en .

DnD5eCharacter:WoodenStaff 	a rdfs:Class ;
              rdfs:subClassOf TTRpg:Tools ;
              rdfs:label "Wooden Staff"@en .

DnD5eCharacter:YewWand 	a rdfs:Class ;
              rdfs:subClassOf TTRpg:Tools ;
              rdfs:label "Yew Wand"@en .

## D&D Magic Schools

DnD5eCharacter:MagicSchool 	a rdfs:Class ;
              rdfs:subClassOf TTRpg:SpellType ;
              rdfs:label "Magic School"@en .

DnD5eCharacter:Conjuration 	a rdfs:Class ;
              rdfs:subClassOf DnD5eCharacter:MagicSchool ;
              rdfs:label "Conjuration"@en .

DnD5eCharacter:Necromancy 	a rdfs:Class ;
              rdfs:subClassOf DnD5eCharacter:MagicSchool ;
              rdfs:label "Necromancy"@en .

DnD5eCharacter:Evocation 	a rdfs:Class ;
              rdfs:subClassOf DnD5eCharacter:MagicSchool ;
              rdfs:label "Evocation"@en .

DnD5eCharacter:Abjuration 	a rdfs:Class ;
              rdfs:subClassOf DnD5eCharacter:MagicSchool ;
              rdfs:label "Abjuration"@en .

DnD5eCharacter:Transmutation 	a rdfs:Class ;
              rdfs:subClassOf DnD5eCharacter:MagicSchool ;
              rdfs:label "Transmutation"@en .

DnD5eCharacter:Divination 	a rdfs:Class ;
              rdfs:subClassOf DnD5eCharacter:MagicSchool ;
              rdfs:label "Divination"@en .

DnD5eCharacter:Enchantment 	a rdfs:Class ;
              rdfs:subClassOf DnD5eCharacter:MagicSchool ;
              rdfs:label "Enchantment"@en .

DnD5eCharacter:Illusion 	a rdfs:Class ;
              rdfs:subClassOf DnD5eCharacter:MagicSchool ;
              rdfs:label "Illusion"@en .

## D&D Spells

DnD5eCharacter:AcidArrow 	a rdfs:Class ;
              rdfs:subClassOf TTRpg:Spell ;
              DnD5eCharacter:inMagicSchool DnD5eCharacter:Evocation ;
              rdfs:label "Acid Arrow"@en ;
              rdfs:comment "A shimmering green arrow streaks toward a target within range and bursts in a spray of acid. Make a ranged spell attack against the target. On a hit, the target takes 4d4 acid damage immediately and 2d4 acid damage at the end of its next turn. On a miss, the arrow splashes the target with acid for half as much of the initial damage and no damage at the end of its next turn."@en .

DnD5eCharacter:AcidSplash 	a rdfs:Class ;
              rdfs:subClassOf TTRpg:Spell ;
              DnD5eCharacter:inMagicSchool DnD5eCharacter:Conjuration ;
              rdfs:label "Acid Splash"@en ;
              rdfs:comment "You hurl a bubble of acid. Choose one creature within range, or choose two creatures within range that are within 5 feet of each other. A target must succeed on a dexterity saving throw or take 1d6 acid damage."@en .

DnD5eCharacter:Aid 	a rdfs:Class ;
              rdfs:subClassOf TTRpg:Spell ;
              DnD5eCharacter:inMagicSchool DnD5eCharacter:Abjuration ;
              rdfs:label "Aid"@en ;
              rdfs:comment "Your spell bolsters your allies with toughness and resolve. Choose up to three creatures within range. Each target's hit point maximum and current hit points increase by 5 for the duration."@en .

DnD5eCharacter:Alarm 	a rdfs:Class ;
              rdfs:subClassOf TTRpg:Spell ;
              DnD5eCharacter:inMagicSchool DnD5eCharacter:Abjuration ;
              rdfs:label "Alarm"@en ;
              rdfs:comment "You set an alarm against unwanted intrusion. Choose a door, a window, or an area within range that is no larger than a 20-foot cube. Until the spell ends, an alarm alerts you whenever a Tiny or larger creature touches or enters the warded area. When you cast the spell, you can designate creatures that won't set off the alarm. You also choose whether the alarm is mental or audible."@en .

DnD5eCharacter:AlterSelf 	a rdfs:Class ;
              rdfs:subClassOf TTRpg:Spell ;
              DnD5eCharacter:inMagicSchool DnD5eCharacter:Transmutation ;
              rdfs:label "Alter Self"@en ;
              rdfs:comment "You assume a different form. When you cast the spell, choose one of the following options, the effects of which last for the duration of the spell. While the spell lasts, you can end one option as an action to gain the benefits of a different one."@en .

DnD5eCharacter:AnimalFriendship 	a rdfs:Class ;
              rdfs:subClassOf TTRpg:Spell ;
              DnD5eCharacter:inMagicSchool DnD5eCharacter:Enchantment ;
              rdfs:label "Animal Friendship"@en ;
              rdfs:comment "This spell lets you convince a beast that you mean it no harm. Choose a beast that you can see within range. It must see and hear you. If the beast's Intelligence is 4 or higher, the spell fails. Otherwise, the beast must succeed on a wisdom saving throw or be charmed by you for the spell's duration. If you or one of your companions harms the target, the spells ends."@en .

DnD5eCharacter:AnimalMessenger 	a rdfs:Class ;
              rdfs:subClassOf TTRpg:Spell ;
              DnD5eCharacter:inMagicSchool DnD5eCharacter:Enchantment ;
              rdfs:label "Animal Messenger"@en ;
              rdfs:comment "By means of this spell, you use an animal to deliver a message. Choose a Tiny beast you can see within range, such as a squirrel, a blue jay, or a bat. You specify a location, which you must have visited, and a recipient who matches a general description, such as 'a man or woman dressed in the uniform of the town guard' or 'a red-haired dwarf wearing a pointed hat.' You also speak a message of up to twenty-five words. The target beast travels for the duration of the spell toward the specified location, covering about 50 miles per 24 hours for a flying messenger, or 25 miles for other animals."@en .

DnD5eCharacter:AnimalShapes 	a rdfs:Class ;
              rdfs:subClassOf TTRpg:Spell ;
              DnD5eCharacter:inMagicSchool DnD5eCharacter:Transmutation ;
              rdfs:label "Animal Shapes"@en ;
              rdfs:comment "Your magic turns others into beasts. Choose any number of willing creatures that you can see within range. You transform each target into the form of a Large or smaller beast with a challenge rating of 4 or lower. On subsequent turns, you can use your action to transform affected creatures into new forms."@en .

DnD5eCharacter:AnimateDead 	a rdfs:Class ;
              rdfs:subClassOf TTRpg:Spell ;
              DnD5eCharacter:inMagicSchool DnD5eCharacter:Necromancy ;
              rdfs:label "Animate Dead"@en ;
              rdfs:comment "This spell creates an undead servant. Choose a pile of bones or a corpse of a Medium or Small humanoid within range. Your spell imbues the target with a foul mimicry of life, raising it as an undead creature. The target becomes a skeleton if you chose bones or a zombie if you chose a corpse (the DM has the creature's game statistics)."@en .

DnD5eCharacter:AnimateObjects 	a rdfs:Class ;
              rdfs:subClassOf TTRpg:Spell ;
              DnD5eCharacter:inMagicSchool DnD5eCharacter:Transmutation ;
              rdfs:label "Animate Objects"@en ;
              rdfs:comment "Objects come to life at your command. Choose up to ten nonmagical objects within range that are not being worn or carried. Medium targets count as two objects, Large targets count as four objects, Huge targets count as eight objects. You can't animate any object larger than Huge. Each target animates and becomes a creature under your control until the spell ends or until reduced to 0 hit points."@en .

DnD5eCharacter:AntilifeShell 	a rdfs:Class ;
              rdfs:subClassOf TTRpg:Spell ;
              DnD5eCharacter:inMagicSchool DnD5eCharacter:Abjuration ;
              rdfs:label "Antilife Shell"@en ;
              rdfs:comment "A shimmering barrier extends out from you in a 10-foot radius and moves with you, remaining centered on you and hedging out creatures other than undead and constructs. The barrier lasts for the duration."@en .

DnD5eCharacter:AntimagicField 	a rdfs:Class ;
              rdfs:subClassOf TTRpg:Spell ;
              DnD5eCharacter:inMagicSchool DnD5eCharacter:Abjuration ;
              rdfs:label "Antimagic Field"@en ;
              rdfs:comment "A 10-foot-radius invisible sphere of antimagic surrounds you. This area is divorced from the magical energy that suffuses the multiverse. Within the sphere, spells can't be cast, summoned creatures disappear, and even magic items become mundane. Until the spell ends, the sphere moves with you, centered on you."@en .

DnD5eCharacter:AntipathySympathy 	a rdfs:Class ;
              rdfs:subClassOf TTRpg:Spell ;
              DnD5eCharacter:inMagicSchool DnD5eCharacter:Enchantment ;
              rdfs:label "Antipathy Sympathy"@en ;
              rdfs:comment "This spell attracts or repels creatures of your choice. You target something within range, either a Huge or smaller object or creature or an area that is no larger than a 200-foot cube. Then specify a kind of intelligent creature, such as red dragons, goblins, or vampires. You invest the target with an aura that either attracts or repels the specified creatures for the duration. Choose antipathy or sympathy as the aura's effect."@en .

DnD5eCharacter:ArcaneEye 	a rdfs:Class ;
              rdfs:subClassOf TTRpg:Spell ;
              DnD5eCharacter:inMagicSchool DnD5eCharacter:Divination ;
              rdfs:label "Arcane Eye"@en ;
              rdfs:comment "You create an invisible, magical eye within range that hovers in the air for the duration."@en .

DnD5eCharacter:ArcaneHand 	a rdfs:Class ;
              rdfs:subClassOf TTRpg:Spell ;
              DnD5eCharacter:inMagicSchool DnD5eCharacter:Evocation ;
              rdfs:label "Arcane Hand"@en ;
              rdfs:comment "You create a Large hand of shimmering, translucent force in an unoccupied space that you can see within range. The hand lasts for the spell's duration, and it moves at your command, mimicking the movements of your own hand."@en .

DnD5eCharacter:ArcaneLock 	a rdfs:Class ;
              rdfs:subClassOf TTRpg:Spell ;
              DnD5eCharacter:inMagicSchool DnD5eCharacter:Abjuration ;
              rdfs:label "Arcane Lock"@en ;
              rdfs:comment "You touch a closed door, window, gate, chest, or other entryway, and it becomes locked for the duration. You and the creatures you designate when you cast this spell can open the object normally. You can also set a password that, when spoken within 5 feet of the object, suppresses this spell for 1 minute. Otherwise, it is impassable until it is broken or the spell is dispelled or suppressed. Casting knock on the object suppresses arcane lock for 10 minutes."@en .

DnD5eCharacter:ArcaneSword 	a rdfs:Class ;
              rdfs:subClassOf TTRpg:Spell ;
              DnD5eCharacter:inMagicSchool DnD5eCharacter:Evocation ;
              rdfs:label "Arcane Sword"@en ;
              rdfs:comment "You create a sword-shaped plane of force that hovers within range. It lasts for the duration."@en .

DnD5eCharacter:ArcanistsMagicAura 	a rdfs:Class ;
              rdfs:subClassOf TTRpg:Spell ;
              DnD5eCharacter:inMagicSchool DnD5eCharacter:Illusion ;
              rdfs:label "Arcanists Magic Aura"@en ;
              rdfs:comment "You place an illusion on a creature or an object you touch so that divination spells reveal false information about it. The target can be a willing creature or an object that isn't being carried or worn by another creature."@en .

DnD5eCharacter:AstralProjection 	a rdfs:Class ;
              rdfs:subClassOf TTRpg:Spell ;
              DnD5eCharacter:inMagicSchool DnD5eCharacter:Necromancy ;
              rdfs:label "Astral Projection"@en ;
              rdfs:comment "You and up to eight willing creatures within range project your astral bodies into the Astral Plane (the spell fails and the casting is wasted if you are already on that plane). The material body you leave behind is unconscious and in a state of suspended animation; it doesn't need food or air and doesn't age."@en .

DnD5eCharacter:Augury 	a rdfs:Class ;
              rdfs:subClassOf TTRpg:Spell ;
              DnD5eCharacter:inMagicSchool DnD5eCharacter:Divination ;
              rdfs:label "Augury"@en ;
              rdfs:comment "By casting gem-inlaid sticks, rolling dragon bones, laying out ornate cards, or employing some other divining tool, you receive an omen from an otherworldly entity about the results of a specific course of action that you plan to take within the next 30 minutes. The DM chooses from the following possible omens:"@en .

DnD5eCharacter:Awaken 	a rdfs:Class ;
              rdfs:subClassOf TTRpg:Spell ;
              DnD5eCharacter:inMagicSchool DnD5eCharacter:Transmutation ;
              rdfs:label "Awaken"@en ;
              rdfs:comment "After spending the casting time tracing magical pathways within a precious gemstone, you touch a Huge or smaller beast or plant. The target must have either no Intelligence score or an Intelligence of 3 or less. The target gains an Intelligence of 10. The target also gains the ability to speak one language you know. If the target is a plant, it gains the ability to move its limbs, roots, vines, creepers, and so forth, and it gains senses similar to a human's. Your DM chooses statistics appropriate for the awakened plant, such as the statistics for the awakened shrub or the awakened tree."@en .

DnD5eCharacter:Bane 	a rdfs:Class ;
              rdfs:subClassOf TTRpg:Spell ;
              DnD5eCharacter:inMagicSchool DnD5eCharacter:Enchantment ;
              rdfs:label "Bane"@en ;
              rdfs:comment "Up to three creatures of your choice that you can see within range must make charisma saving throws. Whenever a target that fails this saving throw makes an attack roll or a saving throw before the spell ends, the target must roll a d4 and subtract the number rolled from the attack roll or saving throw."@en .

DnD5eCharacter:Banishment 	a rdfs:Class ;
              rdfs:subClassOf TTRpg:Spell ;
              DnD5eCharacter:inMagicSchool DnD5eCharacter:Abjuration ;
              rdfs:label "Banishment"@en ;
              rdfs:comment "You attempt to send one creature that you can see within range to another plane of existence. The target must succeed on a charisma saving throw or be banished."@en .

DnD5eCharacter:Barkskin 	a rdfs:Class ;
              rdfs:subClassOf TTRpg:Spell ;
              DnD5eCharacter:inMagicSchool DnD5eCharacter:Transmutation ;
              rdfs:label "Barkskin"@en ;
              rdfs:comment "You touch a willing creature. Until the spell ends, the target's skin has a rough, bark-like appearance, and the target's AC can't be less than 16, regardless of what kind of armor it is wearing."@en .

DnD5eCharacter:BeaconOfHope 	a rdfs:Class ;
              rdfs:subClassOf TTRpg:Spell ;
              DnD5eCharacter:inMagicSchool DnD5eCharacter:Abjuration ;
              rdfs:label "Beacon Of Hope"@en ;
              rdfs:comment "This spell bestows hope and vitality. Choose any number of creatures within range. For the duration, each target has advantage on wisdom saving throws and death saving throws, and regains the maximum number of hit points possible from any healing."@en .

DnD5eCharacter:BestowCurse 	a rdfs:Class ;
              rdfs:subClassOf TTRpg:Spell ;
              DnD5eCharacter:inMagicSchool DnD5eCharacter:Necromancy ;
              rdfs:label "Bestow Curse"@en ;
              rdfs:comment "You touch a creature, and that creature must succeed on a wisdom saving throw or become cursed for the duration of the spell. When you cast this spell, choose the nature of the curse from the following options:"@en .

DnD5eCharacter:BlackTentacles 	a rdfs:Class ;
              rdfs:subClassOf TTRpg:Spell ;
              DnD5eCharacter:inMagicSchool DnD5eCharacter:Conjuration ;
              rdfs:label "Black Tentacles"@en ;
              rdfs:comment "Squirming, ebony tentacles fill a 20-foot square on ground that you can see within range. For the duration, these tentacles turn the ground in the area into difficult terrain."@en .

DnD5eCharacter:BladeBarrier 	a rdfs:Class ;
              rdfs:subClassOf TTRpg:Spell ;
              DnD5eCharacter:inMagicSchool DnD5eCharacter:Evocation ;
              rdfs:label "Blade Barrier"@en ;
              rdfs:comment "You create a vertical wall of whirling, razor-sharp blades made of magical energy. The wall appears within range and lasts for the duration. You can make a straight wall up to 100 feet long, 20 feet high, and 5 feet thick, or a ringed wall up to 60 feet in diameter, 20 feet high, and 5 feet thick. The wall provides three-quarters cover to creatures behind it, and its space is difficult terrain."@en .

DnD5eCharacter:Bless 	a rdfs:Class ;
              rdfs:subClassOf TTRpg:Spell ;
              DnD5eCharacter:inMagicSchool DnD5eCharacter:Enchantment ;
              rdfs:label "Bless"@en ;
              rdfs:comment "You bless up to three creatures of your choice within range. Whenever a target makes an attack roll or a saving throw before the spell ends, the target can roll a d4 and add the number rolled to the attack roll or saving throw."@en .

DnD5eCharacter:Blight 	a rdfs:Class ;
              rdfs:subClassOf TTRpg:Spell ;
              DnD5eCharacter:inMagicSchool DnD5eCharacter:Necromancy ;
              rdfs:label "Blight"@en ;
              rdfs:comment "Necromantic energy washes over a creature of your choice that you can see within range, draining moisture and vitality from it. The target must make a constitution saving throw. The target takes 8d8 necrotic damage on a failed save, or half as much damage on a successful one. The spell has no effect on undead or constructs."@en .

DnD5eCharacter:BlindnessDeafness 	a rdfs:Class ;
              rdfs:subClassOf TTRpg:Spell ;
              DnD5eCharacter:inMagicSchool DnD5eCharacter:Necromancy ;
              rdfs:label "Blindness Deafness"@en ;
              rdfs:comment "You can blind or deafen a foe. Choose one creature that you can see within range to make a constitution saving throw. If it fails, the target is either blinded or deafened (your choice) for the duration. At the end of each of its turns, the target can make a constitution saving throw. On a success, the spell ends."@en .

DnD5eCharacter:Blink 	a rdfs:Class ;
              rdfs:subClassOf TTRpg:Spell ;
              DnD5eCharacter:inMagicSchool DnD5eCharacter:Transmutation ;
              rdfs:label "Blink"@en ;
              rdfs:comment "Roll a d20 at the end of each of your turns for the duration of the spell. On a roll of 11 or higher, you vanish from your current plane of existence and appear in the Ethereal Plane (the spell fails and the casting is wasted if you were already on that plane). At the start of your next turn, and when the spell ends if you are on the Ethereal Plane, you return to an unoccupied space of your choice that you can see within 10 feet of the space you vanished from. If no unoccupied space is available within that range, you appear in the nearest unoccupied space (chosen at random if more than one space is equally near). You can dismiss this spell as an action."@en .

DnD5eCharacter:Blur 	a rdfs:Class ;
              rdfs:subClassOf TTRpg:Spell ;
              DnD5eCharacter:inMagicSchool DnD5eCharacter:Illusion ;
              rdfs:label "Blur"@en ;
              rdfs:comment "Your body becomes blurred, shifting and wavering to all who can see you. For the duration, any creature has disadvantage on attack rolls against you. An attacker is immune to this effect if it doesn't rely on sight, as with blindsight, or can see through illusions, as with truesight."@en .

DnD5eCharacter:BrandingSmite 	a rdfs:Class ;
              rdfs:subClassOf TTRpg:Spell ;
              DnD5eCharacter:inMagicSchool DnD5eCharacter:Evocation ;
              rdfs:label "Branding Smite"@en ;
              rdfs:comment "The next time you hit a creature with a weapon attack before this spell ends, the weapon gleams with astral radiance as you strike. The attack deals an extra 2d6 radiant damage to the target, which becomes visible if it's invisible, and the target sheds dim light in a 5-foot radius and can't become invisible until the spell ends."@en .

DnD5eCharacter:BurningHands 	a rdfs:Class ;
              rdfs:subClassOf TTRpg:Spell ;
              DnD5eCharacter:inMagicSchool DnD5eCharacter:Evocation ;
              rdfs:label "Burning Hands"@en ;
              rdfs:comment "As you hold your hands with thumbs touching and fingers spread, a thin sheet of flames shoots forth from your outstretched fingertips. Each creature in a 15-foot cone must make a dexterity saving throw. A creature takes 3d6 fire damage on a failed save, or half as much damage on a successful one."@en .

DnD5eCharacter:CallLightning 	a rdfs:Class ;
              rdfs:subClassOf TTRpg:Spell ;
              DnD5eCharacter:inMagicSchool DnD5eCharacter:Conjuration ;
              rdfs:label "Call Lightning"@en ;
              rdfs:comment "A storm cloud appears in the shape of a cylinder that is 10 feet tall with a 60-foot radius, centered on a point you can see 100 feet directly above you. The spell fails if you can't see a point in the air where the storm cloud could appear (for example, if you are in a room that can't accommodate the cloud)."@en .

DnD5eCharacter:CalmEmotions 	a rdfs:Class ;
              rdfs:subClassOf TTRpg:Spell ;
              DnD5eCharacter:inMagicSchool DnD5eCharacter:Enchantment ;
              rdfs:label "Calm Emotions"@en ;
              rdfs:comment "You attempt to suppress strong emotions in a group of people. Each humanoid in a 20-foot-radius sphere centered on a point you choose within range must make a charisma saving throw; a creature can choose to fail this saving throw if it wishes. If a creature fails its saving throw, choose one of the following two effects. You can suppress any effect causing a target to be charmed or frightened. When this spell ends, any suppressed effect resumes, provided that its duration has not expired in the meantime."@en .

DnD5eCharacter:ChainLightning 	a rdfs:Class ;
              rdfs:subClassOf TTRpg:Spell ;
              DnD5eCharacter:inMagicSchool DnD5eCharacter:Evocation ;
              rdfs:label "Chain Lightning"@en ;
              rdfs:comment "You create a bolt of lightning that arcs toward a target of your choice that you can see within range. Three bolts then leap from that target to as many as three other targets, each of which must be within 30 feet of the first target. A target can be a creature or an object and can be targeted by only one of the bolts."@en .

DnD5eCharacter:CharmPerson 	a rdfs:Class ;
              rdfs:subClassOf TTRpg:Spell ;
              DnD5eCharacter:inMagicSchool DnD5eCharacter:Enchantment ;
              rdfs:label "Charm Person"@en ;
              rdfs:comment "You attempt to charm a humanoid you can see within range. It must make a wisdom saving throw, and does so with advantage if you or your companions are fighting it. If it fails the saving throw, it is charmed by you until the spell ends or until you or your companions do anything harmful to it. The charmed creature regards you as a friendly acquaintance. When the spell ends, the creature knows it was charmed by you."@en .

DnD5eCharacter:ChillTouch 	a rdfs:Class ;
              rdfs:subClassOf TTRpg:Spell ;
              DnD5eCharacter:inMagicSchool DnD5eCharacter:Necromancy ;
              rdfs:label "Chill Touch"@en ;
              rdfs:comment "You create a ghostly, skeletal hand in the space of a creature within range. Make a ranged spell attack against the creature to assail it with the chill of the grave. On a hit, the target takes 1d8 necrotic damage, and it can't regain hit points until the start of your next turn. Until then, the hand clings to the target."@en .

DnD5eCharacter:CircleOfDeath 	a rdfs:Class ;
              rdfs:subClassOf TTRpg:Spell ;
              DnD5eCharacter:inMagicSchool DnD5eCharacter:Necromancy ;
              rdfs:label "Circle Of Death"@en ;
              rdfs:comment "A sphere of negative energy ripples out in a 60-foot radius sphere from a point within range. Each creature in that area must make a constitution saving throw. A target takes 8d6 necrotic damage on a failed save, or half as much damage on a successful one."@en .

DnD5eCharacter:Clairvoyance 	a rdfs:Class ;
              rdfs:subClassOf TTRpg:Spell ;
              DnD5eCharacter:inMagicSchool DnD5eCharacter:Divination ;
              rdfs:label "Clairvoyance"@en ;
              rdfs:comment "You create an invisible sensor within range in a location familiar to you (a place you have visited or seen before) or in an obvious location that is unfamiliar to you (such as behind a door, around a corner, or in a grove of trees). The sensor remains in place for the duration, and it can't be attacked or otherwise interacted with."@en .

DnD5eCharacter:Clone 	a rdfs:Class ;
              rdfs:subClassOf TTRpg:Spell ;
              DnD5eCharacter:inMagicSchool DnD5eCharacter:Necromancy ;
              rdfs:label "Clone"@en ;
              rdfs:comment "This spell grows an inert duplicate of a living creature as a safeguard against death. This clone forms inside a sealed vessel and grows to full size and maturity after 120 days; you can also choose to have the clone be a younger version of the same creature. It remains inert and endures indefinitely, as long as its vessel remains undisturbed."@en .

DnD5eCharacter:Cloudkill 	a rdfs:Class ;
              rdfs:subClassOf TTRpg:Spell ;
              DnD5eCharacter:inMagicSchool DnD5eCharacter:Conjuration ;
              rdfs:label "Cloudkill"@en ;
              rdfs:comment "You create a 20-foot-radius sphere of poisonous, yellow-green fog centered on a point you choose within range. The fog spreads around corners. It lasts for the duration or until strong wind disperses the fog, ending the spell. Its area is heavily obscured."@en .

DnD5eCharacter:ColorSpray 	a rdfs:Class ;
              rdfs:subClassOf TTRpg:Spell ;
              DnD5eCharacter:inMagicSchool DnD5eCharacter:Illusion ;
              rdfs:label "Color Spray"@en ;
              rdfs:comment "A dazzling array of flashing, colored light springs from your hand. Roll 6d10; the total is how many hit points of creatures this spell can effect. Creatures in a 15-foot cone originating from you are affected in ascending order of their current hit points (ignoring unconscious creatures and creatures that can't see)."@en .

DnD5eCharacter:Command 	a rdfs:Class ;
              rdfs:subClassOf TTRpg:Spell ;
              DnD5eCharacter:inMagicSchool DnD5eCharacter:Enchantment ;
              rdfs:label "Command"@en ;
              rdfs:comment "You speak a one-word command to a creature you can see within range. The target must succeed on a wisdom saving throw or follow the command on its next turn. The spell has no effect if the target is undead, if it doesn't understand your language, or if your command is directly harmful to it."@en .

DnD5eCharacter:Commune 	a rdfs:Class ;
              rdfs:subClassOf TTRpg:Spell ;
              DnD5eCharacter:inMagicSchool DnD5eCharacter:Divination ;
              rdfs:label "Commune"@en ;
              rdfs:comment "You contact your deity or a divine proxy and ask up to three questions that can be answered with a yes or no. You must ask your questions before the spell ends. You receive a correct answer for each question."@en .

DnD5eCharacter:CommuneWithNature 	a rdfs:Class ;
              rdfs:subClassOf TTRpg:Spell ;
              DnD5eCharacter:inMagicSchool DnD5eCharacter:Divination ;
              rdfs:label "Commune With Nature"@en ;
              rdfs:comment "You briefly become one with nature and gain knowledge of the surrounding territory. In the outdoors, the spell gives you knowledge of the land within 3 miles of you. In caves and other natural underground settings, the radius is limited to 300 feet. The spell doesn't function where nature has been replaced by construction, such as in dungeons and towns."@en .

DnD5eCharacter:ComprehendLanguages 	a rdfs:Class ;
              rdfs:subClassOf TTRpg:Spell ;
              DnD5eCharacter:inMagicSchool DnD5eCharacter:Divination ;
              rdfs:label "Comprehend Languages"@en ;
              rdfs:comment "For the duration, you understand the literal meaning of any spoken language that you hear. You also understand any written language that you see, but you must be touching the surface on which the words are written. It takes about 1 minute to read one page of text."@en .

DnD5eCharacter:Compulsion 	a rdfs:Class ;
              rdfs:subClassOf TTRpg:Spell ;
              DnD5eCharacter:inMagicSchool DnD5eCharacter:Enchantment ;
              rdfs:label "Compulsion"@en ;
              rdfs:comment "Creatures of your choice that you can see within range and that can hear you must make a wisdom saving throw. A target automatically succeeds on this saving throw if it can't be charmed. On a failed save, a target is affected by this spell. Until the spell ends, you can use a bonus action on each of your turns to designate a direction that is horizontal to you. Each affected target must use as much of its movement as possible to move in that direction on its next turn. It can take any action before it moves. After moving in this way, it can make another Wisdom save to try to end the effect."@en .

DnD5eCharacter:ConeOfCold 	a rdfs:Class ;
              rdfs:subClassOf TTRpg:Spell ;
              DnD5eCharacter:inMagicSchool DnD5eCharacter:Evocation ;
              rdfs:label "Cone Of Cold"@en ;
              rdfs:comment "A blast of cold air erupts from your hands. Each creature in a 60-foot cone must make a constitution saving throw. A creature takes 8d8 cold damage on a failed save, or half as much damage on a successful one."@en .

DnD5eCharacter:Confusion 	a rdfs:Class ;
              rdfs:subClassOf TTRpg:Spell ;
              DnD5eCharacter:inMagicSchool DnD5eCharacter:Enchantment ;
              rdfs:label "Confusion"@en ;
              rdfs:comment "This spell assaults and twists creatures' minds, spawning delusions and provoking uncontrolled action. Each creature in a 10-foot-radius sphere centered on a point you choose within range must succeed on a Wisdom saving throw when you cast this spell or be affected by it."@en .

DnD5eCharacter:ConjureAnimals 	a rdfs:Class ;
              rdfs:subClassOf TTRpg:Spell ;
              DnD5eCharacter:inMagicSchool DnD5eCharacter:Conjuration ;
              rdfs:label "Conjure Animals"@en ;
              rdfs:comment "You summon fey spirits that take the form of beasts and appear in unoccupied spaces that you can see within range. Choose one of the following options for what appears:"@en .

DnD5eCharacter:ConjureCelestial 	a rdfs:Class ;
              rdfs:subClassOf TTRpg:Spell ;
              DnD5eCharacter:inMagicSchool DnD5eCharacter:Conjuration ;
              rdfs:label "Conjure Celestial"@en ;
              rdfs:comment "You summon a celestial of challenge rating 4 or lower, which appears in an unoccupied space that you can see within range. The celestial disappears when it drops to 0 hit points or when the spell ends."@en .

DnD5eCharacter:ConjureElemental 	a rdfs:Class ;
              rdfs:subClassOf TTRpg:Spell ;
              DnD5eCharacter:inMagicSchool DnD5eCharacter:Conjuration ;
              rdfs:label "Conjure Elemental"@en ;
              rdfs:comment "You call forth an elemental servant. Choose an area of air, earth, fire, or water that fills a 10-foot cube within range. An elemental of challenge rating 5 or lower appropriate to the area you chose appears in an unoccupied space within 10 feet of it. For example, a fire elemental emerges from a bonfire, and an earth elemental rises up from the ground. The elemental disappears when it drops to 0 hit points or when the spell ends."@en .

DnD5eCharacter:ConjureFey 	a rdfs:Class ;
              rdfs:subClassOf TTRpg:Spell ;
              DnD5eCharacter:inMagicSchool DnD5eCharacter:Conjuration ;
              rdfs:label "Conjure Fey"@en ;
              rdfs:comment "You summon a fey creature of challenge rating 6 or lower, or a fey spirit that takes the form of a beast of challenge rating 6 or lower. It appears in an unoccupied space that you can see within range. The fey creature disappears when it drops to 0 hit points or when the spell ends."@en .

DnD5eCharacter:ConjureMinorElementals 	a rdfs:Class ;
              rdfs:subClassOf TTRpg:Spell ;
              DnD5eCharacter:inMagicSchool DnD5eCharacter:Conjuration ;
              rdfs:label "Conjure Minor Elementals"@en ;
              rdfs:comment "You summon elementals that appear in unoccupied spaces that you can see within range. You choose one the following options for what appears:"@en .

DnD5eCharacter:ConjureWoodlandBeings 	a rdfs:Class ;
              rdfs:subClassOf TTRpg:Spell ;
              DnD5eCharacter:inMagicSchool DnD5eCharacter:Conjuration ;
              rdfs:label "Conjure Woodland Beings"@en ;
              rdfs:comment "You summon fey creatures that appear in unoccupied spaces that you can see within range. Choose one of the following options for what appears:"@en .

DnD5eCharacter:ContactOtherPlane 	a rdfs:Class ;
              rdfs:subClassOf TTRpg:Spell ;
              DnD5eCharacter:inMagicSchool DnD5eCharacter:Divination ;
              rdfs:label "Contact Other Plane"@en ;
              rdfs:comment "You mentally contact a demigod, the spirit of a long-dead sage, or some other mysterious entity from another plane. Contacting this extraplanar intelligence can strain or even break your mind. When you cast this spell, make a DC 15 intelligence saving throw. On a failure, you take 6d6 psychic damage and are insane until you finish a long rest. While insane, you can't take actions, can't understand what other creatures say, can't read, and speak only in gibberish. A greater restoration spell cast on you ends this effect."@en .

DnD5eCharacter:Contagion 	a rdfs:Class ;
              rdfs:subClassOf TTRpg:Spell ;
              DnD5eCharacter:inMagicSchool DnD5eCharacter:Necromancy ;
              rdfs:label "Contagion"@en ;
              rdfs:comment "Your touch inflicts disease. Make a melee spell attack against a creature within your reach. On a hit, you afflict the creature with a disease of your choice from any of the ones described below."@en .

DnD5eCharacter:Contingency 	a rdfs:Class ;
              rdfs:subClassOf TTRpg:Spell ;
              DnD5eCharacter:inMagicSchool DnD5eCharacter:Evocation ;
              rdfs:label "Contingency"@en ;
              rdfs:comment "Choose a spell of 5th level or lower that you can cast, that has a casting time of 1 action, and that can target you. You cast that spell--called the contingent spell--as part of casting contingency, expending spell slots for both, but the contingent spell doesn't come into effect. Instead, it takes effect when a certain circumstance occurs. You describe that circumstance when you cast the two spells. For example, a contingency cast with water breathing might stipulate that water breathing comes into effect when you are engulfed in water or a similar liquid."@en .

DnD5eCharacter:ContinualFlame 	a rdfs:Class ;
              rdfs:subClassOf TTRpg:Spell ;
              DnD5eCharacter:inMagicSchool DnD5eCharacter:Evocation ;
              rdfs:label "Continual Flame"@en ;
              rdfs:comment "A flame, equivalent in brightness to a torch, springs forth from an object that you touch. The effect looks like a regular flame, but it creates no heat and doesn't use oxygen. A continual flame can be covered or hidden but not smothered or quenched."@en .

DnD5eCharacter:ControlWater 	a rdfs:Class ;
              rdfs:subClassOf TTRpg:Spell ;
              DnD5eCharacter:inMagicSchool DnD5eCharacter:Transmutation ;
              rdfs:label "Control Water"@en ;
              rdfs:comment "Until the spell ends, you control any freestanding water inside an area you choose that is a cube up to 100 feet on a side. You can choose from any of the following effects when you cast this spell. As an action on your turn, you can repeat the same effect or choose a different one."@en .

DnD5eCharacter:ControlWeather 	a rdfs:Class ;
              rdfs:subClassOf TTRpg:Spell ;
              DnD5eCharacter:inMagicSchool DnD5eCharacter:Transmutation ;
              rdfs:label "Control Weather"@en ;
              rdfs:comment "You take control of the weather within 5 miles of you for the duration. You must be outdoors to cast this spell. Moving to a place where you don't have a clear path to the sky ends the spell early."@en .

DnD5eCharacter:Counterspell 	a rdfs:Class ;
              rdfs:subClassOf TTRpg:Spell ;
              DnD5eCharacter:inMagicSchool DnD5eCharacter:Abjuration ;
              rdfs:label "Counterspell"@en ;
              rdfs:comment "You attempt to interrupt a creature in the process of casting a spell. If the creature is casting a spell of 3rd level or lower, its spell fails and has no effect. If it is casting a spell of 4th level or higher, make an ability check using your spellcasting ability. The DC equals 10 + the spell's level. On a success, the creature's spell fails and has no effect."@en .

DnD5eCharacter:CreateFoodAndWater 	a rdfs:Class ;
              rdfs:subClassOf TTRpg:Spell ;
              DnD5eCharacter:inMagicSchool DnD5eCharacter:Conjuration ;
              rdfs:label "Create Food And Water"@en ;
              rdfs:comment "You create 45 pounds of food and 30 gallons of water on the ground or in containers within range, enough to sustain up to fifteen humanoids or five steeds for 24 hours. The food is bland but nourishing, and spoils if uneaten after 24 hours. The water is clean and doesn't go bad."@en .

DnD5eCharacter:CreateOrDestroyWater 	a rdfs:Class ;
              rdfs:subClassOf TTRpg:Spell ;
              DnD5eCharacter:inMagicSchool DnD5eCharacter:Transmutation ;
              rdfs:label "Create Or Destroy Water"@en ;
              rdfs:comment "You either create or destroy water."@en .

DnD5eCharacter:CreateUndead 	a rdfs:Class ;
              rdfs:subClassOf TTRpg:Spell ;
              DnD5eCharacter:inMagicSchool DnD5eCharacter:Necromancy ;
              rdfs:label "Create Undead"@en ;
              rdfs:comment "You can cast this spell only at night. Choose up to three corpses of Medium or Small humanoids within range. Each corpse becomes a ghoul under your control. (The DM has game statistics for these creatures.)"@en .

DnD5eCharacter:Creation 	a rdfs:Class ;
              rdfs:subClassOf TTRpg:Spell ;
              DnD5eCharacter:inMagicSchool DnD5eCharacter:Illusion ;
              rdfs:label "Creation"@en ;
              rdfs:comment "You pull wisps of shadow material from the Shadowfell to create a nonliving object of vegetable matter within range: soft goods, rope, wood, or something similar. You can also use this spell to create mineral objects such as stone, crystal, or metal. The object created must be no larger than a 5-foot cube, and the object must be of a form and material that you have seen before."@en .

DnD5eCharacter:CureWounds 	a rdfs:Class ;
              rdfs:subClassOf TTRpg:Spell ;
              DnD5eCharacter:inMagicSchool DnD5eCharacter:Evocation ;
              rdfs:label "Cure Wounds"@en ;
              rdfs:comment "A creature you touch regains a number of hit points equal to 1d8 + your spellcasting ability modifier. This spell has no effect on undead or constructs."@en .

DnD5eCharacter:DancingLights 	a rdfs:Class ;
              rdfs:subClassOf TTRpg:Spell ;
              DnD5eCharacter:inMagicSchool DnD5eCharacter:Evocation ;
              rdfs:label "Dancing Lights"@en ;
              rdfs:comment "You create up to four torch-sized lights within range, making them appear as torches, lanterns, or glowing orbs that hover in the air for the duration. You can also combine the four lights into one glowing vaguely humanoid form of Medium size. Whichever form you choose, each light sheds dim light in a 10-foot radius."@en .

DnD5eCharacter:Darkness 	a rdfs:Class ;
              rdfs:subClassOf TTRpg:Spell ;
              DnD5eCharacter:inMagicSchool DnD5eCharacter:Evocation ;
              rdfs:label "Darkness"@en ;
              rdfs:comment "Magical darkness spreads from a point you choose within range to fill a 15-foot-radius sphere for the duration. The darkness spreads around corners. A creature with darkvision can't see through this darkness, and nonmagical light can't illuminate it."@en .

DnD5eCharacter:Darkvision 	a rdfs:Class ;
              rdfs:subClassOf TTRpg:Spell ;
              DnD5eCharacter:inMagicSchool DnD5eCharacter:Transmutation ;
              rdfs:label "Darkvision"@en ;
              rdfs:comment "You touch a willing creature to grant it the ability to see in the dark. For the duration, that creature has darkvision out to a range of 60 feet."@en .

DnD5eCharacter:Daylight 	a rdfs:Class ;
              rdfs:subClassOf TTRpg:Spell ;
              DnD5eCharacter:inMagicSchool DnD5eCharacter:Evocation ;
              rdfs:label "Daylight"@en ;
              rdfs:comment "A 60-foot-radius sphere of light spreads out from a point you choose within range. The sphere is bright light and sheds dim light for an additional 60 feet."@en .

DnD5eCharacter:DeathWard 	a rdfs:Class ;
              rdfs:subClassOf TTRpg:Spell ;
              DnD5eCharacter:inMagicSchool DnD5eCharacter:Abjuration ;
              rdfs:label "Death Ward"@en ;
              rdfs:comment "You touch a creature and grant it a measure of protection from death."@en .

DnD5eCharacter:DelayedBlastFireball 	a rdfs:Class ;
              rdfs:subClassOf TTRpg:Spell ;
              DnD5eCharacter:inMagicSchool DnD5eCharacter:Evocation ;
              rdfs:label "Delayed Blast Fireball"@en ;
              rdfs:comment "A beam of yellow light flashes from your pointing finger, then condenses to linger at a chosen point within range as a glowing bead for the duration. When the spell ends, either because your concentration is broken or because you decide to end it, the bead blossoms with a low roar into an explosion of flame that spreads around corners. Each creature in a 20-foot-radius sphere centered on that point must make a dexterity saving throw. A creature takes fire damage equal to the total accumulated damage on a failed save, or half as much damage on a successful one."@en .

DnD5eCharacter:Demiplane 	a rdfs:Class ;
              rdfs:subClassOf TTRpg:Spell ;
              DnD5eCharacter:inMagicSchool DnD5eCharacter:Conjuration ;
              rdfs:label "Demiplane"@en ;
              rdfs:comment "You create a shadowy door on a flat solid surface that you can see within range. The door is large enough to allow Medium creatures to pass through unhindered. When opened, the door leads to a demiplane that appears to be an empty room 30 feet in each dimension, made of wood or stone. When the spell ends, the door disappears, and any creatures or objects inside the demiplane remain trapped there, as the door also disappears from the other side."@en .

DnD5eCharacter:DetectEvilAndGood 	a rdfs:Class ;
              rdfs:subClassOf TTRpg:Spell ;
              DnD5eCharacter:inMagicSchool DnD5eCharacter:Divination ;
              rdfs:label "Detect Evil And Good"@en ;
              rdfs:comment "For the duration, you know if there is an aberration, celestial, elemental, fey, fiend, or undead within 30 feet of you, as well as where the creature is located. Similarly, you know if there is a place or object within 30 feet of you that has been magically consecrated or desecrated."@en .

DnD5eCharacter:DetectMagic 	a rdfs:Class ;
              rdfs:subClassOf TTRpg:Spell ;
              DnD5eCharacter:inMagicSchool DnD5eCharacter:Divination ;
              rdfs:label "Detect Magic"@en ;
              rdfs:comment "For the duration, you sense the presence of magic within 30 feet of you. If you sense magic in this way, you can use your action to see a faint aura around any visible creature or object in the area that bears magic, and you learn its school of magic, if any."@en .

DnD5eCharacter:DetectPoisonAndDisease 	a rdfs:Class ;
              rdfs:subClassOf TTRpg:Spell ;
              DnD5eCharacter:inMagicSchool DnD5eCharacter:Divination ;
              rdfs:label "Detect Poison And Disease"@en ;
              rdfs:comment "For the duration, you can sense the presence and location of poisons, poisonous creatures, and diseases within 30 feet of you. You also identify the kind of poison, poisonous creature, or disease in each case."@en .

DnD5eCharacter:DetectThoughts 	a rdfs:Class ;
              rdfs:subClassOf TTRpg:Spell ;
              DnD5eCharacter:inMagicSchool DnD5eCharacter:Divination ;
              rdfs:label "Detect Thoughts"@en ;
              rdfs:comment "For the duration, you can read the thoughts of certain creatures. When you cast the spell and as your action on each turn until the spell ends, you can focus your mind on any one creature that you can see within 30 feet of you. If the creature you choose has an Intelligence of 3 or lower or doesn't speak any language, the creature is unaffected."@en .

DnD5eCharacter:DimensionDoor 	a rdfs:Class ;
              rdfs:subClassOf TTRpg:Spell ;
              DnD5eCharacter:inMagicSchool DnD5eCharacter:Conjuration ;
              rdfs:label "Dimension Door"@en ;
              rdfs:comment "You teleport yourself from your current location to any other spot within range. You arrive at exactly the spot desired. It can be a place you can see, one you can visualize, or one you can describe by stating distance and direction, such as '200 feet straight downward' or 'upward to the northwest at a 45-degree angle, 300 feet.'"@en .

DnD5eCharacter:DisguiseSelf 	a rdfs:Class ;
              rdfs:subClassOf TTRpg:Spell ;
              DnD5eCharacter:inMagicSchool DnD5eCharacter:Illusion ;
              rdfs:label "Disguise Self"@en ;
              rdfs:comment "You make yourself--including your clothing, armor, weapons, and other belongings on your person--look different until the spell ends or until you use your action to dismiss it. You can seem 1 foot shorter or taller and can appear thin, fat, or in between. You can't change your body type, so you must adopt a form that has the same basic arrangement of limbs. Otherwise, the extent of the illusion is up to you."@en .

DnD5eCharacter:Disintegrate 	a rdfs:Class ;
              rdfs:subClassOf TTRpg:Spell ;
              DnD5eCharacter:inMagicSchool DnD5eCharacter:Transmutation ;
              rdfs:label "Disintegrate"@en ;
              rdfs:comment "A thin green ray springs from your pointing finger to a target that you can see within range. The target can be a creature, an object, or a creation of magical force, such as the wall created by wall of force."@en .

DnD5eCharacter:DispelEvilAndGood 	a rdfs:Class ;
              rdfs:subClassOf TTRpg:Spell ;
              DnD5eCharacter:inMagicSchool DnD5eCharacter:Abjuration ;
              rdfs:label "Dispel Evil And Good"@en ;
              rdfs:comment "Shimmering energy surrounds and protects you from fey, undead, and creatures originating from beyond the Material Plane. For the duration, celestials, elementals, fey, fiends, and undead have disadvantage on attack rolls against you."@en .

DnD5eCharacter:DispelMagic 	a rdfs:Class ;
              rdfs:subClassOf TTRpg:Spell ;
              DnD5eCharacter:inMagicSchool DnD5eCharacter:Abjuration ;
              rdfs:label "Dispel Magic"@en ;
              rdfs:comment "Choose one creature, object, or magical effect within range. Any spell of 3rd level or lower on the target ends. For each spell of 4th level or higher on the target, make an ability check using your spellcasting ability. The DC equals 10 + the spell's level. On a successful check, the spell ends."@en .

DnD5eCharacter:Divination 	a rdfs:Class ;
              rdfs:subClassOf TTRpg:Spell ;
              DnD5eCharacter:inMagicSchool DnD5eCharacter:Divination ;
              rdfs:label "Divination"@en ;
              rdfs:comment "Your magic and an offering put you in contact with a god or a god's servants. You ask a single question concerning a specific goal, event, or activity to occur within 7 days. The DM offers a truthful reply. The reply might be a short phrase, a cryptic rhyme, or an omen."@en .

DnD5eCharacter:DivineFavor 	a rdfs:Class ;
              rdfs:subClassOf TTRpg:Spell ;
              DnD5eCharacter:inMagicSchool DnD5eCharacter:Evocation ;
              rdfs:label "Divine Favor"@en ;
              rdfs:comment "Your prayer empowers you with divine radiance. Until the spell ends, your weapon attacks deal an extra 1d4 radiant damage on a hit."@en .

DnD5eCharacter:DivineWord 	a rdfs:Class ;
              rdfs:subClassOf TTRpg:Spell ;
              DnD5eCharacter:inMagicSchool DnD5eCharacter:Evocation ;
              rdfs:label "Divine Word"@en ;
              rdfs:comment "You utter a divine word, imbued with the power that shaped the world at the dawn of creation. Choose any number of creatures you can see within range. Each creature that can hear you must make a Charisma saving throw. On a failed save, a creature suffers an effect based on its current hit points:"@en .

DnD5eCharacter:DominateBeast 	a rdfs:Class ;
              rdfs:subClassOf TTRpg:Spell ;
              DnD5eCharacter:inMagicSchool DnD5eCharacter:Enchantment ;
              rdfs:label "Dominate Beast"@en ;
              rdfs:comment "You attempt to beguile a creature that you can see within range. It must succeed on a wisdom saving throw or be charmed by you for the duration. If you or creatures that are friendly to you are fighting it, it has advantage on the saving throw."@en .

DnD5eCharacter:DominateMonster 	a rdfs:Class ;
              rdfs:subClassOf TTRpg:Spell ;
              DnD5eCharacter:inMagicSchool DnD5eCharacter:Enchantment ;
              rdfs:label "Dominate Monster"@en ;
              rdfs:comment "You attempt to beguile a creature that you can see within range. It must succeed on a wisdom saving throw or be charmed by you for the duration. If you or creatures that are friendly to you are fighting it, it has advantage on the saving throw."@en .

DnD5eCharacter:DominatePerson 	a rdfs:Class ;
              rdfs:subClassOf TTRpg:Spell ;
              DnD5eCharacter:inMagicSchool DnD5eCharacter:Enchantment ;
              rdfs:label "Dominate Person"@en ;
              rdfs:comment "You attempt to beguile a humanoid that you can see within range. It must succeed on a wisdom saving throw or be charmed by you for the duration. If you or creatures that are friendly to you are fighting it, it has advantage on the saving throw."@en .

DnD5eCharacter:Dream 	a rdfs:Class ;
              rdfs:subClassOf TTRpg:Spell ;
              DnD5eCharacter:inMagicSchool DnD5eCharacter:Illusion ;
              rdfs:label "Dream"@en ;
              rdfs:comment "This spell shapes a creature's dreams. Choose a creature known to you as the target of this spell. The target must be on the same plane of existence as you. Creatures that don't sleep, such as elves, can't be contacted by this spell. You, or a willing creature you touch, enters a trance state, acting as a messenger."@en .

DnD5eCharacter:Druidcraft 	a rdfs:Class ;
              rdfs:subClassOf TTRpg:Spell ;
              DnD5eCharacter:inMagicSchool DnD5eCharacter:Transmutation ;
              rdfs:label "Druidcraft"@en ;
              rdfs:comment "Whispering to the spirits of nature, you create one of the following effects within 'range':"@en .

DnD5eCharacter:Earthquake 	a rdfs:Class ;
              rdfs:subClassOf TTRpg:Spell ;
              DnD5eCharacter:inMagicSchool DnD5eCharacter:Evocation ;
              rdfs:label "Earthquake"@en ;
              rdfs:comment "You create a seismic disturbance at a point on the ground that you can see within range. For the duration, an intense tremor rips through the ground in a 100-foot-radius circle centered on that point and shakes creatures and structures in contact with the ground in that area."@en .

DnD5eCharacter:EldritchBlast 	a rdfs:Class ;
              rdfs:subClassOf TTRpg:Spell ;
              DnD5eCharacter:inMagicSchool DnD5eCharacter:Evocation ;
              rdfs:label "Eldritch Blast"@en ;
              rdfs:comment "A beam of crackling energy streaks toward a creature within range. Make a ranged spell attack against the target. On a hit, the target takes 1d10 force damage. The spell creates more than one beam when you reach higher levels: two beams at 5th level, three beams at 11th level, and four beams at 17th level. You can direct the beams at the same target or at different ones. Make a separate attack roll for each beam."@en .

DnD5eCharacter:EnhanceAbility 	a rdfs:Class ;
              rdfs:subClassOf TTRpg:Spell ;
              DnD5eCharacter:inMagicSchool DnD5eCharacter:Transmutation ;
              rdfs:label "Enhance Ability"@en ;
              rdfs:comment "You touch a creature and bestow upon it a magical enhancement. Choose one of the following effects; the target gains that effect until the spell ends."@en .

DnD5eCharacter:EnlargeReduce 	a rdfs:Class ;
              rdfs:subClassOf TTRpg:Spell ;
              DnD5eCharacter:inMagicSchool DnD5eCharacter:Transmutation ;
              rdfs:label "Enlarge Reduce"@en ;
              rdfs:comment "You cause a creature or an object you can see within range to grow larger or smaller for the duration. Choose either a creature or an object that is neither worn nor carried. If the target is unwilling, it can make a Constitution saving throw. On a success, the spell has no effect."@en .

DnD5eCharacter:Entangle 	a rdfs:Class ;
              rdfs:subClassOf TTRpg:Spell ;
              DnD5eCharacter:inMagicSchool DnD5eCharacter:Conjuration ;
              rdfs:label "Entangle"@en ;
              rdfs:comment "Grasping weeds and vines sprout from the ground in a 20-foot square starting form a point within range. For the duration, these plants turn the ground in the area into difficult terrain."@en .

DnD5eCharacter:Enthrall 	a rdfs:Class ;
              rdfs:subClassOf TTRpg:Spell ;
              DnD5eCharacter:inMagicSchool DnD5eCharacter:Enchantment ;
              rdfs:label "Enthrall"@en ;
              rdfs:comment "You weave a distracting string of words, causing creatures of your choice that you can see within range and that can hear you to make a wisdom saving throw. Any creature that can't be charmed succeeds on this saving throw automatically, and if you or your companions are fighting a creature, it has advantage on the save. On a failed save, the target has disadvantage on Wisdom (Perception) checks made to perceive any creature other than you until the spell ends or until the target can no longer hear you. The spell ends if you are incapacitated or can no longer speak."@en .

DnD5eCharacter:Etherealness 	a rdfs:Class ;
              rdfs:subClassOf TTRpg:Spell ;
              DnD5eCharacter:inMagicSchool DnD5eCharacter:Transmutation ;
              rdfs:label "Etherealness"@en ;
              rdfs:comment "You step into the border regions of the Ethereal Plane, in the area where it overlaps with your current plane. You remain in the Border Ethereal for the duration or until you use your action to dismiss the spell. During this time, you can move in any direction. If you move up or down, every foot of movement costs an extra foot. You can see and hear the plane you originated from, but everything there looks gray, and you can't see anything more than 60 feet away."@en .

DnD5eCharacter:ExpeditiousRetreat 	a rdfs:Class ;
              rdfs:subClassOf TTRpg:Spell ;
              DnD5eCharacter:inMagicSchool DnD5eCharacter:Transmutation ;
              rdfs:label "Expeditious Retreat"@en ;
              rdfs:comment "This spell allows you to move at an incredible pace. When you cast this spell, and then as a bonus action on each of your turns until the spell ends, you can take the Dash action."@en .

DnD5eCharacter:Eyebite 	a rdfs:Class ;
              rdfs:subClassOf TTRpg:Spell ;
              DnD5eCharacter:inMagicSchool DnD5eCharacter:Necromancy ;
              rdfs:label "Eyebite"@en ;
              rdfs:comment "For the spell's duration, your eyes become an inky void imbued with dread power. One creature of your choice within 60 feet of you that you can see must succeed on a wisdom saving throw or be affected by one of the following effects of your choice for the duration. On each of your turns until the spell ends, you can use your action to target another creature but can't target a creature again if it has succeeded on a saving throw against this casting of eyebite."@en .

DnD5eCharacter:Fabricate 	a rdfs:Class ;
              rdfs:subClassOf TTRpg:Spell ;
              DnD5eCharacter:inMagicSchool DnD5eCharacter:Transmutation ;
              rdfs:label "Fabricate"@en ;
              rdfs:comment "You convert raw materials into products of the same material. For example, you can fabricate a wooden bridge from a clump of trees, a rope from a patch of hemp, and clothes from flax or wool."@en .

DnD5eCharacter:FaerieFire 	a rdfs:Class ;
              rdfs:subClassOf TTRpg:Spell ;
              DnD5eCharacter:inMagicSchool DnD5eCharacter:Evocation ;
              rdfs:label "Faerie Fire"@en ;
              rdfs:comment "Each object in a 20-foot cube within range is outlined in blue, green, or violet light (your choice). Any creature in the area when the spell is cast is also outlined in light if it fails a dexterity saving throw. For the duration, objects and affected creatures shed dim light in a 10-foot radius."@en .

DnD5eCharacter:FaithfulHound 	a rdfs:Class ;
              rdfs:subClassOf TTRpg:Spell ;
              DnD5eCharacter:inMagicSchool DnD5eCharacter:Conjuration ;
              rdfs:label "Faithful Hound"@en ;
              rdfs:comment "You conjure a phantom watchdog in an unoccupied space that you can see within range, where it remains for the duration, until you dismiss it as an action, or until you move more than 100 feet away from it."@en .

DnD5eCharacter:FalseLife 	a rdfs:Class ;
              rdfs:subClassOf TTRpg:Spell ;
              DnD5eCharacter:inMagicSchool DnD5eCharacter:Necromancy ;
              rdfs:label "False Life"@en ;
              rdfs:comment "Bolstering yourself with a necromantic facsimile of life, you gain 1d4 + 4 temporary hit points for the duration."@en .

DnD5eCharacter:Fear 	a rdfs:Class ;
              rdfs:subClassOf TTRpg:Spell ;
              DnD5eCharacter:inMagicSchool DnD5eCharacter:Illusion ;
              rdfs:label "Fear"@en ;
              rdfs:comment "You project a phantasmal image of a creature's worst fears. Each creature in a 30-foot cone must succeed on a wisdom saving throw or drop whatever it is holding and become frightened for the duration."@en .

DnD5eCharacter:FeatherFall 	a rdfs:Class ;
              rdfs:subClassOf TTRpg:Spell ;
              DnD5eCharacter:inMagicSchool DnD5eCharacter:Transmutation ;
              rdfs:label "Feather Fall"@en ;
              rdfs:comment "Choose up to five falling creatures within range. A falling creature's rate of descent slows to 60 feet per round until the spell ends. If the creature lands before the spell ends, it takes no falling damage and can land on its feet, and the spell ends for that creature."@en .

DnD5eCharacter:Feeblemind 	a rdfs:Class ;
              rdfs:subClassOf TTRpg:Spell ;
              DnD5eCharacter:inMagicSchool DnD5eCharacter:Enchantment ;
              rdfs:label "Feeblemind"@en ;
              rdfs:comment "You blast the mind of a creature that you can see within range, attempting to shatter its intellect and personality. The target takes 4d6 psychic damage and must make an intelligence saving throw."@en .

DnD5eCharacter:FindFamiliar 	a rdfs:Class ;
              rdfs:subClassOf TTRpg:Spell ;
              DnD5eCharacter:inMagicSchool DnD5eCharacter:Conjuration ;
              rdfs:label "Find Familiar"@en ;
              rdfs:comment "You gain the service of a familiar, a spirit that takes an animal form you choose: bat, cat, crab, frog (toad), hawk, lizard, octopus, owl, poisonous snake, fish (quipper), rat, raven, sea horse, spider, or weasel. Appearing in an unoccupied space within range, the familiar has the statistics of the chosen form, though it is a celestial, fey, or fiend (your choice) instead of a beast."@en .

DnD5eCharacter:FindSteed 	a rdfs:Class ;
              rdfs:subClassOf TTRpg:Spell ;
              DnD5eCharacter:inMagicSchool DnD5eCharacter:Conjuration ;
              rdfs:label "Find Steed"@en ;
              rdfs:comment "You summon a spirit that assumes the form of an unusually intelligent, strong, and loyal steed, creating a long-lasting bond with it. Appearing in an unoccupied space within range, the steed takes on a form that you choose, such as a warhorse, a pony, a camel, an elk, or a mastiff. (Your DM might allow other animals to be summoned as steeds.) The steed has the statistics of the chosen form, though it is a celestial, fey, or fiend (your choice) instead of its normal type. Additionally, if your steed has an Intelligence of 5 or less, its Intelligence becomes 6, and it gains the ability to understand one language of your choice that you speak."@en .

DnD5eCharacter:FindThePath 	a rdfs:Class ;
              rdfs:subClassOf TTRpg:Spell ;
              DnD5eCharacter:inMagicSchool DnD5eCharacter:Divination ;
              rdfs:label "Find The Path"@en ;
              rdfs:comment "This spell allows you to find the shortest, most direct physical route to a specific fixed location that you are familiar with on the same plane of existence. If you name a destination on another plane of existence, a destination that moves (such as a mobile fortress), or a destination that isn't specific (such as a green dragon's lair), the spell fails."@en .

DnD5eCharacter:FindTraps 	a rdfs:Class ;
              rdfs:subClassOf TTRpg:Spell ;
              DnD5eCharacter:inMagicSchool DnD5eCharacter:Divination ;
              rdfs:label "Find Traps"@en ;
              rdfs:comment "You sense the presence of any trap within range that is within line of sight. A trap, for the purpose of this spell, includes anything that would inflict a sudden or unexpected effect you consider harmful or undesirable, which was specifically intended as such by its creator. Thus, the spell would sense an area affected by the alarm spell, a glyph of warding, or a mechanical pit trap, but it would not reveal a natural weakness in the floor, an unstable ceiling, or a hidden sinkhole."@en .

DnD5eCharacter:FingerOfDeath 	a rdfs:Class ;
              rdfs:subClassOf TTRpg:Spell ;
              DnD5eCharacter:inMagicSchool DnD5eCharacter:Necromancy ;
              rdfs:label "Finger Of Death"@en ;
              rdfs:comment "You send negative energy coursing through a creature that you can see within range, causing it searing pain. The target must make a constitution saving throw. It takes 7d8 + 30 necrotic damage on a failed save, or half as much damage on a successful one."@en .

DnD5eCharacter:FireBolt 	a rdfs:Class ;
              rdfs:subClassOf TTRpg:Spell ;
              DnD5eCharacter:inMagicSchool DnD5eCharacter:Evocation ;
              rdfs:label "Fire Bolt"@en ;
              rdfs:comment "You hurl a mote of fire at a creature or object within range. Make a ranged spell attack against the target. On a hit, the target takes 1d10 fire damage. A flammable object hit by this spell ignites if it isn't being worn or carried."@en .

DnD5eCharacter:FireShield 	a rdfs:Class ;
              rdfs:subClassOf TTRpg:Spell ;
              DnD5eCharacter:inMagicSchool DnD5eCharacter:Evocation ;
              rdfs:label "Fire Shield"@en ;
              rdfs:comment "Thin and vaporous flame surround your body for the duration of the spell, radiating a bright light bright light in a 10-foot radius and dim light for an additional 10 feet. You can end the spell using an action to make it disappear."@en .

DnD5eCharacter:FireStorm 	a rdfs:Class ;
              rdfs:subClassOf TTRpg:Spell ;
              DnD5eCharacter:inMagicSchool DnD5eCharacter:Evocation ;
              rdfs:label "Fire Storm"@en ;
              rdfs:comment "A storm made up of sheets of roaring flame appears in a location you choose within range. The area of the storm consists of up to ten 10-foot cubes, which you can arrange as you wish. Each cube must have at least one face adjacent to the face of another cube. Each creature in the area must make a dexterity saving throw. It takes 7d10 fire damage on a failed save, or half as much damage on a successful one."@en .

DnD5eCharacter:Fireball 	a rdfs:Class ;
              rdfs:subClassOf TTRpg:Spell ;
              DnD5eCharacter:inMagicSchool DnD5eCharacter:Evocation ;
              rdfs:label "Fireball"@en ;
              rdfs:comment "A bright streak flashes from your pointing finger to a point you choose within range and then blossoms with a low roar into an explosion of flame. Each creature in a 20-foot-radius sphere centered on that point must make a dexterity saving throw. A target takes 8d6 fire damage on a failed save, or half as much damage on a successful one."@en .

DnD5eCharacter:FlameBlade 	a rdfs:Class ;
              rdfs:subClassOf TTRpg:Spell ;
              DnD5eCharacter:inMagicSchool DnD5eCharacter:Evocation ;
              rdfs:label "Flame Blade"@en ;
              rdfs:comment "You evoke a fiery blade in your free hand. The blade is similar in size and shape to a scimitar, and it lasts for the duration. If you let go of the blade, it disappears, but you can evoke the blade again as a bonus action."@en .

DnD5eCharacter:FlameStrike 	a rdfs:Class ;
              rdfs:subClassOf TTRpg:Spell ;
              DnD5eCharacter:inMagicSchool DnD5eCharacter:Evocation ;
              rdfs:label "Flame Strike"@en ;
              rdfs:comment "A vertical column of divine fire roars down from the heavens in a location you specify. Each creature in a 10-foot-radius, 40-foot-high cylinder centered on a point within range must make a dexterity saving throw. A creature takes 4d6 fire damage and 4d6 radiant damage on a failed save, or half as much damage on a successful one."@en .

DnD5eCharacter:FlamingSphere 	a rdfs:Class ;
              rdfs:subClassOf TTRpg:Spell ;
              DnD5eCharacter:inMagicSchool DnD5eCharacter:Conjuration ;
              rdfs:label "Flaming Sphere"@en ;
              rdfs:comment "A 5-foot-diameter sphere of fire appears in an unoccupied space of your choice within range and lasts for the duration. Any creature that ends its turn within 5 feet of the sphere must make a dexterity saving throw. The creature takes 2d6 fire damage on a failed save, or half as much damage on a successful one."@en .

DnD5eCharacter:FleshToStone 	a rdfs:Class ;
              rdfs:subClassOf TTRpg:Spell ;
              DnD5eCharacter:inMagicSchool DnD5eCharacter:Transmutation ;
              rdfs:label "Flesh To Stone"@en ;
              rdfs:comment "You attempt to turn one creature that you can see within range into stone. If the target's body is made of flesh, the creature must make a constitution saving throw. On a failed save, it is restrained as its flesh begins to harden. On a successful save, the creature isn't affected."@en .

DnD5eCharacter:FloatingDisk 	a rdfs:Class ;
              rdfs:subClassOf TTRpg:Spell ;
              DnD5eCharacter:inMagicSchool DnD5eCharacter:Conjuration ;
              rdfs:label "Floating Disk"@en ;
              rdfs:comment "This spell creates a circular, horizontal plane of force, 3 feet in diameter and 1 inch thick, that floats 3 feet above the ground in an unoccupied space of your choice that you can see within range. The disk remains for the duration, and can hold up to 500 pounds. If more weight is placed on it, the spell ends, and everything on the disk falls to the ground."@en .

DnD5eCharacter:Fly 	a rdfs:Class ;
              rdfs:subClassOf TTRpg:Spell ;
              DnD5eCharacter:inMagicSchool DnD5eCharacter:Transmutation ;
              rdfs:label "Fly"@en ;
              rdfs:comment "You touch a willing creature. The target gains a flying speed of 60 feet for the duration. When the spell ends, the target falls if it is still aloft, unless it can stop the fall."@en .

DnD5eCharacter:FogCloud 	a rdfs:Class ;
              rdfs:subClassOf TTRpg:Spell ;
              DnD5eCharacter:inMagicSchool DnD5eCharacter:Conjuration ;
              rdfs:label "Fog Cloud"@en ;
              rdfs:comment "You create a 20-foot-radius sphere of fog centered on a point within range. The sphere spreads around corners, and its area is heavily obscured. It lasts for the duration or until a wind of moderate or greater speed (at least 10 miles per hour) disperses it."@en .

DnD5eCharacter:Forbiddance 	a rdfs:Class ;
              rdfs:subClassOf TTRpg:Spell ;
              DnD5eCharacter:inMagicSchool DnD5eCharacter:Abjuration ;
              rdfs:label "Forbiddance"@en ;
              rdfs:comment "You create a ward against magical travel that protects up to 40,000 square feet of floor space to a height of 30 feet above the floor. For the duration, creatures can't teleport into the area or use portals, such as those created by the gate spell, to enter the area. The spell proofs the area against planar travel, and therefore prevents creatures from accessing the area by way of the Astral Plane, Ethereal Plane, Feywild, Shadowfell, or the plane shift spell."@en .

DnD5eCharacter:Forcecage 	a rdfs:Class ;
              rdfs:subClassOf TTRpg:Spell ;
              DnD5eCharacter:inMagicSchool DnD5eCharacter:Evocation ;
              rdfs:label "Forcecage"@en ;
              rdfs:comment "An immobile, invisible, cube-shaped prison composed of magical force springs into existence around an area you choose within range. The prison can be a cage or a solid box, as you choose."@en .

DnD5eCharacter:Foresight 	a rdfs:Class ;
              rdfs:subClassOf TTRpg:Spell ;
              DnD5eCharacter:inMagicSchool DnD5eCharacter:Divination ;
              rdfs:label "Foresight"@en ;
              rdfs:comment "You touch a willing creature and bestow a limited ability to see into the immediate future. For the duration, the target can't be surprised and has advantage on attack rolls, ability checks, and saving throws. Additionally, other creatures have disadvantage on attack rolls against the target for the duration."@en .

DnD5eCharacter:FreedomOfMovement 	a rdfs:Class ;
              rdfs:subClassOf TTRpg:Spell ;
              DnD5eCharacter:inMagicSchool DnD5eCharacter:Abjuration ;
              rdfs:label "Freedom Of Movement"@en ;
              rdfs:comment "You touch a willing creature. For the duration, the target's movement is unaffected by difficult terrain, and spells and other magical effects can neither reduce the target's speed nor cause the target to be paralyzed or restrained."@en .

DnD5eCharacter:FreezingSphere 	a rdfs:Class ;
              rdfs:subClassOf TTRpg:Spell ;
              DnD5eCharacter:inMagicSchool DnD5eCharacter:Evocation ;
              rdfs:label "Freezing Sphere"@en ;
              rdfs:comment "A frigid globe of cold energy streaks from your fingertips to a point of your choice within range, where it explodes in a 60-foot-radius sphere. Each creature within the area must make a constitution saving throw. On a failed save, a creature takes 10d6 cold damage. On a successful save, it takes half as much damage."@en .

DnD5eCharacter:GaseousForm 	a rdfs:Class ;
              rdfs:subClassOf TTRpg:Spell ;
              DnD5eCharacter:inMagicSchool DnD5eCharacter:Transmutation ;
              rdfs:label "Gaseous Form"@en ;
              rdfs:comment "You transform a willing creature you touch, along with everything it's wearing and carrying, into a misty cloud for the duration. The spell ends if the creature drops to 0 hit points. An incorporeal creature isn't affected."@en .

DnD5eCharacter:Gate 	a rdfs:Class ;
              rdfs:subClassOf TTRpg:Spell ;
              DnD5eCharacter:inMagicSchool DnD5eCharacter:Conjuration ;
              rdfs:label "Gate"@en ;
              rdfs:comment "You conjure a portal linking an unoccupied space you can see within range to a precise location on a different plane of existence. The portal is a circular opening, which you can make 5 to 20 feet in diameter. You can orient the portal in any direction you choose. The portal lasts for the duration."@en .

DnD5eCharacter:Geas 	a rdfs:Class ;
              rdfs:subClassOf TTRpg:Spell ;
              DnD5eCharacter:inMagicSchool DnD5eCharacter:Enchantment ;
              rdfs:label "Geas"@en ;
              rdfs:comment "You place a magical command on a creature that you can see within range, forcing it to carry out some service or refrain from some action or course of activity as you decide. If the creature can understand you, it must succeed on a wisdom saving throw or become charmed by you for the duration. While the creature is charmed by you, it takes 5d10 psychic damage each time it acts in a manner directly counter to your instructions, but no more than once each day. A creature that can't understand you is unaffected by the spell."@en .

DnD5eCharacter:GentleRepose 	a rdfs:Class ;
              rdfs:subClassOf TTRpg:Spell ;
              DnD5eCharacter:inMagicSchool DnD5eCharacter:Necromancy ;
              rdfs:label "Gentle Repose"@en ;
              rdfs:comment "You touch a corpse or other remains. For the duration, the target is protected from decay and can't become undead."@en .

DnD5eCharacter:GiantInsect 	a rdfs:Class ;
              rdfs:subClassOf TTRpg:Spell ;
              DnD5eCharacter:inMagicSchool DnD5eCharacter:Transmutation ;
              rdfs:label "Giant Insect"@en ;
              rdfs:comment "You transform up to ten centipedes, three spiders, five wasps, or one scorpion within range into giant versions of their natural forms for the duration. A centipede becomes a giant centipede, a spider becomes a giant spider, a wasp becomes a giant wasp, and a scorpion becomes a giant scorpion."@en .

DnD5eCharacter:Glibness 	a rdfs:Class ;
              rdfs:subClassOf TTRpg:Spell ;
              DnD5eCharacter:inMagicSchool DnD5eCharacter:Transmutation ;
              rdfs:label "Glibness"@en ;
              rdfs:comment "Until the spell ends, when you make a Charisma check, you can replace the number you roll with a 15. Additionally, no matter what you say, magic that would determine if you are telling the truth indicates that you are being truthful."@en .

DnD5eCharacter:GlobeOfInvulnerability 	a rdfs:Class ;
              rdfs:subClassOf TTRpg:Spell ;
              DnD5eCharacter:inMagicSchool DnD5eCharacter:Abjuration ;
              rdfs:label "Globe Of Invulnerability"@en ;
              rdfs:comment "An immobile, faintly shimmering barrier springs into existence in a 10-foot radius around you and remains for the duration."@en .

DnD5eCharacter:GlyphOfWarding 	a rdfs:Class ;
              rdfs:subClassOf TTRpg:Spell ;
              DnD5eCharacter:inMagicSchool DnD5eCharacter:Abjuration ;
              rdfs:label "Glyph Of Warding"@en ;
              rdfs:comment "When you cast this spell, you inscribe a glyph that harms other creatures, either upon a surface (such as a table or a section of floor or wall) or within an object that can be closed (such as a book, a scroll, or a treasure chest) to conceal the glyph. If you choose a surface, the glyph can cover an area of the surface no larger than 10 feet in diameter. If you choose an object, that object must remain in its place; if the object is moved more than 10 feet from where you cast this spell, the glyph is broken, and the spell ends without being triggered."@en .

DnD5eCharacter:Goodberry 	a rdfs:Class ;
              rdfs:subClassOf TTRpg:Spell ;
              DnD5eCharacter:inMagicSchool DnD5eCharacter:Transmutation ;
              rdfs:label "Goodberry"@en ;
              rdfs:comment "Up to ten berries appear in your hand and are infused with magic for the duration. A creature can use its action to eat one berry. Eating a berry restores 1 hit point, and the berry provides enough nourishment to sustain a creature for a day."@en .

DnD5eCharacter:Grease 	a rdfs:Class ;
              rdfs:subClassOf TTRpg:Spell ;
              DnD5eCharacter:inMagicSchool DnD5eCharacter:Conjuration ;
              rdfs:label "Grease"@en ;
              rdfs:comment "Slick grease covers the ground in a 10-foot square centered on a point within range and turns it into difficult terrain for the duration."@en .

DnD5eCharacter:GreaterInvisibility 	a rdfs:Class ;
              rdfs:subClassOf TTRpg:Spell ;
              DnD5eCharacter:inMagicSchool DnD5eCharacter:Illusion ;
              rdfs:label "Greater Invisibility"@en ;
              rdfs:comment "You or a creature you touch becomes invisible until the spell ends. Anything the target is wearing or carrying is invisible as long as it is on the target's person."@en .

DnD5eCharacter:GreaterRestoration 	a rdfs:Class ;
              rdfs:subClassOf TTRpg:Spell ;
              DnD5eCharacter:inMagicSchool DnD5eCharacter:Abjuration ;
              rdfs:label "Greater Restoration"@en ;
              rdfs:comment "You imbue a creature you touch with positive energy to undo a debilitating effect. You can reduce the target's exhaustion level by one, or end one of the following effects on the target:"@en .

DnD5eCharacter:GuardianOfFaith 	a rdfs:Class ;
              rdfs:subClassOf TTRpg:Spell ;
              DnD5eCharacter:inMagicSchool DnD5eCharacter:Conjuration ;
              rdfs:label "Guardian Of Faith"@en ;
              rdfs:comment "A Large spectral guardian appears and hovers for the duration in an unoccupied space of your choice that you can see within range. The guardian occupies that space and is indistinct except for a gleaming sword and shield emblazoned with the symbol of your deity."@en .

DnD5eCharacter:GuardsAndWards 	a rdfs:Class ;
              rdfs:subClassOf TTRpg:Spell ;
              DnD5eCharacter:inMagicSchool DnD5eCharacter:Abjuration ;
              rdfs:label "Guards And Wards"@en ;
              rdfs:comment "You create a ward that protects up to 2,500 square feet of floor space (an area 50 feet square, or one hundred 5-foot squares or twenty-five 10-foot squares). The warded area can be up to 20 feet tall, and shaped as you desire. You can ward several stories of a stronghold by dividing the area among them, as long as you can walk into each contiguous area while you are casting the spell."@en .

DnD5eCharacter:Guidance 	a rdfs:Class ;
              rdfs:subClassOf TTRpg:Spell ;
              DnD5eCharacter:inMagicSchool DnD5eCharacter:Divination ;
              rdfs:label "Guidance"@en ;
              rdfs:comment "You touch one willing creature. Once before the spell ends, the target can roll a d4 and add the number rolled to one ability check of its choice. It can roll the die before or after making the ability check. The spell then ends."@en .

DnD5eCharacter:GuidingBolt 	a rdfs:Class ;
              rdfs:subClassOf TTRpg:Spell ;
              DnD5eCharacter:inMagicSchool DnD5eCharacter:Evocation ;
              rdfs:label "Guiding Bolt"@en ;
              rdfs:comment "A flash of light streaks toward a creature of your choice within range. Make a ranged spell attack against the target. On a hit, the target takes 4d6 radiant damage, and the next attack roll made against this target before the end of your next turn has advantage, thanks to the mystical dim light glittering on the target until then."@en .

DnD5eCharacter:GustOfWind 	a rdfs:Class ;
              rdfs:subClassOf TTRpg:Spell ;
              DnD5eCharacter:inMagicSchool DnD5eCharacter:Evocation ;
              rdfs:label "Gust Of Wind"@en ;
              rdfs:comment "A line of strong wind 60 feet long and 10 feet wide blasts from you in a direction you choose for the spell's duration. Each creature that starts its turn in the line must succeed on a strength saving throw or be pushed 15 feet away from you in a direction following the line."@en .

DnD5eCharacter:Hallow 	a rdfs:Class ;
              rdfs:subClassOf TTRpg:Spell ;
              DnD5eCharacter:inMagicSchool DnD5eCharacter:Evocation ;
              rdfs:label "Hallow"@en ;
              rdfs:comment "You touch a point and infuse an area around it with holy (or unholy) power. The area can have a radius up to 60 feet, and the spell fails if the radius includes an area already under the effect a hallow spell. The affected area is subject to the following effects."@en .

DnD5eCharacter:HallucinatoryTerrain 	a rdfs:Class ;
              rdfs:subClassOf TTRpg:Spell ;
              DnD5eCharacter:inMagicSchool DnD5eCharacter:Illusion ;
              rdfs:label "Hallucinatory Terrain"@en ;
              rdfs:comment "You make natural terrain in a 150-foot cube in range look, sound, and smell like some other sort of natural terrain. Thus, open fields or a road can be made to resemble a swamp, hill, crevasse, or some other difficult or impassable terrain. A pond can be made to seem like a grassy meadow, a precipice like a gentle slope, or a rock-strewn gully like a wide and smooth road. Manufactured structures, equipment, and creatures within the area aren't changed in appearance."@en .

DnD5eCharacter:Harm 	a rdfs:Class ;
              rdfs:subClassOf TTRpg:Spell ;
              DnD5eCharacter:inMagicSchool DnD5eCharacter:Necromancy ;
              rdfs:label "Harm"@en ;
              rdfs:comment "You unleash a virulent disease on a creature that you can see within range. The target must make a constitution saving throw. On a failed save, it takes 14d6 necrotic damage, or half as much damage on a successful save. The damage can't reduce the target's hit points below 1. If the target fails the saving throw, its hit point maximum is reduced for 1 hour by an amount equal to the necrotic damage it took. Any effect that removes a disease allows a creature's hit point maximum to return to normal before that time passes."@en .

DnD5eCharacter:Haste 	a rdfs:Class ;
              rdfs:subClassOf TTRpg:Spell ;
              DnD5eCharacter:inMagicSchool DnD5eCharacter:Transmutation ;
              rdfs:label "Haste"@en ;
              rdfs:comment "Choose a willing creature that you can see within range. Until the spell ends, the target's speed is doubled, it gains a +2 bonus to AC, it has advantage on dexterity saving throws, and it gains an additional action on each of its turns. That action can be used only to take the Attack (one weapon attack only), Dash, Disengage, Hide, or Use an Object action."@en .

DnD5eCharacter:Heal 	a rdfs:Class ;
              rdfs:subClassOf TTRpg:Spell ;
              DnD5eCharacter:inMagicSchool DnD5eCharacter:Evocation ;
              rdfs:label "Heal"@en ;
              rdfs:comment "Choose a creature that you can see within range. A surge of positive energy washes through the creature, causing it to regain 70 hit points. This spell also ends blindness, deafness, and any diseases affecting the target. This spell has no effect on constructs or undead."@en .

DnD5eCharacter:HealingWord 	a rdfs:Class ;
              rdfs:subClassOf TTRpg:Spell ;
              DnD5eCharacter:inMagicSchool DnD5eCharacter:Evocation ;
              rdfs:label "Healing Word"@en ;
              rdfs:comment "A creature of your choice that you can see within range regains hit points equal to 1d4 + your spellcasting ability modifier. This spell has no effect on undead or constructs."@en .

DnD5eCharacter:HeatMetal 	a rdfs:Class ;
              rdfs:subClassOf TTRpg:Spell ;
              DnD5eCharacter:inMagicSchool DnD5eCharacter:Transmutation ;
              rdfs:label "Heat Metal"@en ;
              rdfs:comment "Choose a manufactured metal object, such as a metal weapon or a suit of heavy or medium metal armor, that you can see within range. You cause the object to glow red-hot. Any creature in physical contact with the object takes 2d8 fire damage when you cast the spell. Until the spell ends, you can use a bonus action on each of your subsequent turns to cause this damage again."@en .

DnD5eCharacter:HellishRebuke 	a rdfs:Class ;
              rdfs:subClassOf TTRpg:Spell ;
              DnD5eCharacter:inMagicSchool DnD5eCharacter:Evocation ;
              rdfs:label "Hellish Rebuke"@en ;
              rdfs:comment "You point your finger, and the creature that damaged you is momentarily surrounded by hellish flames. The creature must make a dexterity saving throw. It takes 2d10 fire damage on a failed save, or half as much damage on a successful one."@en .

DnD5eCharacter:HeroesFeast 	a rdfs:Class ;
              rdfs:subClassOf TTRpg:Spell ;
              DnD5eCharacter:inMagicSchool DnD5eCharacter:Conjuration ;
              rdfs:label "Heroes Feast"@en ;
              rdfs:comment "You bring forth a great feast, including magnificent food and drink. The feast takes 1 hour to consume and disappears at the end of that time, and the beneficial effects don't set in until this hour is over. Up to twelve other creatures can partake of the feast."@en .

DnD5eCharacter:Heroism 	a rdfs:Class ;
              rdfs:subClassOf TTRpg:Spell ;
              DnD5eCharacter:inMagicSchool DnD5eCharacter:Enchantment ;
              rdfs:label "Heroism"@en ;
              rdfs:comment "A willing creature you touch is imbued with bravery. Until the spell ends, the creature is immune to being frightened and gains temporary hit points equal to your spellcasting ability modifier at the start of each of its turns. When the spell ends, the target loses any remaining temporary hit points from this spell."@en .

DnD5eCharacter:HideousLaughter 	a rdfs:Class ;
              rdfs:subClassOf TTRpg:Spell ;
              DnD5eCharacter:inMagicSchool DnD5eCharacter:Enchantment ;
              rdfs:label "Hideous Laughter"@en ;
              rdfs:comment "A creature of your choice that you can see within range perceives everything as hilariously funny and falls into fits of laughter if this spell affects it. The target must succeed on a wisdom saving throw or fall prone, becoming incapacitated and unable to stand up for the duration. A creature with an Intelligence score of 4 or less isn't affected."@en .

DnD5eCharacter:HoldMonster 	a rdfs:Class ;
              rdfs:subClassOf TTRpg:Spell ;
              DnD5eCharacter:inMagicSchool DnD5eCharacter:Enchantment ;
              rdfs:label "Hold Monster"@en ;
              rdfs:comment "Choose a creature you can see and reach. The target must make a saving throw of Wisdom or be paralyzed for the duration of the spell. This spell has no effect against the undead. At the end of each round, the target can make a new saving throw of Wisdom. If successful, the spell ends for the creature."@en .

DnD5eCharacter:HoldPerson 	a rdfs:Class ;
              rdfs:subClassOf TTRpg:Spell ;
              DnD5eCharacter:inMagicSchool DnD5eCharacter:Enchantment ;
              rdfs:label "Hold Person"@en ;
              rdfs:comment "Choose a humanoid that you can see within range. The target must succeed on a wisdom saving throw or be paralyzed for the duration. At the end of each of its turns, the target can make another wisdom saving throw. On a success, the spell ends on the target."@en .

DnD5eCharacter:HolyAura 	a rdfs:Class ;
              rdfs:subClassOf TTRpg:Spell ;
              DnD5eCharacter:inMagicSchool DnD5eCharacter:Abjuration ;
              rdfs:label "Holy Aura"@en ;
              rdfs:comment "Divine light washes out from you and coalesces in a soft radiance in a 30-foot radius around you. Creatures of your choice in that radius when you cast this spell shed dim light in a 5-foot radius and have advantage on all saving throws, and other creatures have disadvantage on attack rolls against them until the spell ends. In addition, when a fiend or an undead hits an affected creature with a melee attack, the aura flashes with brilliant light. The attacker must succeed on a constitution saving throw or be blinded until the spell ends."@en .

DnD5eCharacter:HuntersMark 	a rdfs:Class ;
              rdfs:subClassOf TTRpg:Spell ;
              DnD5eCharacter:inMagicSchool DnD5eCharacter:Divination ;
              rdfs:label "Hunters Mark"@en ;
              rdfs:comment "You choose a creature you can see within range and mystically mark it as your quarry. Until the spell ends, you deal an extra 1d6 damage to the target whenever you hit it with a weapon attack, and you have advantage on any Wisdom (Perception) or Wisdom (Survival) check you make to find it. If the target drops to 0 hit points before this spell ends, you can use a bonus action on a subsequent turn of yours to mark a new creature."@en .

DnD5eCharacter:HypnoticPattern 	a rdfs:Class ;
              rdfs:subClassOf TTRpg:Spell ;
              DnD5eCharacter:inMagicSchool DnD5eCharacter:Illusion ;
              rdfs:label "Hypnotic Pattern"@en ;
              rdfs:comment "You create a twisting pattern of colors that weaves through the air inside a 30-foot cube within range. The pattern appears for a moment and vanishes. Each creature in the area who sees the pattern must make a wisdom saving throw. On a failed save, the creature becomes charmed for the duration. While charmed by this spell, the creature is incapacitated and has a speed of 0."@en .

DnD5eCharacter:IceStorm 	a rdfs:Class ;
              rdfs:subClassOf TTRpg:Spell ;
              DnD5eCharacter:inMagicSchool DnD5eCharacter:Evocation ;
              rdfs:label "Ice Storm"@en ;
              rdfs:comment "A hail of rock-hard ice pounds to the ground in a 20-foot-radius, 40-foot-high cylinder centered on a point within range. Each creature in the cylinder must make a dexterity saving throw. A creature takes 2d8 bludgeoning damage and 4d6 cold damage on a failed save, or half as much damage on a successful one."@en .

DnD5eCharacter:Identify 	a rdfs:Class ;
              rdfs:subClassOf TTRpg:Spell ;
              DnD5eCharacter:inMagicSchool DnD5eCharacter:Divination ;
              rdfs:label "Identify"@en ;
              rdfs:comment "You choose one object that you must touch throughout the casting of the spell. If it is a magic item or some other magic-imbued object, you learn its properties and how to use them, whether it requires attunement to use, and how many charges it has, if any. You learn whether any spells are affecting the item and what they are. If the item was created by a spell, you learn which spell created it."@en .

DnD5eCharacter:IllusoryScript 	a rdfs:Class ;
              rdfs:subClassOf TTRpg:Spell ;
              DnD5eCharacter:inMagicSchool DnD5eCharacter:Illusion ;
              rdfs:label "Illusory Script"@en ;
              rdfs:comment "You write on parchment, paper, or some other suitable writing material and imbue it with a potent illusion that lasts for the duration."@en .

DnD5eCharacter:Imprisonment 	a rdfs:Class ;
              rdfs:subClassOf TTRpg:Spell ;
              DnD5eCharacter:inMagicSchool DnD5eCharacter:Abjuration ;
              rdfs:label "Imprisonment"@en ;
              rdfs:comment "You create a magical restraint to hold a creature that you can see within range. The target must succeed on a wisdom saving throw or be bound by the spell; if it succeeds, it is immune to this spell if you cast it again. While affected by this spell, the creature doesn't need to breathe, eat, or drink, and it doesn't age. Divination spells can't locate or perceive the target."@en .

DnD5eCharacter:IncendiaryCloud 	a rdfs:Class ;
              rdfs:subClassOf TTRpg:Spell ;
              DnD5eCharacter:inMagicSchool DnD5eCharacter:Conjuration ;
              rdfs:label "Incendiary Cloud"@en ;
              rdfs:comment "A swirling cloud of smoke shot through with white-hot embers appears in a 20-foot-radius sphere centered on a point within range. The cloud spreads around corners and is heavily obscured. It lasts for the duration or until a wind of moderate or greater speed (at least 10 miles per hour) disperses it."@en .

DnD5eCharacter:InflictWounds 	a rdfs:Class ;
              rdfs:subClassOf TTRpg:Spell ;
              DnD5eCharacter:inMagicSchool DnD5eCharacter:Necromancy ;
              rdfs:label "Inflict Wounds"@en ;
              rdfs:comment "Make a melee spell attack against a creature you can reach. On a hit, the target takes 3d10 necrotic damage."@en .

DnD5eCharacter:InsectPlague 	a rdfs:Class ;
              rdfs:subClassOf TTRpg:Spell ;
              DnD5eCharacter:inMagicSchool DnD5eCharacter:Conjuration ;
              rdfs:label "Insect Plague"@en ;
              rdfs:comment "Swarming, biting locusts fill a 20-foot-radius sphere centered on a point you choose within range. The sphere spreads around corners. The sphere remains for the duration, and its area is lightly obscured. The sphere's area is difficult terrain."@en .

DnD5eCharacter:InstantSummons 	a rdfs:Class ;
              rdfs:subClassOf TTRpg:Spell ;
              DnD5eCharacter:inMagicSchool DnD5eCharacter:Conjuration ;
              rdfs:label "Instant Summons"@en ;
              rdfs:comment "You touch an object weighing 10 pounds or less whose longest dimension is 6 feet or less. The spell leaves an invisible mark on its surface and invisibly inscribes the name of the item on the sapphire you use as the material component. Each time you cast this spell, you must use a different sapphire."@en .

DnD5eCharacter:Invisibility 	a rdfs:Class ;
              rdfs:subClassOf TTRpg:Spell ;
              DnD5eCharacter:inMagicSchool DnD5eCharacter:Illusion ;
              rdfs:label "Invisibility"@en ;
              rdfs:comment "A creature you touch becomes invisible until the spell ends. Anything the target is wearing or carrying is invisible as long as it is on the target's person. The spell ends for a target that attacks or casts a spell."@en .

DnD5eCharacter:IrresistibleDance 	a rdfs:Class ;
              rdfs:subClassOf TTRpg:Spell ;
              DnD5eCharacter:inMagicSchool DnD5eCharacter:Enchantment ;
              rdfs:label "Irresistible Dance"@en ;
              rdfs:comment "Choose one creature that you can see within range. The target begins a comic dance in place: shuffling, tapping its feet, and capering for the duration. Creatures that can't be charmed are immune to this spell."@en .

DnD5eCharacter:Jump 	a rdfs:Class ;
              rdfs:subClassOf TTRpg:Spell ;
              DnD5eCharacter:inMagicSchool DnD5eCharacter:Transmutation ;
              rdfs:label "Jump"@en ;
              rdfs:comment "You touch a creature. The creature's jump distance is tripled until the spell ends."@en .

DnD5eCharacter:Knock 	a rdfs:Class ;
              rdfs:subClassOf TTRpg:Spell ;
              DnD5eCharacter:inMagicSchool DnD5eCharacter:Transmutation ;
              rdfs:label "Knock"@en ;
              rdfs:comment "Choose an object that you can see within range. The object can be a door, a box, a chest, a set of manacles, a padlock, or another object that contains a mundane or magical means that prevents access."@en .

DnD5eCharacter:LegendLore 	a rdfs:Class ;
              rdfs:subClassOf TTRpg:Spell ;
              DnD5eCharacter:inMagicSchool DnD5eCharacter:Divination ;
              rdfs:label "Legend Lore"@en ;
              rdfs:comment "Name or describe a person, place, or object. The spell brings to your mind a brief summary of the significant lore about the thing you named. The lore might consist of current tales, forgotten stories, or even secret lore that has never been widely known. If the thing you named isn't of legendary importance, you gain no information. The more information you already have about the thing, the more precise and detailed the information you receive is."@en .

DnD5eCharacter:LesserRestoration 	a rdfs:Class ;
              rdfs:subClassOf TTRpg:Spell ;
              DnD5eCharacter:inMagicSchool DnD5eCharacter:Abjuration ;
              rdfs:label "Lesser Restoration"@en ;
              rdfs:comment "You touch a creature and can end either one disease or one condition afflicting it. The condition can be blinded, deafened, paralyzed, or poisoned."@en .

DnD5eCharacter:Levitate 	a rdfs:Class ;
              rdfs:subClassOf TTRpg:Spell ;
              DnD5eCharacter:inMagicSchool DnD5eCharacter:Transmutation ;
              rdfs:label "Levitate"@en ;
              rdfs:comment "One creature or object of your choice that you can see within range rises vertically, up to 20 feet, and remains suspended there for the duration. The spell can levitate a target that weighs up to 500 pounds. An unwilling creature that succeeds on a constitution saving throw is unaffected."@en .

DnD5eCharacter:Light 	a rdfs:Class ;
              rdfs:subClassOf TTRpg:Spell ;
              DnD5eCharacter:inMagicSchool DnD5eCharacter:Evocation ;
              rdfs:label "Light"@en ;
              rdfs:comment "You touch one object that is no larger than 10 feet in any dimension. Until the spell ends, the object sheds bright light in a 20-foot radius and dim light for an additional 20 feet. The light can be colored as you like. Completely covering the object with something opaque blocks the light. The spell ends if you cast it again or dismiss it as an action."@en .

DnD5eCharacter:LightningBolt 	a rdfs:Class ;
              rdfs:subClassOf TTRpg:Spell ;
              DnD5eCharacter:inMagicSchool DnD5eCharacter:Evocation ;
              rdfs:label "Lightning Bolt"@en ;
              rdfs:comment "A stroke of lightning forming a line 100 feet long and 5 feet wide blasts out from you in a direction you choose. Each creature in the line must make a dexterity saving throw. A creature takes 8d6 lightning damage on a failed save, or half as much damage on a successful one."@en .

DnD5eCharacter:LocateAnimalsOrPlants 	a rdfs:Class ;
              rdfs:subClassOf TTRpg:Spell ;
              DnD5eCharacter:inMagicSchool DnD5eCharacter:Divination ;
              rdfs:label "Locate Animals Or Plants"@en ;
              rdfs:comment "Describe or name a specific kind of beast or plant. Concentrating on the voice of nature in your surroundings, you learn the direction and distance to the closest creature or plant of that kind within 5 miles, if any are present."@en .

DnD5eCharacter:LocateCreature 	a rdfs:Class ;
              rdfs:subClassOf TTRpg:Spell ;
              DnD5eCharacter:inMagicSchool DnD5eCharacter:Divination ;
              rdfs:label "Locate Creature"@en ;
              rdfs:comment "Describe or name a creature that is familiar to you. You sense the direction to the creature's location, as long as that creature is within 1,000 feet of you. If the creature is moving, you know the direction of its movement."@en .

DnD5eCharacter:LocateObject 	a rdfs:Class ;
              rdfs:subClassOf TTRpg:Spell ;
              DnD5eCharacter:inMagicSchool DnD5eCharacter:Divination ;
              rdfs:label "Locate Object"@en ;
              rdfs:comment "Describe or name an object that is familiar to you. You sense the direction to the object's location, as long as that object is within 1,000 feet of you. If the object is in motion, you know the direction of its movement."@en .

DnD5eCharacter:Longstrider 	a rdfs:Class ;
              rdfs:subClassOf TTRpg:Spell ;
              DnD5eCharacter:inMagicSchool DnD5eCharacter:Transmutation ;
              rdfs:label "Longstrider"@en ;
              rdfs:comment "You touch a creature. The target's speed increases by 10 feet until the spell ends."@en .

DnD5eCharacter:MageArmor 	a rdfs:Class ;
              rdfs:subClassOf TTRpg:Spell ;
              DnD5eCharacter:inMagicSchool DnD5eCharacter:Abjuration ;
              rdfs:label "Mage Armor"@en ;
              rdfs:comment "You touch a willing creature who isn't wearing armor, and a protective magical force surrounds it until the spell ends. The target's base AC becomes 13 + its Dexterity modifier. The spell ends if the target dons armor or if you dismiss the spell as an action."@en .

DnD5eCharacter:MageHand 	a rdfs:Class ;
              rdfs:subClassOf TTRpg:Spell ;
              DnD5eCharacter:inMagicSchool DnD5eCharacter:Conjuration ;
              rdfs:label "Mage Hand"@en ;
              rdfs:comment "A spectral, floating hand appears at a point you choose within range. The hand lasts for the duration or until you dismiss it as an action. The hand vanishes if it is ever more than 30 feet away from you or if you cast this spell again."@en .

DnD5eCharacter:MagicCircle 	a rdfs:Class ;
              rdfs:subClassOf TTRpg:Spell ;
              DnD5eCharacter:inMagicSchool DnD5eCharacter:Abjuration ;
              rdfs:label "Magic Circle"@en ;
              rdfs:comment "You create a 10-foot radius, 20-foot-tall cylinder of magical energy centered on a point on the ground that you can see within range. Glowing runes appear whetever the cylinder intersects with the floor or other surface."@en .

DnD5eCharacter:MagicJar 	a rdfs:Class ;
              rdfs:subClassOf TTRpg:Spell ;
              DnD5eCharacter:inMagicSchool DnD5eCharacter:Necromancy ;
              rdfs:label "Magic Jar"@en ;
              rdfs:comment "Your body falls into a catatonic state as your soul leaves it and enters the container you used for the spell's material component. While your soul inhabits the container, you are aware of your surroundings as if you were in the container's space. You can't move or use reactions. The only action you can take is to project your soul up to 100 feet out of the container, either returning to your living body (and ending the spell) or attempting to possess a humanoids body."@en .

DnD5eCharacter:MagicMissile 	a rdfs:Class ;
              rdfs:subClassOf TTRpg:Spell ;
              DnD5eCharacter:inMagicSchool DnD5eCharacter:Evocation ;
              rdfs:label "Magic Missile"@en ;
              rdfs:comment "You create three glowing darts of magical force. Each dart hits a creature of your choice that you can see within range. A dart deals 1d4 + 1 force damage to its target. The darts all strike simultaneously, and you can direct them to hit one creature or several."@en .

DnD5eCharacter:MagicMouth 	a rdfs:Class ;
              rdfs:subClassOf TTRpg:Spell ;
              DnD5eCharacter:inMagicSchool DnD5eCharacter:Illusion ;
              rdfs:label "Magic Mouth"@en ;
              rdfs:comment "You plant a message to an object in the range of the spell. The message is verbalized when the trigger conditions are met. Choose an object that you see, and that is not worn or carried by another creature. Then say the message, which should not exceed 25 words but listening can take up to 10 minutes. Finally, establish the circumstances that trigger the spell to deliver your message."@en .

DnD5eCharacter:MagicWeapon 	a rdfs:Class ;
              rdfs:subClassOf TTRpg:Spell ;
              DnD5eCharacter:inMagicSchool DnD5eCharacter:Transmutation ;
              rdfs:label "Magic Weapon"@en ;
              rdfs:comment "You touch a nonmagical weapon. Until the spell ends, that weapon becomes a magic weapon with a +1 bonus to attack rolls and damage rolls."@en .

DnD5eCharacter:MagnificentMansion 	a rdfs:Class ;
              rdfs:subClassOf TTRpg:Spell ;
              DnD5eCharacter:inMagicSchool DnD5eCharacter:Conjuration ;
              rdfs:label "Magnificent Mansion"@en ;
              rdfs:comment "You conjure an extradimensional dwelling in range that lasts for the duration. You choose where its one entrance is located. The entrance shimmers faintly and is 5 feet wide and 10 feet tall. You and any creature you designate when you cast the spell can enter the extradimensional dwelling as long as the portal remains open. You can open or close the portal if you are within 30 feet of it. While closed, the portal is invisible."@en .

DnD5eCharacter:MajorImage 	a rdfs:Class ;
              rdfs:subClassOf TTRpg:Spell ;
              DnD5eCharacter:inMagicSchool DnD5eCharacter:Illusion ;
              rdfs:label "Major Image"@en ;
              rdfs:comment "You create the image of an object, a creature, or some other visible phenomenon that is no larger than a 20-foot cube. The image appears at a spot that you can see within range and lasts for the duration. It seems completely real, including sounds, smells, and temperature appropriate to the thing depicted. You can't create sufficient heat or cold to cause damage, a sound loud enough to deal thunder damage or deafen a creature, or a smell that might sicken a creature (like a troglodyte's stench)."@en .

DnD5eCharacter:MassCureWounds 	a rdfs:Class ;
              rdfs:subClassOf TTRpg:Spell ;
              DnD5eCharacter:inMagicSchool DnD5eCharacter:Conjuration ;
              rdfs:label "Mass Cure Wounds"@en ;
              rdfs:comment "A wave of healing energy washes out from a point of your choice within range. Choose up to six creatures in a 30-foot-radius sphere centered on that point. Each target regains hit points equal to 3d8 + your spellcasting ability modifier. This spell has no effect on undead or constructs."@en .

DnD5eCharacter:MassHeal 	a rdfs:Class ;
              rdfs:subClassOf TTRpg:Spell ;
              DnD5eCharacter:inMagicSchool DnD5eCharacter:Conjuration ;
              rdfs:label "Mass Heal"@en ;
              rdfs:comment "A flood of healing energy flows from you into injured creatures around you. You restore up to 700 hit points, divided as you choose among any number of creatures that you can see within range. Creatures healed by this spell are also cured of all diseases and any effect making them blinded or deafened. This spell has no effect on undead or constructs."@en .

DnD5eCharacter:MassHealingWord 	a rdfs:Class ;
              rdfs:subClassOf TTRpg:Spell ;
              DnD5eCharacter:inMagicSchool DnD5eCharacter:Evocation ;
              rdfs:label "Mass Healing Word"@en ;
              rdfs:comment "As you call out words of restoration, up to six creatures of your choice that you can see within range regain hit points equal to 1d4 + your spellcasting ability modifier. This spell has no effect on undead or constructs."@en .

DnD5eCharacter:MassSuggestion 	a rdfs:Class ;
              rdfs:subClassOf TTRpg:Spell ;
              DnD5eCharacter:inMagicSchool DnD5eCharacter:Enchantment ;
              rdfs:label "Mass Suggestion"@en ;
              rdfs:comment "You suggest a course of activity (limited to a sentence or two) and magically influence up to twelve creatures of your choice that you can see within range and that can hear and understand you. Creatures that can't be charmed are immune to this effect. The suggestion must be worded in such a manner as to make the course of action sound reasonable. Asking the creature to stab itself, throw itself onto a spear, immolate itself, or do some other obviously harmful act automatically negates the effect of the spell."@en .

DnD5eCharacter:Maze 	a rdfs:Class ;
              rdfs:subClassOf TTRpg:Spell ;
              DnD5eCharacter:inMagicSchool DnD5eCharacter:Conjuration ;
              rdfs:label "Maze"@en ;
              rdfs:comment "You banish a creature that you can see within range into a labyrinthine demiplane. The target remains there for the duration or until it escapes the maze."@en .

DnD5eCharacter:MeldIntoStone 	a rdfs:Class ;
              rdfs:subClassOf TTRpg:Spell ;
              DnD5eCharacter:inMagicSchool DnD5eCharacter:Transmutation ;
              rdfs:label "Meld Into Stone"@en ;
              rdfs:comment "You step into a stone object or surface large enough to fully contain your body, melding yourself and all the equipment you carry with the stone for the duration. Using your movement, you step into the stone at a point you can touch. Nothing of your presence remains visible or otherwise detectable by nonmagical senses."@en .

DnD5eCharacter:Mending 	a rdfs:Class ;
              rdfs:subClassOf TTRpg:Spell ;
              DnD5eCharacter:inMagicSchool DnD5eCharacter:Transmutation ;
              rdfs:label "Mending"@en ;
              rdfs:comment "This spell repairs a single break or tear in an object you touch, such as a broken key, a torn cloak, or a leaking wineskin. As long as the break or tear is no longer than 1 foot in any dimension, you mend it, leaving no trace of the former damage."@en .

DnD5eCharacter:Message 	a rdfs:Class ;
              rdfs:subClassOf TTRpg:Spell ;
              DnD5eCharacter:inMagicSchool DnD5eCharacter:Transmutation ;
              rdfs:label "Message"@en ;
              rdfs:comment "You point your finger toward a creature within range and whisper a message. The target (and only the target) hears the message and can reply in a whisper that only you can hear."@en .

DnD5eCharacter:MeteorSwarm 	a rdfs:Class ;
              rdfs:subClassOf TTRpg:Spell ;
              DnD5eCharacter:inMagicSchool DnD5eCharacter:Evocation ;
              rdfs:label "Meteor Swarm"@en ;
              rdfs:comment "Blazing orbs of fire plummet to the ground at four different points you can see within range. Each creature in a 40-foot-radius sphere centered on each point you choose must make a dexterity saving throw. The sphere spreads around corners. A creature takes 20d6 fire damage and 20d6 bludgeoning damage on a failed save, or half as much damage on a successful one. A creature in the area of more than one fiery burst is affected only once."@en .

DnD5eCharacter:MindBlank 	a rdfs:Class ;
              rdfs:subClassOf TTRpg:Spell ;
              DnD5eCharacter:inMagicSchool DnD5eCharacter:Abjuration ;
              rdfs:label "Mind Blank"@en ;
              rdfs:comment "Until the spell ends, one willing creature you touch is immune to psychic damage, any effect that would sense its emotions or read its thoughts, divination spells, and the charmed condition. The spell even foils wish spells and spells or effects of similar power used to affect the target's mind or to gain information about the target."@en .

DnD5eCharacter:MinorIllusion 	a rdfs:Class ;
              rdfs:subClassOf TTRpg:Spell ;
              DnD5eCharacter:inMagicSchool DnD5eCharacter:Illusion ;
              rdfs:label "Minor Illusion"@en ;
              rdfs:comment "You create a sound or an image of an object within range that lasts for the duration. The illusion also ends if you dismiss it as an action or cast this spell again."@en .

DnD5eCharacter:MirageArcane 	a rdfs:Class ;
              rdfs:subClassOf TTRpg:Spell ;
              DnD5eCharacter:inMagicSchool DnD5eCharacter:Illusion ;
              rdfs:label "Mirage Arcane"@en ;
              rdfs:comment "You make terrain in an area up to 1 mile square look, sound, smell, and even feel like some other sort of terrain. The terrain's general shape remains the same, however. Open fields or a road could be made to resemble a swamp, hill, crevasse, or some other difficult or impassable terrain. A pond can be made to seem like a grassy meadow, a precipice like a gentle slope, or a rock-strewn gully like a wide and smooth road."@en .

DnD5eCharacter:MirrorImage 	a rdfs:Class ;
              rdfs:subClassOf TTRpg:Spell ;
              DnD5eCharacter:inMagicSchool DnD5eCharacter:Illusion ;
              rdfs:label "Mirror Image"@en ;
              rdfs:comment "Three illusory duplicates of yourself appear in your space. Until the spell ends, the duplicates move with you and mimic your actions, shifting position so it's impossible to track which image is real. You can use your action to dismiss the illusory duplicates."@en .

DnD5eCharacter:Mislead 	a rdfs:Class ;
              rdfs:subClassOf TTRpg:Spell ;
              DnD5eCharacter:inMagicSchool DnD5eCharacter:Illusion ;
              rdfs:label "Mislead"@en ;
              rdfs:comment "You become invisible at the same time that an illusory double of you appears where you are standing. The double lasts for the duration, but the invisibility ends if you attack or cast a spell."@en .

DnD5eCharacter:MistyStep 	a rdfs:Class ;
              rdfs:subClassOf TTRpg:Spell ;
              DnD5eCharacter:inMagicSchool DnD5eCharacter:Conjuration ;
              rdfs:label "Misty Step"@en ;
              rdfs:comment "Briefly surrounded by silvery mist, you teleport up to 30 feet to an unoccupied space that you can see."@en .

DnD5eCharacter:ModifyMemory 	a rdfs:Class ;
              rdfs:subClassOf TTRpg:Spell ;
              DnD5eCharacter:inMagicSchool DnD5eCharacter:Enchantment ;
              rdfs:label "Modify Memory"@en ;
              rdfs:comment "You attempt to reshape another creature's memories. One creature that you can see must make a wisdom saving throw. If you are fighting the creature, it has advantage on the saving throw. On a failed save, the target becomes charmed by you for the duration. The charmed target is incapacitated and unaware of its surroundings, though it can still hear you. If it takes any damage or is targeted by another spell, this spell ends, and none of the target's memories are modified."@en .

DnD5eCharacter:Moonbeam 	a rdfs:Class ;
              rdfs:subClassOf TTRpg:Spell ;
              DnD5eCharacter:inMagicSchool DnD5eCharacter:Evocation ;
              rdfs:label "Moonbeam"@en ;
              rdfs:comment "A silvery beam of pale light shines down in a 5-foot radius, 40-foot-high cylinder centered on a point within range. Until the spell ends, dim light fills the cylinder."@en .

DnD5eCharacter:MoveEarth 	a rdfs:Class ;
              rdfs:subClassOf TTRpg:Spell ;
              DnD5eCharacter:inMagicSchool DnD5eCharacter:Transmutation ;
              rdfs:label "Move Earth"@en ;
              rdfs:comment "Choose an area of terrain no larger than 40 feet on a side within range. You can reshape dirt, sand, or clay in the area in any manner you choose for the duration. You can raise or lower the area's elevation, create or fill in a trench, erect or flatten a wall, or form a pillar. The extent of any such changes can't exceed half the area's largest dimension. So, if you affect a 40-foot square, you can create a pillar up to 20 feet high, raise or lower the square's elevation by up to 20 feet, dig a trench up to 20 feet deep, and so on. It takes 10 minutes for these changes to complete."@en .

DnD5eCharacter:Nondetection 	a rdfs:Class ;
              rdfs:subClassOf TTRpg:Spell ;
              DnD5eCharacter:inMagicSchool DnD5eCharacter:Abjuration ;
              rdfs:label "Nondetection"@en ;
              rdfs:comment "For the duration, you hide a target that you touch from divination magic. The target can be a willing creature or a place or an object no larger than 10 feet in any dimension. The target can't be targeted by any divination magic or perceived through magical scrying sensors."@en .

DnD5eCharacter:PassWithoutTrace 	a rdfs:Class ;
              rdfs:subClassOf TTRpg:Spell ;
              DnD5eCharacter:inMagicSchool DnD5eCharacter:Abjuration ;
              rdfs:label "Pass Without Trace"@en ;
              rdfs:comment "A veil of shadows and silence radiates from you, masking you and your companions from detection. For the duration, each creature you choose within 30 feet of you (including you) has a +10 bonus to Dexterity (Stealth) checks and can't be tracked except by magical means. A creature that receives this bonus leaves behind no tracks or other traces of its passage."@en .

DnD5eCharacter:Passwall 	a rdfs:Class ;
              rdfs:subClassOf TTRpg:Spell ;
              DnD5eCharacter:inMagicSchool DnD5eCharacter:Transmutation ;
              rdfs:label "Passwall"@en ;
              rdfs:comment "A passage appears at a point of your choice that you can see on a wooden, plaster, or stone surface (such as a wall, a ceiling, or a floor) within range, and lasts for the duration. You choose the opening's dimensions: up to 5 feet wide, 8 feet tall, and 20 feet deep. The passage creates no instability in a structure surrounding it."@en .

DnD5eCharacter:PhantasmalKiller 	a rdfs:Class ;
              rdfs:subClassOf TTRpg:Spell ;
              DnD5eCharacter:inMagicSchool DnD5eCharacter:Illusion ;
              rdfs:label "Phantasmal Killer"@en ;
              rdfs:comment "You tap into the nightmares of a creature you can see within range and create an illusory manifestation of its deepest fears, visible only to that creature. The target must make a wisdom saving throw. On a failed save, the target becomes frightened for the duration. At the start of each of the target's turns before the spell ends, the target must succeed on a wisdom saving throw or take 4d10 psychic damage. On a successful save, the spell ends."@en .

DnD5eCharacter:PhantomSteed 	a rdfs:Class ;
              rdfs:subClassOf TTRpg:Spell ;
              DnD5eCharacter:inMagicSchool DnD5eCharacter:Illusion ;
              rdfs:label "Phantom Steed"@en ;
              rdfs:comment "A Large quasi-real, horselike creature appears on the ground in an unoccupied space of your choice within range. You decide the creature's appearance, but it is equipped with a saddle, bit, and bridle. Any of the equipment created by the spell vanishes in a puff of smoke if it is carried more than 10 feet away from the steed."@en .

DnD5eCharacter:PlanarAlly 	a rdfs:Class ;
              rdfs:subClassOf TTRpg:Spell ;
              DnD5eCharacter:inMagicSchool DnD5eCharacter:Conjuration ;
              rdfs:label "Planar Ally"@en ;
              rdfs:comment "You beseech an otherworldly entity for aid. The being must be known to you: a god, a primordial, a demon prince, or some other being of cosmic power. That entity sends a celestial, an elemental, or a fiend loyal to it to aid you, making the creature appear in an unoccupied space within range. If you know a specific creature's name, you can speak that name when you cast this spell to request that creature, though you might get a different creature anyway (DM's choice)."@en .

DnD5eCharacter:PlanarBinding 	a rdfs:Class ;
              rdfs:subClassOf TTRpg:Spell ;
              DnD5eCharacter:inMagicSchool DnD5eCharacter:Abjuration ;
              rdfs:label "Planar Binding"@en ;
              rdfs:comment "With this spell, you attempt to bind a celestial, an elemental, a fey, or a fiend to your service. The creature must be within range for the entire casting of the spell. (Typically, the creature is first summoned into the center of an inverted magic circle in order to keep it trapped while this spell is cast.) At the completion of the casting, the target must make a charisma saving throw. On a failed save, it is bound to serve you for the duration. If the creature was summoned or created by another spell, that spell's duration is extended to match the duration of this spell."@en .

DnD5eCharacter:PlaneShift 	a rdfs:Class ;
              rdfs:subClassOf TTRpg:Spell ;
              DnD5eCharacter:inMagicSchool DnD5eCharacter:Conjuration ;
              rdfs:label "Plane Shift"@en ;
              rdfs:comment "You and up to eight willing creatures who link hands in a circle are transported to a different plane of existence. You can specify a target destination in general terms, such as the City of Brass on the Elemental Plane of Fire or the palace of Dispater on the second level of the Nine Hells, and you appear in or near that destination. If you are trying to reach the City of Brass, for example, you might arrive in its Street of Steel, before its Gate of Ashes, or looking at the city from across the Sea of Fire, at the DM's discretion."@en .

DnD5eCharacter:PlantGrowth 	a rdfs:Class ;
              rdfs:subClassOf TTRpg:Spell ;
              DnD5eCharacter:inMagicSchool DnD5eCharacter:Transmutation ;
              rdfs:label "Plant Growth"@en ;
              rdfs:comment "This spell channels vitality into plants within a specific area. There are two possible uses for the spell, granting either immediate or long-term benefits."@en .

DnD5eCharacter:PoisonSpray 	a rdfs:Class ;
              rdfs:subClassOf TTRpg:Spell ;
              DnD5eCharacter:inMagicSchool DnD5eCharacter:Conjuration ;
              rdfs:label "Poison Spray"@en ;
              rdfs:comment "You extend your hand toward a creature you can see within range and project a puff of noxious gas from your palm. The creature must succeed on a constitution saving throw or take 1d12 poison damage."@en .

DnD5eCharacter:Polymorph 	a rdfs:Class ;
              rdfs:subClassOf TTRpg:Spell ;
              DnD5eCharacter:inMagicSchool DnD5eCharacter:Transmutation ;
              rdfs:label "Polymorph"@en ;
              rdfs:comment "This spell transforms a creature that you can see within range into a new form. An unwilling creature must make a wisdom saving throw to avoid the effect. A shapechanger automatically succeeds on this saving throw."@en .

DnD5eCharacter:PowerWordKill 	a rdfs:Class ;
              rdfs:subClassOf TTRpg:Spell ;
              DnD5eCharacter:inMagicSchool DnD5eCharacter:Enchantment ;
              rdfs:label "Power Word Kill"@en ;
              rdfs:comment "You utter a word of power that can compel one creature you can see within range to die instantly. If the creature you choose has 100 hit points or fewer, it dies. Otherwise, the spell has no effect."@en .

DnD5eCharacter:PowerWordStun 	a rdfs:Class ;
              rdfs:subClassOf TTRpg:Spell ;
              DnD5eCharacter:inMagicSchool DnD5eCharacter:Enchantment ;
              rdfs:label "Power Word Stun"@en ;
              rdfs:comment "You speak a word of power that can overwhelm the mind of one creature you can see within range, leaving it dumbfounded. If the target has 150 hit points or fewer, it is stunned. Otherwise, the spell has no effect."@en .

DnD5eCharacter:PrayerOfHealing 	a rdfs:Class ;
              rdfs:subClassOf TTRpg:Spell ;
              DnD5eCharacter:inMagicSchool DnD5eCharacter:Evocation ;
              rdfs:label "Prayer Of Healing"@en ;
              rdfs:comment "Up to six creatures of your choice that you can see within range each regain hit points equal to 2d8 + your spellcasting ability modifier. This spell has no effect on undead or constructs."@en .

DnD5eCharacter:Prestidigitation 	a rdfs:Class ;
              rdfs:subClassOf TTRpg:Spell ;
              DnD5eCharacter:inMagicSchool DnD5eCharacter:Transmutation ;
              rdfs:label "Prestidigitation"@en ;
              rdfs:comment "This spell is a minor magical trick that novice spellcasters use for practice. You create one of the following magical effects within 'range':"@en .

DnD5eCharacter:PrismaticSpray 	a rdfs:Class ;
              rdfs:subClassOf TTRpg:Spell ;
              DnD5eCharacter:inMagicSchool DnD5eCharacter:Evocation ;
              rdfs:label "Prismatic Spray"@en ;
              rdfs:comment "Eight multicolored rays of light flash from your hand. Each ray is a different color and has a different power and purpose. Each creature in a 60-foot cone must make a dexterity saving throw. For each target, roll a d8 to determine which color ray affects it."@en .

DnD5eCharacter:PrismaticWall 	a rdfs:Class ;
              rdfs:subClassOf TTRpg:Spell ;
              DnD5eCharacter:inMagicSchool DnD5eCharacter:Abjuration ;
              rdfs:label "Prismatic Wall"@en ;
              rdfs:comment "A shimmering, multicolored plane of light forms a vertical opaque wall--up to 90 feet long, 30 feet high, and 1 inch thick--centered on a point you can see within range. Alternatively, you can shape the wall into a sphere up to 30 feet in diameter centered on a point you choose within range. The wall remains in place for the duration. If you position the wall so that it passes through a space occupied by a creature, the spell fails, and your action and the spell slot are wasted."@en .

DnD5eCharacter:PrivateSanctum 	a rdfs:Class ;
              rdfs:subClassOf TTRpg:Spell ;
              DnD5eCharacter:inMagicSchool DnD5eCharacter:Abjuration ;
              rdfs:label "Private Sanctum"@en ;
              rdfs:comment "You make an area within range magically secure. The area is a cube that can be as small as 5 feet to as large as 100 feet on each side. The spell lasts for the duration or until you use an action to dismiss it."@en .

DnD5eCharacter:ProduceFlame 	a rdfs:Class ;
              rdfs:subClassOf TTRpg:Spell ;
              DnD5eCharacter:inMagicSchool DnD5eCharacter:Conjuration ;
              rdfs:label "Produce Flame"@en ;
              rdfs:comment "A flickering flame appears in your hand. The flame remains there for the duration and harms neither you nor your equipment. The flame sheds bright light in a 10-foot radius and dim light for an additional 10 feet. The spell ends if you dismiss it as an action or if you cast it again."@en .

DnD5eCharacter:ProgrammedIllusion 	a rdfs:Class ;
              rdfs:subClassOf TTRpg:Spell ;
              DnD5eCharacter:inMagicSchool DnD5eCharacter:Illusion ;
              rdfs:label "Programmed Illusion"@en ;
              rdfs:comment "You create an illusion of an object, a creature, or some other visible phenomenon within range that activates when a specific condition occurs. The illusion is imperceptible until then. It must be no larger than a 30-foot cube, and you decide when you cast the spell how the illusion behaves and what sounds it makes. This scripted performance can last up to 5 minutes."@en .

DnD5eCharacter:ProjectImage 	a rdfs:Class ;
              rdfs:subClassOf TTRpg:Spell ;
              DnD5eCharacter:inMagicSchool DnD5eCharacter:Illusion ;
              rdfs:label "Project Image"@en ;
              rdfs:comment "You create an illusory copy of yourself that lasts for the duration. The copy can appear at any location within range that you have seen before, regardless of intervening obstacles. The illusion looks and sounds like you but is intangible. If the illusion takes any damage, it disappears, and the spell ends."@en .

DnD5eCharacter:ProtectionFromEnergy 	a rdfs:Class ;
              rdfs:subClassOf TTRpg:Spell ;
              DnD5eCharacter:inMagicSchool DnD5eCharacter:Abjuration ;
              rdfs:label "Protection From Energy"@en ;
              rdfs:comment "For the duration, the willing creature you touch has resistance to one damage type of your choice: acid, cold, fire, lightning, or thunder."@en .

DnD5eCharacter:ProtectionFromEvilAndGood 	a rdfs:Class ;
              rdfs:subClassOf TTRpg:Spell ;
              DnD5eCharacter:inMagicSchool DnD5eCharacter:Abjuration ;
              rdfs:label "Protection From Evil And Good"@en ;
              rdfs:comment "Until the spell ends, one willing creature you touch is protected against certain types of creatures: aberrations, celestials, elementals, fey, fiends, and undead."@en .

DnD5eCharacter:ProtectionFromPoison 	a rdfs:Class ;
              rdfs:subClassOf TTRpg:Spell ;
              DnD5eCharacter:inMagicSchool DnD5eCharacter:Abjuration ;
              rdfs:label "Protection From Poison"@en ;
              rdfs:comment "You touch a creature. If it is poisoned, you neutralize the poison. If more than one poison afflicts the target, you neutralize one poison that you know is present, or you neutralize one at random."@en .

DnD5eCharacter:PurifyFoodAndDrink 	a rdfs:Class ;
              rdfs:subClassOf TTRpg:Spell ;
              DnD5eCharacter:inMagicSchool DnD5eCharacter:Transmutation ;
              rdfs:label "Purify Food And Drink"@en ;
              rdfs:comment "All nonmagical food and drink within a 5-foot radius sphere centered on a point of your choice within range is purified and rendered free of poison and disease."@en .

DnD5eCharacter:RaiseDead 	a rdfs:Class ;
              rdfs:subClassOf TTRpg:Spell ;
              DnD5eCharacter:inMagicSchool DnD5eCharacter:Necromancy ;
              rdfs:label "Raise Dead"@en ;
              rdfs:comment "You return a dead creature you touch to life, provided that it has been dead no longer than 10 days. If the creature's soul is both willing and at liberty to rejoin the body, the creature returns to life with 1 hit point."@en .

DnD5eCharacter:RayOfEnfeeblement 	a rdfs:Class ;
              rdfs:subClassOf TTRpg:Spell ;
              DnD5eCharacter:inMagicSchool DnD5eCharacter:Necromancy ;
              rdfs:label "Ray Of Enfeeblement"@en ;
              rdfs:comment "A black beam of enervating energy springs from your finger toward a creature within range. Make a ranged spell attack against the target. On a hit, the target deals only half damage with weapon attacks that use Strength until the spell ends."@en .

DnD5eCharacter:RayOfFrost 	a rdfs:Class ;
              rdfs:subClassOf TTRpg:Spell ;
              DnD5eCharacter:inMagicSchool DnD5eCharacter:Evocation ;
              rdfs:label "Ray Of Frost"@en ;
              rdfs:comment "A frigid beam of blue-white light streaks toward a creature within range. Make a ranged spell attack against the target. On a hit, it takes 1d8 cold damage, and its speed is reduced by 10 feet until the start of your next turn."@en .

DnD5eCharacter:Regenerate 	a rdfs:Class ;
              rdfs:subClassOf TTRpg:Spell ;
              DnD5eCharacter:inMagicSchool DnD5eCharacter:Transmutation ;
              rdfs:label "Regenerate"@en ;
              rdfs:comment "You touch a creature and stimulate its natural healing ability. The target regains 4d8 + 15 hit points. For the duration of the spell, the target regains 1 hit point at the start of each of its turns (10 hit points each minute)."@en .

DnD5eCharacter:Reincarnate 	a rdfs:Class ;
              rdfs:subClassOf TTRpg:Spell ;
              DnD5eCharacter:inMagicSchool DnD5eCharacter:Transmutation ;
              rdfs:label "Reincarnate"@en ;
              rdfs:comment "You touch a dead humanoid or a piece of a dead humanoid. Provided that the creature has been dead no longer than 10 days, the spell forms a new adult body for it and then calls the soul to enter that body. If the target's soul isn't free or willing to do so, the spell fails."@en .

DnD5eCharacter:RemoveCurse 	a rdfs:Class ;
              rdfs:subClassOf TTRpg:Spell ;
              DnD5eCharacter:inMagicSchool DnD5eCharacter:Abjuration ;
              rdfs:label "Remove Curse"@en ;
              rdfs:comment "At your touch, all curses affecting one creature or object end. If the object is a cursed magic item, its curse remains, but the spell breaks its owner's attunement to the object so it can be removed or discarded."@en .

DnD5eCharacter:ResilientSphere 	a rdfs:Class ;
              rdfs:subClassOf TTRpg:Spell ;
              DnD5eCharacter:inMagicSchool DnD5eCharacter:Evocation ;
              rdfs:label "Resilient Sphere"@en ;
              rdfs:comment "A sphere of shimmering force encloses a creature or object of Large size or smaller within range. An unwilling creature must make a dexterity saving throw. On a failed save, the creature is enclosed for the duration."@en .

DnD5eCharacter:Resistance 	a rdfs:Class ;
              rdfs:subClassOf TTRpg:Spell ;
              DnD5eCharacter:inMagicSchool DnD5eCharacter:Abjuration ;
              rdfs:label "Resistance"@en ;
              rdfs:comment "You touch one willing creature. Once before the spell ends, the target can roll a d4 and add the number rolled to one saving throw of its choice. It can roll the die before or after making the saving throw. The spell then ends."@en .

DnD5eCharacter:Resurrection 	a rdfs:Class ;
              rdfs:subClassOf TTRpg:Spell ;
              DnD5eCharacter:inMagicSchool DnD5eCharacter:Necromancy ;
              rdfs:label "Resurrection"@en ;
              rdfs:comment "You touch a dead creature that has been dead for no more than a century, that didn't die of old age, and that isn't undead. If its soul is free and willing, the target returns to life with all its hit points."@en .

DnD5eCharacter:ReverseGravity 	a rdfs:Class ;
              rdfs:subClassOf TTRpg:Spell ;
              DnD5eCharacter:inMagicSchool DnD5eCharacter:Transmutation ;
              rdfs:label "Reverse Gravity"@en ;
              rdfs:comment "This spell reverses gravity in a 50-foot-radius, 100-foot high cylinder centered on a point within range. All creatures and objects that aren't somehow anchored to the ground in the area fall upward and reach the top of the area when you cast this spell. A creature can make a dexterity saving throw to grab onto a fixed object it can reach, thus avoiding the fall."@en .

DnD5eCharacter:Revivify 	a rdfs:Class ;
              rdfs:subClassOf TTRpg:Spell ;
              DnD5eCharacter:inMagicSchool DnD5eCharacter:Conjuration ;
              rdfs:label "Revivify"@en ;
              rdfs:comment "You touch a creature that has died within the last minute. That creature returns to life with 1 hit point. This spell can't return to life a creature that has died of old age, nor can it restore any missing body parts."@en .

DnD5eCharacter:RopeTrick 	a rdfs:Class ;
              rdfs:subClassOf TTRpg:Spell ;
              DnD5eCharacter:inMagicSchool DnD5eCharacter:Transmutation ;
              rdfs:label "Rope Trick"@en ;
              rdfs:comment "You touch a length of rope that is up to 60 feet long. One end of the rope then rises into the air until the whole rope hangs perpendicular to the ground. At the upper end of the rope, an invisible entrance opens to an extradimensional space that lasts until the spell ends."@en .

DnD5eCharacter:SacredFlame 	a rdfs:Class ;
              rdfs:subClassOf TTRpg:Spell ;
              DnD5eCharacter:inMagicSchool DnD5eCharacter:Evocation ;
              rdfs:label "Sacred Flame"@en ;
              rdfs:comment "Flame-like radiance descends on a creature that you can see within range. The target must succeed on a dexterity saving throw or take 1d8 radiant damage. The target gains no benefit from cover for this saving throw."@en .

DnD5eCharacter:Sanctuary 	a rdfs:Class ;
              rdfs:subClassOf TTRpg:Spell ;
              DnD5eCharacter:inMagicSchool DnD5eCharacter:Abjuration ;
              rdfs:label "Sanctuary"@en ;
              rdfs:comment "You ward a creature within range against attack. Until the spell ends, any creature who targets the warded creature with an attack or a harmful spell must first make a wisdom saving throw. On a failed save, the creature must choose a new target or lose the attack or spell. This spell doesn't protect the warded creature from area effects, such as the explosion of a fireball."@en .

DnD5eCharacter:ScorchingRay 	a rdfs:Class ;
              rdfs:subClassOf TTRpg:Spell ;
              DnD5eCharacter:inMagicSchool DnD5eCharacter:Evocation ;
              rdfs:label "Scorching Ray"@en ;
              rdfs:comment "You create three rays of fire and hurl them at targets within range. You can hurl them at one target or several."@en .

DnD5eCharacter:Scrying 	a rdfs:Class ;
              rdfs:subClassOf TTRpg:Spell ;
              DnD5eCharacter:inMagicSchool DnD5eCharacter:Divination ;
              rdfs:label "Scrying"@en ;
              rdfs:comment "You can see and hear a particular creature you choose that is on the same plane of existence as you. The target must make a wisdom saving throw, which is modified by how well you know the target and the sort of physical connection you have to it. If a target knows you're casting this spell, it can fail the saving throw voluntarily if it wants to be observed."@en .

DnD5eCharacter:SecretChest 	a rdfs:Class ;
              rdfs:subClassOf TTRpg:Spell ;
              DnD5eCharacter:inMagicSchool DnD5eCharacter:Conjuration ;
              rdfs:label "Secret Chest"@en ;
              rdfs:comment "You hide a chest, and all its contents, on the Ethereal Plane. You must touch the chest and the miniature replica that serves as a material component for the spell. The chest can contain up to 12 cubic feet of nonliving material (3 feet by 2 feet by 2 feet)."@en .

DnD5eCharacter:SeeInvisibility 	a rdfs:Class ;
              rdfs:subClassOf TTRpg:Spell ;
              DnD5eCharacter:inMagicSchool DnD5eCharacter:Divination ;
              rdfs:label "See Invisibility"@en ;
              rdfs:comment "For the duration of the spell, you see invisible creatures and objects as if they were visible, and you can see through Ethereal. The ethereal objects and creatures appear ghostly translucent."@en .

DnD5eCharacter:Seeming 	a rdfs:Class ;
              rdfs:subClassOf TTRpg:Spell ;
              DnD5eCharacter:inMagicSchool DnD5eCharacter:Illusion ;
              rdfs:label "Seeming"@en ;
              rdfs:comment "This spell allows you to change the appearance of any number of creatures that you can see within range. You give each target you choose a new, illusory appearance. An unwilling target can make a charisma saving throw, and if it succeeds, it is unaffected by this spell."@en .

DnD5eCharacter:Sending 	a rdfs:Class ;
              rdfs:subClassOf TTRpg:Spell ;
              DnD5eCharacter:inMagicSchool DnD5eCharacter:Evocation ;
              rdfs:label "Sending"@en ;
              rdfs:comment "You send a short message of twenty-five words or less to a creature with which you are familiar. The creature hears the message in its mind, recognizes you as the sender if it knows you, and can answer in a like manner immediately. The spell enables creatures with Intelligence scores of at least 1 to understand the meaning of your message."@en .

DnD5eCharacter:Sequester 	a rdfs:Class ;
              rdfs:subClassOf TTRpg:Spell ;
              DnD5eCharacter:inMagicSchool DnD5eCharacter:Transmutation ;
              rdfs:label "Sequester"@en ;
              rdfs:comment "By means of this spell, a willing creature or an object can be hidden away, safe from detection for the duration. When you cast the spell and touch the target, it becomes invisible and can't be targeted by divination spells or perceived through scrying sensors created by divination spells."@en .

DnD5eCharacter:Shapechange 	a rdfs:Class ;
              rdfs:subClassOf TTRpg:Spell ;
              DnD5eCharacter:inMagicSchool DnD5eCharacter:Transmutation ;
              rdfs:label "Shapechange"@en ;
              rdfs:comment "You assume the form of a different creature for the duration. The new form can be of any creature with a challenge rating equal to your level or lower. The creature can't be a construct or an undead, and you must have seen the sort of creature at least once. You transform into an average example of that creature, one without any class levels or the Spellcasting trait."@en .

DnD5eCharacter:Shatter 	a rdfs:Class ;
              rdfs:subClassOf TTRpg:Spell ;
              DnD5eCharacter:inMagicSchool DnD5eCharacter:Evocation ;
              rdfs:label "Shatter"@en ;
              rdfs:comment "A strong resonant sound painfully intense sounds of a desired point in the range of the spell. Each creature has a sphere with a 10-foot-radius sphere centered on that point must make a constitution saving throw or it suffers 3d8 thunder damage. If successful, the damage is halved. A creature made of inorganic materials such as stone, crystal or metal, makes its saving throw with a disadvantage."@en .

DnD5eCharacter:Shield 	a rdfs:Class ;
              rdfs:subClassOf TTRpg:Spell ;
              DnD5eCharacter:inMagicSchool DnD5eCharacter:Abjuration ;
              rdfs:label "Shield"@en ;
              rdfs:comment "An invisible barrier of magical force appears and protects you. Until the start of your next turn, you have a +5 bonus to AC, including against the triggering attack, and you take no damage from magic missile."@en .

DnD5eCharacter:ShieldOfFaith 	a rdfs:Class ;
              rdfs:subClassOf TTRpg:Spell ;
              DnD5eCharacter:inMagicSchool DnD5eCharacter:Abjuration ;
              rdfs:label "Shield Of Faith"@en ;
              rdfs:comment "A shimmering field appears and surrounds a creature of your choice within range, granting it a +2 bonus to AC for the duration."@en .

DnD5eCharacter:Shillelagh 	a rdfs:Class ;
              rdfs:subClassOf TTRpg:Spell ;
              DnD5eCharacter:inMagicSchool DnD5eCharacter:Transmutation ;
              rdfs:label "Shillelagh"@en ;
              rdfs:comment "The wood of a club or a quarterstaff you are holding is imbued with nature's power. For the duration, you can use your spellcasting ability instead of Strength for the attack and damage rolls of melee attacks using that weapon, and the weapon's damage die becomes a d8. The weapon also becomes magical, if it isn't already. The spell ends if you cast it again or if you let go of the weapon."@en .

DnD5eCharacter:ShockingGrasp 	a rdfs:Class ;
              rdfs:subClassOf TTRpg:Spell ;
              DnD5eCharacter:inMagicSchool DnD5eCharacter:Evocation ;
              rdfs:label "Shocking Grasp"@en ;
              rdfs:comment "Lightning springs from your hand to deliver a shock to a creature you try to touch. Make a melee spell attack against the target. You have advantage on the attack roll if the target is wearing armor made of metal. On a hit, the target takes 1d8 lightning damage, and it can't take reactions until the start of its next turn."@en .

DnD5eCharacter:Silence 	a rdfs:Class ;
              rdfs:subClassOf TTRpg:Spell ;
              DnD5eCharacter:inMagicSchool DnD5eCharacter:Illusion ;
              rdfs:label "Silence"@en ;
              rdfs:comment "For the duration, no sound can be created within or pass through a 20-foot-radius sphere centered on a point you choose within range. Any creature or object entirely inside the sphere is immune to thunder damage, and creatures are deafened while entirely inside it."@en .

DnD5eCharacter:SilentImage 	a rdfs:Class ;
              rdfs:subClassOf TTRpg:Spell ;
              DnD5eCharacter:inMagicSchool DnD5eCharacter:Illusion ;
              rdfs:label "Silent Image"@en ;
              rdfs:comment "You create the image of an object, a creature, or some other visible phenomenon that is no larger than a 15-foot cube. The image appears at a spot within range and lasts for the duration. The image is purely visual; it isn't accompanied by sound, smell, or other sensory effects."@en .

DnD5eCharacter:Simulacrum 	a rdfs:Class ;
              rdfs:subClassOf TTRpg:Spell ;
              DnD5eCharacter:inMagicSchool DnD5eCharacter:Illusion ;
              rdfs:label "Simulacrum"@en ;
              rdfs:comment "You shape an illusory duplicate of one beast or humanoid that is within range for the entire casting time of the spell. The duplicate is a creature, partially real and formed from ice or snow, and it can take actions and otherwise be affected as a normal creature. It appears to be the same as the original, but it has half the creature's hit point maximum and is formed without any equipment. Otherwise, the illusion uses all the statistics of the creature it duplicates."@en .

DnD5eCharacter:Sleep 	a rdfs:Class ;
              rdfs:subClassOf TTRpg:Spell ;
              DnD5eCharacter:inMagicSchool DnD5eCharacter:Enchantment ;
              rdfs:label "Sleep"@en ;
              rdfs:comment "This spell sends creatures into a magical slumber. Roll 5d8; the total is how many hit points of creatures this spell can affect. Creatures within 20 feet of a point you choose within range are affected in ascending order of their current hit points (ignoring unconscious creatures)."@en .

DnD5eCharacter:SleetStorm 	a rdfs:Class ;
              rdfs:subClassOf TTRpg:Spell ;
              DnD5eCharacter:inMagicSchool DnD5eCharacter:Conjuration ;
              rdfs:label "Sleet Storm"@en ;
              rdfs:comment "Until the spell ends, freezing rain and sleet fall in a 20-foot-tall cylinder with a 40-foot radius centered on a point you choose within range. The area is heavily obscured, and exposed flames in the area are doused."@en .

DnD5eCharacter:Slow 	a rdfs:Class ;
              rdfs:subClassOf TTRpg:Spell ;
              DnD5eCharacter:inMagicSchool DnD5eCharacter:Transmutation ;
              rdfs:label "Slow"@en ;
              rdfs:comment "You alter time around up to six creatures of your choice in a 40-foot cube within range. Each target must succeed on a wisdom saving throw or be affected by this spell for the duration."@en .

DnD5eCharacter:SpareTheDying 	a rdfs:Class ;
              rdfs:subClassOf TTRpg:Spell ;
              DnD5eCharacter:inMagicSchool DnD5eCharacter:Necromancy ;
              rdfs:label "Spare The Dying"@en ;
              rdfs:comment "You touch a living creature that has 0 hit points. The creature becomes stable. This spell has no effect on undead or constructs."@en .

DnD5eCharacter:SpeakWithAnimals 	a rdfs:Class ;
              rdfs:subClassOf TTRpg:Spell ;
              DnD5eCharacter:inMagicSchool DnD5eCharacter:Divination ;
              rdfs:label "Speak With Animals"@en ;
              rdfs:comment "You gain the ability to comprehend and verbally communicate with beasts for the duration. The knowledge and awareness of many beasts is limited by their intelligence, but at a minimum, beasts can give you information about nearby locations and monsters, including whatever they can perceive or have perceived within the past day. You might be able to persuade a beast to perform a small favor for you, at the DM's discretion."@en .

DnD5eCharacter:SpeakWithDead 	a rdfs:Class ;
              rdfs:subClassOf TTRpg:Spell ;
              DnD5eCharacter:inMagicSchool DnD5eCharacter:Necromancy ;
              rdfs:label "Speak With Dead"@en ;
              rdfs:comment "You grant the semblance of life and intelligence to a corpse of your choice within range, allowing it to answer the questions you pose. The corpse must still have a mouth and can't be undead. The spell fails if the corpse was the target of this spell within the last 10 days."@en .

DnD5eCharacter:SpeakWithPlants 	a rdfs:Class ;
              rdfs:subClassOf TTRpg:Spell ;
              DnD5eCharacter:inMagicSchool DnD5eCharacter:Transmutation ;
              rdfs:label "Speak With Plants"@en ;
              rdfs:comment "You imbue plants within 30 feet of you with limited sentience and animation, giving them the ability to communicate with you and follow your simple commands. You can question plants about events in the spell's area within the past day, gaining information about creatures that have passed, weather, and other circumstances."@en .

DnD5eCharacter:SpiderClimb 	a rdfs:Class ;
              rdfs:subClassOf TTRpg:Spell ;
              DnD5eCharacter:inMagicSchool DnD5eCharacter:Transmutation ;
              rdfs:label "Spider Climb"@en ;
              rdfs:comment "Until the spell ends, one willing creature you touch gains the ability to move up, down, and across vertical surfaces and upside down along ceilings, while leaving its hands free. The target also gains a climbing speed equal to its walking speed."@en .

DnD5eCharacter:SpikeGrowth 	a rdfs:Class ;
              rdfs:subClassOf TTRpg:Spell ;
              DnD5eCharacter:inMagicSchool DnD5eCharacter:Transmutation ;
              rdfs:label "Spike Growth"@en ;
              rdfs:comment "The ground in a 20-foot radius centered on a point within range twists and sprouts hard spikes and thorns. The area becomes difficult terrain for the duration. When a creature moves into or within the area, it takes 2d4 piercing damage for every 5 feet it travels."@en .

DnD5eCharacter:SpiritGuardians 	a rdfs:Class ;
              rdfs:subClassOf TTRpg:Spell ;
              DnD5eCharacter:inMagicSchool DnD5eCharacter:Conjuration ;
              rdfs:label "Spirit Guardians"@en ;
              rdfs:comment "You call forth spirits to protect you. They flit around you to a distance of 15 feet for the duration. If you are good or neutral, their spectral form appears angelic or fey (your choice). If you are evil, they appear fiendish."@en .

DnD5eCharacter:SpiritualWeapon 	a rdfs:Class ;
              rdfs:subClassOf TTRpg:Spell ;
              DnD5eCharacter:inMagicSchool DnD5eCharacter:Evocation ;
              rdfs:label "Spiritual Weapon"@en ;
              rdfs:comment "You create a floating, spectral weapon within range that lasts for the duration or until you cast this spell again. When you cast the spell, you can make a melee spell attack against a creature within 5 feet of the weapon. On a hit, the target takes force damage equal to 1d8 + your spellcasting ability modifier."@en .

DnD5eCharacter:StinkingCloud 	a rdfs:Class ;
              rdfs:subClassOf TTRpg:Spell ;
              DnD5eCharacter:inMagicSchool DnD5eCharacter:Conjuration ;
              rdfs:label "Stinking Cloud"@en ;
              rdfs:comment "You create a 20-foot-radius sphere of yellow, nauseating gas centered on a point within range. The cloud spreads around corners, and its area is heavily obscured. The cloud lingers in the air for the duration."@en .

DnD5eCharacter:StoneShape 	a rdfs:Class ;
              rdfs:subClassOf TTRpg:Spell ;
              DnD5eCharacter:inMagicSchool DnD5eCharacter:Transmutation ;
              rdfs:label "Stone Shape"@en ;
              rdfs:comment "You touch a stone object of Medium size or smaller or a section of stone no more than 5 feet in any dimension and form it into any shape that suits your purpose. So, for example, you could shape a large rock into a weapon, idol, or coffer, or make a small passage through a wall, as long as the wall is less than 5 feet thick. You could also shape a stone door or its frame to seal the door shut. The object you create can have up to two hinges and a latch, but finer mechanical detail isn't possible."@en .

DnD5eCharacter:Stoneskin 	a rdfs:Class ;
              rdfs:subClassOf TTRpg:Spell ;
              DnD5eCharacter:inMagicSchool DnD5eCharacter:Abjuration ;
              rdfs:label "Stoneskin"@en ;
              rdfs:comment "This spell turns the flesh of a willing creature you touch as hard as stone. Until the spell ends, the target has resistance to nonmagical bludgeoning, piercing, and slashing damage."@en .

DnD5eCharacter:StormOfVengeance 	a rdfs:Class ;
              rdfs:subClassOf TTRpg:Spell ;
              DnD5eCharacter:inMagicSchool DnD5eCharacter:Conjuration ;
              rdfs:label "Storm Of Vengeance"@en ;
              rdfs:comment "A churning storm cloud forms, centered on a point you can see and spreading to a radius of 360 feet. Lightning flashes in the area, thunder booms, and strong winds roar. Each creature under the cloud (no more than 5,000 feet beneath the cloud) when it appears must make a constitution saving throw. On a failed save, a creature takes 2d6 thunder damage and becomes deafened for 5 minutes."@en .

DnD5eCharacter:Suggestion 	a rdfs:Class ;
              rdfs:subClassOf TTRpg:Spell ;
              DnD5eCharacter:inMagicSchool DnD5eCharacter:Enchantment ;
              rdfs:label "Suggestion"@en ;
              rdfs:comment "You suggest a course of activity (limited to a sentence or two) and magically influence a creature you can see within range that can hear and understand you. Creatures that can't be charmed are immune to this effect. The suggestion must be worded in such a manner as to make the course of action sound reasonable. Asking the creature to stab itself, throw itself onto a spear, immolate itself, or do some other obviously harmful act ends the spell."@en .

DnD5eCharacter:Sunbeam 	a rdfs:Class ;
              rdfs:subClassOf TTRpg:Spell ;
              DnD5eCharacter:inMagicSchool DnD5eCharacter:Evocation ;
              rdfs:label "Sunbeam"@en ;
              rdfs:comment "A beam of brilliant light flashes out from your hand in a 5-foot-wide, 60-foot-long line. Each creature in the line must make a constitution saving throw. On a failed save, a creature takes 6d8 radiant damage and is blinded until your next turn. On a successful save, it takes half as much damage and isn't blinded by this spell. Undead and oozes have disadvantage on this saving throw."@en .

DnD5eCharacter:Sunburst 	a rdfs:Class ;
              rdfs:subClassOf TTRpg:Spell ;
              DnD5eCharacter:inMagicSchool DnD5eCharacter:Evocation ;
              rdfs:label "Sunburst"@en ;
              rdfs:comment "Brilliant sunlight flashes in a 60-foot radius centered on a point you choose within range. Each creature in that light must make a constitution saving throw. On a failed save, a creature takes 12d6 radiant damage and is blinded for 1 minute. On a successful save, it takes half as much damage and isn't blinded by this spell. Undead and oozes have disadvantage on this saving throw."@en .

DnD5eCharacter:Symbol 	a rdfs:Class ;
              rdfs:subClassOf TTRpg:Spell ;
              DnD5eCharacter:inMagicSchool DnD5eCharacter:Abjuration ;
              rdfs:label "Symbol"@en ;
              rdfs:comment "When you cast this spell, you inscribe a harmful glyph either on a surface (such as a section of floor, a wall, or a table) or within an object that can be closed to conceal the glyph (such as a book, a scroll, or a treasure chest). If you choose a surface, the glyph can cover an area of the surface no larger than 10 feet in diameter. If you choose an object, that object must remain in its place; if the object is moved more than 10 feet from where you cast this spell, the glyph is broken, and the spell ends without being triggered."@en .

DnD5eCharacter:Telekinesis 	a rdfs:Class ;
              rdfs:subClassOf TTRpg:Spell ;
              DnD5eCharacter:inMagicSchool DnD5eCharacter:Transmutation ;
              rdfs:label "Telekinesis"@en ;
              rdfs:comment "You gain the ability to move or manipulate creatures or objects by thought. When you cast the spell, and as your action each round for the duration, you can exert your will on one creature or object that you can see within range, causing the appropriate effect below. You can affect the same target round after round, or choose a new one at any time. If you switch targets, the prior target is no longer affected by the spell."@en .

DnD5eCharacter:TelepathicBond 	a rdfs:Class ;
              rdfs:subClassOf TTRpg:Spell ;
              DnD5eCharacter:inMagicSchool DnD5eCharacter:Divination ;
              rdfs:label "Telepathic Bond"@en ;
              rdfs:comment "You forge a telepathic link among up to eight willing creatures of your choice within range, psychically linking each creature to all the others for the duration. Creatures with Intelligence scores of 2 or less aren't affected by this spell."@en .

DnD5eCharacter:Teleport 	a rdfs:Class ;
              rdfs:subClassOf TTRpg:Spell ;
              DnD5eCharacter:inMagicSchool DnD5eCharacter:Conjuration ;
              rdfs:label "Teleport"@en ;
              rdfs:comment "This spell instantly transports you and up to eight willing creatures of your choice that you can see within range, or a single object that you can see within range, to a destination you select. If you target an object, it must be able to fit entirely inside a 10-foot cube, and it can't be held or carried by an unwilling creature."@en .

DnD5eCharacter:TeleportationCircle 	a rdfs:Class ;
              rdfs:subClassOf TTRpg:Spell ;
              DnD5eCharacter:inMagicSchool DnD5eCharacter:Conjuration ;
              rdfs:label "Teleportation Circle"@en ;
              rdfs:comment "As you cast the spell, you draw a 10-foot-diameter circle on the ground inscribed with sigils that link your location to a permanent teleportation circle of your choice whose sigil sequence you know and that is on the same plane of existence as you. A shimmering portal opens within the circle you drew and remains open until the end of your next turn. Any creature that enters the portal instantly appears within 5 feet of the destination circle or in the nearest unoccupied space if that space is occupied."@en .

DnD5eCharacter:Thaumaturgy 	a rdfs:Class ;
              rdfs:subClassOf TTRpg:Spell ;
              DnD5eCharacter:inMagicSchool DnD5eCharacter:Transmutation ;
              rdfs:label "Thaumaturgy"@en ;
              rdfs:comment "You manifest a minor wonder, a sign of supernatural power, within range. You create one of the following magical effects within range."@en .

DnD5eCharacter:Thunderwave 	a rdfs:Class ;
              rdfs:subClassOf TTRpg:Spell ;
              DnD5eCharacter:inMagicSchool DnD5eCharacter:Evocation ;
              rdfs:label "Thunderwave"@en ;
              rdfs:comment "A wave of thunderous force sweeps out from you. Each creature in a 15-foot cube originating from you must make a constitution saving throw. On a failed save, a creature takes 2d8 thunder damage and is pushed 10 feet away from you. On a successful save, the creature takes half as much damage and isn't pushed."@en .

DnD5eCharacter:TimeStop 	a rdfs:Class ;
              rdfs:subClassOf TTRpg:Spell ;
              DnD5eCharacter:inMagicSchool DnD5eCharacter:Transmutation ;
              rdfs:label "Time Stop"@en ;
              rdfs:comment "You briefly stop the flow of time for everyone but yourself. No time passes for other creatures, while you take 1d4 + 1 turns in a row, during which you can use actions and move as normal."@en .

DnD5eCharacter:TinyHut 	a rdfs:Class ;
              rdfs:subClassOf TTRpg:Spell ;
              DnD5eCharacter:inMagicSchool DnD5eCharacter:Evocation ;
              rdfs:label "Tiny Hut"@en ;
              rdfs:comment "A 10-foot-radius immobile dome of force springs into existence around and above you and remains stationary for the duration. The spell ends if you leave its area."@en .

DnD5eCharacter:Tongues 	a rdfs:Class ;
              rdfs:subClassOf TTRpg:Spell ;
              DnD5eCharacter:inMagicSchool DnD5eCharacter:Divination ;
              rdfs:label "Tongues"@en ;
              rdfs:comment "This spell grants the creature you touch the ability to understand any spoken language it hears. Moreover, when the target speaks, any creature that knows at least one language and can hear the target understands what it says."@en .

DnD5eCharacter:TransportViaPlants 	a rdfs:Class ;
              rdfs:subClassOf TTRpg:Spell ;
              DnD5eCharacter:inMagicSchool DnD5eCharacter:Conjuration ;
              rdfs:label "Transport Via Plants"@en ;
              rdfs:comment "This spell creates a magical link between a Large or larger inanimate plant within range and another plant, at any distance, on the same plane of existence. You must have seen or touched the destination plant at least once before. For the duration, any creature can step into the target plant and exit from the destination plant by using 5 feet of movement."@en .

DnD5eCharacter:TreeStride 	a rdfs:Class ;
              rdfs:subClassOf TTRpg:Spell ;
              DnD5eCharacter:inMagicSchool DnD5eCharacter:Conjuration ;
              rdfs:label "Tree Stride"@en ;
              rdfs:comment "You gain the ability to enter a tree and move from inside it to inside another tree of the same kind within 500 feet. Both trees must be living and at least the same size as you. You must use 5 feet of movement to enter a tree. You instantly know the location of all other trees of the same kind within 500 feet and, as part of the move used to enter the tree, can either pass into one of those trees or step out of the tree you're in. You appear in a spot of your choice within 5 feet of the destination tree, using another 5 feet of movement. If you have no movement left, you appear within 5 feet of the tree you entered."@en .

DnD5eCharacter:TruePolymorph 	a rdfs:Class ;
              rdfs:subClassOf TTRpg:Spell ;
              DnD5eCharacter:inMagicSchool DnD5eCharacter:Transmutation ;
              rdfs:label "True Polymorph"@en ;
              rdfs:comment "Choose one creature or nonmagical object that you can see within range. You transform the creature into a different creature, the creature into an object, or the object into a creature (the object must be neither worn nor carried by another creature). The transformation lasts for the duration, or until the target drops to 0 hit points or dies. If you concentrate on this spell for the full duration, the transformation becomes permanent."@en .

DnD5eCharacter:TrueResurrection 	a rdfs:Class ;
              rdfs:subClassOf TTRpg:Spell ;
              DnD5eCharacter:inMagicSchool DnD5eCharacter:Necromancy ;
              rdfs:label "True Resurrection"@en ;
              rdfs:comment "You touch a creature that has been dead for no longer than 200 years and that died for any reason except old age. If the creature's soul is free and willing, the creature is restored to life with all its hit points."@en .

DnD5eCharacter:TrueSeeing 	a rdfs:Class ;
              rdfs:subClassOf TTRpg:Spell ;
              DnD5eCharacter:inMagicSchool DnD5eCharacter:Divination ;
              rdfs:label "True Seeing"@en ;
              rdfs:comment "This spell gives the willing creature you touch the ability to see things as they actually are. For the duration, the creature has truesight, notices secret doors hidden by magic, and can see into the Ethereal Plane, all out to a range of 120 feet."@en .

DnD5eCharacter:TrueStrike 	a rdfs:Class ;
              rdfs:subClassOf TTRpg:Spell ;
              DnD5eCharacter:inMagicSchool DnD5eCharacter:Divination ;
              rdfs:label "True Strike"@en ;
              rdfs:comment "You extend your hand and point a finger at a target in range. Your magic grants you a brief insight into the target's defenses. On your next turn, you gain advantage on your first attack roll against the target, provided that this spell hasn't ended."@en .

DnD5eCharacter:UnseenServant 	a rdfs:Class ;
              rdfs:subClassOf TTRpg:Spell ;
              DnD5eCharacter:inMagicSchool DnD5eCharacter:Conjuration ;
              rdfs:label "Unseen Servant"@en ;
              rdfs:comment "This spell creates an invisible, mindless, shapeless force that performs simple tasks at your command until the spell ends. The servant springs into existence in an unoccupied space on the ground within range. It has AC 10, 1 hit point, and a Strength of 2, and it can't attack. If it drops to 0 hit points, the spell ends."@en .

DnD5eCharacter:VampiricTouch 	a rdfs:Class ;
              rdfs:subClassOf TTRpg:Spell ;
              DnD5eCharacter:inMagicSchool DnD5eCharacter:Necromancy ;
              rdfs:label "Vampiric Touch"@en ;
              rdfs:comment "The touch of your shadow-wreathed hand can siphon life force from others to heal your wounds. Make a melee spell attack against a creature within your reach. On a hit, the target takes 3d6 necrotic damage, and you regain hit points equal to half the amount of necrotic damage dealt. Until the spell ends, you can make the attack again on each of your turns as an action."@en .

DnD5eCharacter:ViciousMockery 	a rdfs:Class ;
              rdfs:subClassOf TTRpg:Spell ;
              DnD5eCharacter:inMagicSchool DnD5eCharacter:Enchantment ;
              rdfs:label "Vicious Mockery"@en ;
              rdfs:comment "You unleash a string of insults laced with subtle enchantments at a creature you can see within range. If the target can hear you (though it need not understand you), it must succeed on a wisdom saving throw or take 1d4 psychic damage and have disadvantage on the next attack roll it makes before the end of its next turn."@en .

DnD5eCharacter:WallOfFire 	a rdfs:Class ;
              rdfs:subClassOf TTRpg:Spell ;
              DnD5eCharacter:inMagicSchool DnD5eCharacter:Evocation ;
              rdfs:label "Wall Of Fire"@en ;
              rdfs:comment "You create a wall of fire on a solid surface within range. You can make the wall up to 60 feet long, 20 feet high, and 1 foot thick, or a ringed wall up to 20 feet in diameter, 20 feet high, and 1 foot thick. The wall is opaque and lasts for the duration."@en .

DnD5eCharacter:WallOfForce 	a rdfs:Class ;
              rdfs:subClassOf TTRpg:Spell ;
              DnD5eCharacter:inMagicSchool DnD5eCharacter:Evocation ;
              rdfs:label "Wall Of Force"@en ;
              rdfs:comment "An invisible wall of force springs into existence at a point you choose within range. The wall appears in any orientation you choose, as a horizontal or vertical barrier or at an angle. It can be free floating or resting on a solid surface. You can form it into a hemispherical dome or a sphere with a radius of up to 10 feet, or you can shape a flat surface made up of ten 10-foot-by-10-foot panels. Each panel must be contiguous with another panel. In any form, the wall is 1/4 inch thick. It lasts for the duration. If the wall cuts through a creature's space when it appears, the creature is pushed to one side of the wall (your choice which side)."@en .

DnD5eCharacter:WallOfIce 	a rdfs:Class ;
              rdfs:subClassOf TTRpg:Spell ;
              DnD5eCharacter:inMagicSchool DnD5eCharacter:Evocation ;
              rdfs:label "Wall Of Ice"@en ;
              rdfs:comment "You create a wall of ice on a solid surface within range. You can form it into a hemispherical dome or a sphere with a radius of up to 10 feet, or you can shape a flat surface made up of ten 10-foot-square panels. Each panel must be contiguous with another panel. In any form, the wall is 1 foot thick and lasts for the duration."@en .

DnD5eCharacter:WallOfStone 	a rdfs:Class ;
              rdfs:subClassOf TTRpg:Spell ;
              DnD5eCharacter:inMagicSchool DnD5eCharacter:Evocation ;
              rdfs:label "Wall Of Stone"@en ;
              rdfs:comment "A nonmagical wall of solid stone springs into existence at a point you choose within range. The wall is 6 inches thick and is composed of ten 10-foot-by-10-foot panels. Each panel must be contiguous with at least one other panel. Alternatively, you can create 10-foot-by-20-foot panels that are only 3 inches thick."@en .

DnD5eCharacter:WallOfThorns 	a rdfs:Class ;
              rdfs:subClassOf TTRpg:Spell ;
              DnD5eCharacter:inMagicSchool DnD5eCharacter:Conjuration ;
              rdfs:label "Wall Of Thorns"@en ;
              rdfs:comment "You create a wall of tough, pliable, tangled brush bristling with needle-sharp thorns. The wall appears within range on a solid surface and lasts for the duration. You choose to make the wall up to 60 feet long, 10 feet high, and 5 feet thick or a circle that has a 20-foot diameter and is up to 20 feet high and 5 feet thick. The wall blocks line of sight."@en .

DnD5eCharacter:WardingBond 	a rdfs:Class ;
              rdfs:subClassOf TTRpg:Spell ;
              DnD5eCharacter:inMagicSchool DnD5eCharacter:Abjuration ;
              rdfs:label "Warding Bond"@en ;
              rdfs:comment "This spell wards a willing creature you touch and creates a mystic connection between you and the target until the spell ends. While the target is within 60 feet of you, it gains a +1 bonus to AC and saving throws, and it has resistance to all damage. Also, each time it takes damage, you take the same amount of damage."@en .

DnD5eCharacter:WaterBreathing 	a rdfs:Class ;
              rdfs:subClassOf TTRpg:Spell ;
              DnD5eCharacter:inMagicSchool DnD5eCharacter:Transmutation ;
              rdfs:label "Water Breathing"@en ;
              rdfs:comment "This spell gives a maximum of ten willing creatures within range and you can see, the ability to breathe underwater until the end of its term. Affected creatures also retain their normal breathing pattern."@en .

DnD5eCharacter:WaterWalk 	a rdfs:Class ;
              rdfs:subClassOf TTRpg:Spell ;
              DnD5eCharacter:inMagicSchool DnD5eCharacter:Transmutation ;
              rdfs:label "Water Walk"@en ;
              rdfs:comment "This spell grants the ability to move across any liquid surface--such as water, acid, mud, snow, quicksand, or lava--as if it were harmless solid ground (creatures crossing molten lava can still take damage from the heat). Up to ten willing creatures you can see within range gain this ability for the duration."@en .

DnD5eCharacter:Web 	a rdfs:Class ;
              rdfs:subClassOf TTRpg:Spell ;
              DnD5eCharacter:inMagicSchool DnD5eCharacter:Conjuration ;
              rdfs:label "Web"@en ;
              rdfs:comment "You conjure a mass of thick, sticky webbing at a point of your choice within range. The webs fill a 20-foot cube from that point for the duration. The webs are difficult terrain and lightly obscure their area."@en .

DnD5eCharacter:Weird 	a rdfs:Class ;
              rdfs:subClassOf TTRpg:Spell ;
              DnD5eCharacter:inMagicSchool DnD5eCharacter:Illusion ;
              rdfs:label "Weird"@en ;
              rdfs:comment "Drawing on the deepest fears of a group of creatures, you create illusory creatures in their minds, visible only to them. Each creature in a 30-foot-radius sphere centered on a point of your choice within range must make a wisdom saving throw. On a failed save, a creature becomes frightened for the duration. The illusion calls on the creature's deepest fears, manifesting its worst nightmares as an implacable threat. At the start of each of the frightened creature's turns, it must succeed on a wisdom saving throw or take 4d10 psychic damage. On a successful save, the spell ends for that creature."@en .

DnD5eCharacter:WindWalk 	a rdfs:Class ;
              rdfs:subClassOf TTRpg:Spell ;
              DnD5eCharacter:inMagicSchool DnD5eCharacter:Transmutation ;
              rdfs:label "Wind Walk"@en ;
              rdfs:comment "You and up to ten willing creatures you can see within range assume a gaseous form for the duration, appearing as wisps of cloud. While in this cloud form, a creature has a flying speed of 300 feet and has resistance to damage from nonmagical weapons. The only actions a creature can take in this form are the Dash action or to revert to its normal form. Reverting takes 1 minute, during which time a creature is incapacitated and can't move. Until the spell ends, a creature can revert to cloud form, which also requires the 1-minute transformation."@en .

DnD5eCharacter:WindWall 	a rdfs:Class ;
              rdfs:subClassOf TTRpg:Spell ;
              DnD5eCharacter:inMagicSchool DnD5eCharacter:Evocation ;
              rdfs:label "Wind Wall"@en ;
              rdfs:comment "A wall of strong wind rises from the ground at a point you choose within range. You can make the wall up to 50 feet long, 15 feet high, and 1 foot thick. You can shape the wall in any way you choose so long as it makes one continuous path along the ground. The wall lasts for the duration."@en .

DnD5eCharacter:Wish 	a rdfs:Class ;
              rdfs:subClassOf TTRpg:Spell ;
              DnD5eCharacter:inMagicSchool DnD5eCharacter:Conjuration ;
              rdfs:label "Wish"@en ;
              rdfs:comment "Wish is the mightiest spell a mortal creature can cast. By simply speaking aloud, you can alter the very foundations of reality in accord with your desires."@en .

DnD5eCharacter:WordOfRecall 	a rdfs:Class ;
              rdfs:subClassOf TTRpg:Spell ;
              DnD5eCharacter:inMagicSchool DnD5eCharacter:Conjuration ;
              rdfs:label "Word Of Recall"@en ;
              rdfs:comment "You and up to five willing creatures within 5 feet of you instantly teleport to a previously designated sanctuary. You and any creatures that teleport with you appear in the nearest unoccupied space to the spot you designated when you prepared your sanctuary (see below). If you cast this spell without first preparing a sanctuary, the spell has no effect."@en .

DnD5eCharacter:ZoneOfTruth 	a rdfs:Class ;
              rdfs:subClassOf TTRpg:Spell ;
              DnD5eCharacter:inMagicSchool DnD5eCharacter:Enchantment ;
              rdfs:label "Zone Of Truth"@en ;
              rdfs:comment "You create a magical zone that guards against deception in a 15-foot-radius sphere centered on a point of your choice within range. Until the spell ends, a creature that enters the spell's area for the first time on a turn or starts its turn there must make a Charisma saving throw. On a failed save, a creature can't speak a deliberate lie while in the radius. You know whether each creature succeeds or fails on its saving throw."@en .

##### Properties #####

DnD5eCharacter:subclassOf a rdf:Property ;
              rdfs:label "Subclass Of"@en ;
              rdfs:comment ""@en ;
              rdfs:domain DnD5eCharacter:Subclass ;
              rdfs:range DnD5eCharacter:Class .

DnD5eCharacter:subraceOf a rdf:Property ;
              rdfs:label "Subrace Of"@en ;
              rdfs:comment ""@en ;
              rdfs:domain DnD5eCharacter:Subrace ;
              rdfs:range DnD5eCharacter:Race .

DnD5eCharacter:variantOf a rdf:Property ;
              rdfs:label "Variant Of"@en ;
              rdfs:comment ""@en ;
              rdfs:domain DnD5eCharacter:Variant ;
              rdfs:range DnD5eCharacter:Race .

DnD5eCharacter:unlocksAtClassLevel a rdf:Property ;
              rdfs:label "Unlocks At Class Level"@en ;
              rdfs:comment ""@en ;
              rdfs:domain DnD5eCharacter:Subclass ;
              rdfs:range xsd:positiveInteger .

DnD5eCharacter:basedOn a rdf:Property ;
              rdfs:label "Based On"@en ;
              rdfs:comment ""@en ;
              rdfs:domain DnD5eCharacter:Skill ;
              rdfs:range DnD5eCharacter:AbilityScore .

DnD5eCharacter:chooseAmount a rdf:Property ;
              rdfs:label "Choose Amount"@en ;
              rdfs:comment ""@en ;
              rdfs:domain DnD5eCharacter:FavoredHumanoids ;
              rdfs:range xsd:positiveInteger .

DnD5eCharacter:inMagicSchool a rdf:Property ;
              rdfs:label "In Magic School"@en ;
              rdfs:comment ""@en ;
              rdfs:domain TTRpg:Spell ;
              rdfs:range DnD5eCharacter:MagicSchool .

DnD5eCharacter:type a rdf:Property ;
              rdfs:label "Type"@en ;
              rdfs:comment ""@en ;
              rdfs:domain DnD5eCharacter:Monster ;
              rdfs:range DnD5eCharacter:MonsterType .

DnD5eCharacter:proficientIn a rdf:Property ;
              rdfs:label "Proficient In"@en ;
              rdfs:comment ""@en ;
              rdfs:domain DnD5eCharacter:Proficiency ;
              rdfs:range DnD5eCharacter:Skill .

DnD5eCharacter:expertIn a rdf:Property ;
              rdfs:label "Expert In"@en ;
              rdfs:comment ""@en ;
              rdfs:domain DnD5eCharacter:Expertise ;
              rdfs:range DnD5eCharacter:Skill .

DnD5eCharacter:hasAbilityScore a rdf:Property ;
              rdfs:label "Has Ability Score"@en ;
              rdfs:comment ""@en ;
              rdfs:domain TTRpg:Character ;
              rdfs:range DnD5eCharacter:AbilityScore .

DnD5eCharacter:score a rdf:Property ;
              rdfs:label "Score"@en ;
              rdfs:comment ""@en ;
              rdfs:domain DnD5eCharacter:AbilityScore ;
              rdfs:range xsd:positiveInteger .

DnD5eCharacter:hasAlignment a rdf:Property ;
              rdfs:label "Has Alignment"@en ;
              rdfs:comment ""@en ;
              rdfs:domain TTRpg:Character ;
              rdfs:range DnD5eCharacter:Alignemnt .

DnD5eCharacter:hasBackground a rdf:Property ;
              rdfs:label "Has Background"@en ;
              rdfs:comment ""@en ;
              rdfs:domain TTRpg:Character ;
              rdfs:range DnD5eCharacter:Background .

DnD5eCharacter:hasClass a rdf:Property ;
              rdfs:label "Has Class"@en ;
              rdfs:comment ""@en ;
              rdfs:domain TTRpg:Character ;
              rdfs:range DnD5eCharacter:Class .

DnD5eCharacter:hasSubclass a rdf:Property ;
              rdfs:label "Has Subclass"@en ;
              rdfs:comment ""@en ;
              rdfs:domain TTRpg:Character ;
              rdfs:range DnD5eCharacter:Subclass .

DnD5eCharacter:isRace a rdf:Property ;
              rdfs:label "Is Race"@en ;
              rdfs:comment ""@en ;
              rdfs:domain TTRpg:Character ;
              rdfs:range DnD5eCharacter:Race .

DnD5eCharacter:hasTerrain a rdf:Property ;
              rdfs:label "Has Terrain"@en ;
              rdfs:comment ""@en ;
              rdfs:domain TTRpg:Location ;
              rdfs:range DnD5eCharacter:Terrain .

DnD5eCharacter:version a rdf:Property ;
              rdfs:label "Version"@en ;
              rdfs:comment "A property to keep track of the ontology version."@en ;
              rdfs:domain owl:Ontology ;
              rdfs:range xsd:string .
